#### Own prefixes
@base             <http://data.businessgraph.io/> .
@prefix ebg:      <http://data.businessgraph.io/ontology#> .
@prefix ebg-sem:  <http://data.businessgraph.io/ontology-sem#/> .

##### External prefixes
@prefix adms:     <http://www.w3.org/ns/adms#> .
@prefix dbo:      <http://dbpedia.org/ontology/>.
@prefix dc:       <http://purl.org/dc/elements/1.1/>.
@prefix dct:      <http://purl.org/dc/terms/> .
@prefix foaf:     <http://xmlns.com/foaf/0.1/> .
@prefix locn:     <http://www.w3.org/ns/locn#>.
@prefix ngeo:     <http://geovocab.org/geometry#> .
@prefix nuts:     <http://nuts.geovocab.org/id/>.
@prefix org:      <http://www.w3.org/ns/org#>.
@prefix owl:      <http://www.w3.org/2002/07/owl#> .
@prefix puml:     <http://plantuml.com/ontology#>.
@prefix ramon:    <http://rdfdata.eionet.europa.eu/ramon/ontology/> .
@prefix rdf:      <http://www.w3.org/1999/02/22-rdf-syntax-ns#> .
@prefix rdfs:     <http://www.w3.org/2000/01/rdf-schema#> .
@prefix rov:      <http://www.w3.org/ns/regorg#>.
@prefix schema:   <http://schema.org/> .
@prefix sioc:     <http://rdfs.org/sioc/ns#> .
@prefix skos:     <http://www.w3.org/2004/02/skos/core#> .
@prefix spatial:  <http://geovocab.org/spatial#> .
@prefix time:     <http://www.w3.org/2006/time#>.
@prefix vann:     <http://purl.org/vocab/vann/> .
@prefix void:     <http://rdfs.org/ns/void#> .
@prefix xsd:      <http://www.w3.org/2001/XMLSchema#> .
@prefix person:   <http://www.w3.org/ns/person#> .
@prefix sem:      <http://semanticweb.cs.vu.nl/2009/11/sem/> .

#### Imports
ebg-sem: a owl:Ontology ;
  owl:imports <http://data.businessgraph.io/ontology#> .

#### Ontology extension for events
sem:Event a rdfs:Class ;
  rdfs:label "Event" ;
  skos:definition "Hierarchical relationships and historical events that have occured to the organization and organizational sub-units" ;
  skos:scopeNote "Events are things that happen. This comprises everything from historical events to web site sessions and mythical journeys. In the case of Ebg model Events are things that happen to a company or a site".

ebg:hasEvent a owl:DatatypeProperty ;
  schema:domainIncludes rov:RegisteredOrganization, rov:OrganizationalUnit ;
  schema:rangeIncludes sem:Event ;
  rdfs:label "historical event" ;
  skos:definition "Historical event that has occured to the organization" .

ebg:eventValue a owl:DatatypeProperty ;
  schema:domainIncludes sem:Event ;
  schema:rangeIncludes xsd:string ;
  rdfs:label "event type value" ;
  skos:definition "Value linked to an eventType that occurs to a company or a site" ;
  skos:example "C" .

sem:eventType a owl:DatatypeProperty ;
  schema:domainIncludes sem:Event ;
  schema:rangeIncludes xsd:string ;
  rdfs:label "event type" ;
  skos:definition "Type of historical event that has occured to the organization" ;
  skos:example "change_administrative_state"@en .

sem:hasTime a owl:DatatypeProperty ;
  schema:domainIncludes sem:Event ;
  schema:rangeIncludes xsd:string ;
  rdfs:label "time of event" ;
  skos:definition "Has time is used to indicate at which time an Event took place" ;
  skos:example "2010-11-18"^^xsd:date .

ebg:isUnitOf a owl:DatatypeProperty ;
  schema:domainIncludes rov:OrganizationalUnit ;
  schema:rangeIncludes rov:RegisteredOrganization ;
  rdfs:label "is unit of organization" ;
  skos:definition "Indicates that an entity is a sub-unit of a larger organization" .

ebg:hasHQUnit a owl:DatatypeProperty ;
  schema:domainIncludes rov:RegisteredOrganization ;
  schema:rangeIncludes rov:OrganizationalUnit ;
  rdfs:label "headquarter unit" ;
  skos:definition "Indicates that an entity is a headquarter of an organization" .
