@prefix : <http://data.businessgraph.io/ontology##> .
@prefix dc: <http://purl.org/dc/elements/1.1/> .
@prefix dbo: <http://dbpedia.org/ontology/> .
@prefix dct: <http://purl.org/dc/terms/> .
@prefix ebg: <http://data.businessgraph.io/ontology#> .
@prefix lau: <http://data.businessgraph.io/lau/> .
@prefix org: <http://www.w3.org/ns/org#> .
@prefix owl: <http://www.w3.org/2002/07/owl#> .
@prefix rdf: <http://www.w3.org/1999/02/22-rdf-syntax-ns#> .
@prefix rov: <http://www.w3.org/ns/regorg#> .
@prefix xml: <http://www.w3.org/XML/1998/namespace> .
@prefix xsd: <http://www.w3.org/2001/XMLSchema#> .
@prefix adms: <http://www.w3.org/ns/adms#> .
@prefix foaf: <http://xmlns.com/foaf/0.1/> .
@prefix locn: <http://www.w3.org/ns/locn#> .
@prefix nace: <http://data.businessgraph.io/nace/> .
@prefix ngeo: <http://geovocab.org/geometry#> .
@prefix nuts: <http://nuts.geovocab.org/id/> .
@prefix puml: <http://plantuml.com/ontology#> .
@prefix rdfs: <http://www.w3.org/2000/01/rdf-schema#> .
@prefix sioc: <http://rdfs.org/sioc/ns#> .
@prefix skos: <http://www.w3.org/2004/02/skos/core#> .
@prefix time: <http://www.w3.org/2006/time#> .
@prefix vann: <http://purl.org/vocab/vann/> .
@prefix void: <http://rdfs.org/ns/void#> .
@prefix ramon: <http://rdfdata.eionet.europa.eu/ramon/ontology/> .
@prefix ebg-id: <http://data.businessgraph.io/identifier/> .
@prefix schema: <http://schema.org/> .
@prefix spatial: <http://geovocab.org/spatial#> .
@prefix ebg-comp: <http://data.businessgraph.io/company/> .
@base <http://data.businessgraph.io/ontology#> .

<http://data.businessgraph.io/ontology#> rdf:type owl:Ontology ;
                                          dct:type <http://purl.org/adms/assettype/Ontology> ;
                                          dct:modified "2018-02-21"^^xsd:date ;
                                          dct:title "euBusinessGraph ontology" ;
                                          vann:preferredNamespaceUri "http://data.businessgraph.io/ontology#" ;
                                          dct:created "2017-07-11"^^xsd:date ;
                                          rdfs:seeAlso <https://docs.google.com/document/d/1dhMOTlIOC6dOK_jksJRX0CB-GIRoiYY6fWtCnZArUhU/edit> ;
                                          foaf:homepage <http://businessgraph.io> ;
                                          dct:status <http://purl.org/adms/status/UnderDevelopment> ;
                                          vann:preferredNamespacePrefix "ebg" ;
                                          dct:publisher <http://businessgraph.io> .

#################################################################
#    Annotation properties
#################################################################

###  http://purl.org/dc/terms/created
dct:created rdf:type owl:AnnotationProperty .


###  http://purl.org/dc/terms/publisher
dct:publisher rdf:type owl:AnnotationProperty .


###  http://purl.org/dc/terms/source
dct:source rdf:type owl:AnnotationProperty .


###  http://schema.org/domainIncludes
schema:domainIncludes rdf:type owl:AnnotationProperty .


###  http://schema.org/rangeIncludes
schema:rangeIncludes rdf:type owl:AnnotationProperty .


###  http://www.w3.org/2004/02/skos/core#definition
skos:definition rdf:type owl:AnnotationProperty .


###  http://www.w3.org/2004/02/skos/core#example
skos:example rdf:type owl:AnnotationProperty .


###  http://www.w3.org/2004/02/skos/core#scopeNote
skos:scopeNote rdf:type owl:AnnotationProperty .


#################################################################
#    Datatypes
#################################################################

###  http://www.w3.org/1999/02/22-rdf-syntax-ns#langString
rdf:langString rdf:type rdfs:Datatype .


###  http://www.w3.org/2001/XMLSchema#date
xsd:date rdf:type rdfs:Datatype .


###  http://www.w3.org/2001/XMLSchema#gYear
xsd:gYear rdf:type rdfs:Datatype .


###  http://www.w3.org/2001/XMLSchema#gYearMonth
xsd:gYearMonth rdf:type rdfs:Datatype .


#################################################################
#    Object Properties
#################################################################

###  http://data.businessgraph.io/ontology#adminUnit
ebg:adminUnit rdf:type owl:ObjectProperty ;
              schema:domainIncludes locn:Address ;
              schema:rangeIncludes ebg:LAURegion ,
                                   ramon:NUTSRegion ;
              rdfs:comment "All administrative units related to an address. Union of locn:adminUnitL1..2 and ebg:adminUnitL3..6. Used for faceting by place" ;
              rdfs:isDefinedBy <http://data.businessgraph.io/ontology#> ;
              rdfs:label "Admin unit" .


###  http://data.businessgraph.io/ontology#adminUnitL3
ebg:adminUnitL3 rdf:type owl:ObjectProperty ;
                rdfs:subPropertyOf ebg:adminUnit ;
                schema:domainIncludes locn:Address ;
                schema:rangeIncludes ramon:NUTSRegion ;
                rdfs:comment "Use a valid NUTS region, e.g., “Trentino-Alto Adige/Südtirol”, taken from the Geonames hierarchy (see Section 2.1.1.10), is not a NUTS region and should be resolved to valid NUTS2." ;
                rdfs:isDefinedBy <http://data.businessgraph.io/ontology#> ;
                rdfs:label "Administrative Region" ;
                skos:definition "NUTS2 region of the address." ;
                skos:example "nuts:ITC2 Valle d'Aosta/Vallée d'Aoste" ,
                             "nuts:ITH2 Provincia Autonoma di Trento" .


###  http://data.businessgraph.io/ontology#adminUnitL4
ebg:adminUnitL4 rdf:type owl:ObjectProperty ;
                rdfs:subPropertyOf ebg:adminUnit ;
                schema:domainIncludes locn:Address ;
                schema:rangeIncludes ramon:NUTSRegion ;
                rdfs:isDefinedBy <http://data.businessgraph.io/ontology#> ;
                rdfs:label "Province" ;
                skos:definition "NUTS3 region of the address." ;
                skos:example "nuts:ITC20 Aosta" .


###  http://data.businessgraph.io/ontology#adminUnitL5
ebg:adminUnitL5 rdf:type owl:ObjectProperty ;
                rdfs:subPropertyOf ebg:adminUnit ;
                schema:domainIncludes locn:Address ;
                schema:rangeIncludes ebg:LAURegion ;
                rdfs:isDefinedBy <http://data.businessgraph.io/ontology#> ;
                rdfs:label "Municipality/Commune/Settlement" ;
                skos:definition "LAU1, LAU2 region of the address" ;
                skos:scopeNote "Some countries (e.g., Bulgaria) use both LAU1 and LAU2 levels. Others (e.g., Italy) use only LAU2" .


###  http://data.businessgraph.io/ontology#adminUnitL6
ebg:adminUnitL6 rdf:type owl:ObjectProperty ;
                rdfs:subPropertyOf ebg:adminUnit ;
                schema:domainIncludes locn:Address ;
                schema:rangeIncludes ebg:LAURegion ;
                rdfs:isDefinedBy <http://data.businessgraph.io/ontology#> ;
                rdfs:label "Municipality/Commune/Settlement" ;
                skos:definition "LAU1, LAU2 region of the address" ;
                skos:scopeNote "Some countries (e.g., Bulgaria) use both LAU1 and LAU2 levels. Others (e.g., Italy) use only LAU2" .


###  http://data.businessgraph.io/ontology#geoResolution
ebg:geoResolution rdf:type owl:ObjectProperty ;
                  schema:domainIncludes schema:GeoCoordinates ;
                  rdfs:comment """Values:

Values are taken from <resolution/L0> to <resolution/L10>""" ,
                               """● If geo coordinates are present, resolution must be present too, even if it is a guess. There is no default value.
● Values should be mapped to the <resolution/> ConceptScheme (lookup list).""" ;
                  rdfs:isDefinedBy <http://data.businessgraph.io/ontology#> ;
                  rdfs:label "Geocoordinate Resolution" ;
                  skos:definition "Resolution of a geographic coordinate location: from continent (least precise) to individual house number (most precise)" .


###  http://purl.org/dc/terms/creator
dct:creator rdf:type owl:ObjectProperty .


###  http://purl.org/dc/terms/isPartOf
dct:isPartOf rdf:type owl:ObjectProperty ;
             schema:domainIncludes adms:Identifier ;
             schema:rangeIncludes ebg:IdentifierSystem ;
             rdfs:label "identifier is part of system" ;
             skos:definition "The Identifier System this identifier is part of" .


###  http://rdfs.org/sioc/ns#feed
sioc:feed rdf:type owl:ObjectProperty ;
          schema:domainIncludes rov:RegisteredOrganization ;
          schema:rangeIncludes xsd:anyURI ;
          rdfs:label "news/blog feed" ;
          skos:definition "URL of RSS/Atom feed pertaining to the company." ;
          skos:example "http://www.comune.ancona.gov.it/ankonline/anconaentrate/feed/" .


###  http://schema.org/geo
schema:geo rdf:type owl:ObjectProperty ;
           schema:domainIncludes locn:Address ;
           schema:rangeIncludes schema:GeoCoordinates ;
           rdfs:comment "If data is integrated from several providers, we may end up with multiple coordinate pairs in that node, which will need to be resolved into one." ;
           rdfs:label "geographic coordinates" ;
           skos:definition "Geographic coordinates, eg of a geo-located address." .


###  http://schema.org/sameAs
schema:sameAs rdf:type owl:ObjectProperty .


###  http://schema.org/url
schema:url rdf:type owl:ObjectProperty .


###  http://www.w3.org/ns/adms#identifier
adms:identifier rdf:type owl:ObjectProperty ;
                schema:domainIncludes rov:RegisteredOrganization ;
                schema:rangeIncludes adms:Identifier ;
                rdfs:label "registration" ;
                skos:definition """An identifier of a company. This includes, but is not limited to:
● Direct: Identifier in some aggregated dataset, where the official ID is part of the aggregation ID. 
● Indirect: Identifier in some aggregated dataset or for a website, where the aggregation ID bears no resemblance to the official ID
● Multiple: Identifier that has a many-to-many relation with the company, i.e., a company may have several identifiers of the same kind, and the same identifier can be used by several companies.""" ;
                skos:example """Direct: EU VAT number (in those jurisdictions where it is used as the primary company identifier), BRIS ID, OCORP ID.
Indirect: 
● GLEI LEI, SDATI Atoka ID
● BG GUID 617f4edf8c154f4296efdf146513de21, which corresponds to official id 204060254 and can be used to reach the official register page for that company 
Multiple: EU VAT number in jurisdictions such as the UK (where they map n:n with companies), bank license, insurance license, license to trade dual-use goods (arms), Twitter account, Facebook account.""" .


###  http://www.w3.org/ns/locn#adminUnitL1
locn:adminUnitL1 rdf:type owl:ObjectProperty ;
                 rdfs:subPropertyOf ebg:adminUnit ;
                 schema:domainIncludes locn:Address ;
                 schema:rangeIncludes ramon:NUTSRegion ;
                 rdfs:label "Country" ;
                 skos:definition "Country of the address" ;
                 skos:example "nuts:IT (Italy)." .


###  http://www.w3.org/ns/locn#adminUnitL2
locn:adminUnitL2 rdf:type owl:ObjectProperty ;
                 rdfs:subPropertyOf ebg:adminUnit ;
                 schema:domainIncludes locn:Address ;
                 schema:rangeIncludes ramon:NUTSRegion ;
                 rdfs:label "Macroregion" ;
                 skos:definition "NUTS1 region of the address." ;
                 skos:example "nuts:ITC NORD-OVEST (Nord-est)." .


###  http://www.w3.org/ns/org#hasRegisteredSite
org:hasRegisteredSite rdf:type owl:ObjectProperty ;
                      schema:domainIncludes rov:RegisteredOrganization ;
                      schema:rangeIncludes locn:Address ;
                      rdfs:label "registered address" ;
                      skos:definition "Public legal address where legal papers can be served." ;
                      skos:scopeNote "org:hasRegisteredSite leads to a node with types org:Site and locn:Address that has self-link org:siteAddress." .


###  http://www.w3.org/ns/org#hasSite
org:hasSite rdf:type owl:ObjectProperty ;
            schema:domainIncludes rov:RegisteredOrganization ;
            schema:rangeIncludes locn:Address ;
            rdfs:label "address" ;
            skos:definition "Other address/location associated to an organisation." ;
            skos:scopeNote "org:hasSite leads to a node with types org:Site & locn:Address that has self-link org:siteAddress. org:hasRegisteredSite is declared a sub-property of org:hasSite, so querying by org:hasSite will obtain all addresses" .


###  http://www.w3.org/ns/org#siteAddress
org:siteAddress rdf:type owl:ObjectProperty ;
                schema:domainIncludes rov:RegisteredOrganization ;
                schema:rangeIncludes locn:Address ;
                rdfs:label "address" ,
                           "registered address" ;
                skos:scopeNote "org:hasRegisteredSite leads to a node with types org:Site and locn:Address that has self-link org:siteAddress" ,
                               "org:hasSite leads to a node with types org:Site & locn:Address that has self-link org:siteAddress. org:hasRegisteredSite is declared a sub-property of org:hasSite, so querying by org:hasSite will obtain all addresses" .


###  http://www.w3.org/ns/regorg#orgActivity
rov:orgActivity rdf:type owl:ObjectProperty ;
                schema:domainIncludes rov:RegisteredOrganization ;
                rdfs:comment """Each data provider must map codes that are used to established URLs as described below.
• Only the top-level classification or a detailed classification may be provided since we will establish a skos:broader hierarchy.
• There is no need for separate fields for national classifications.""" ,
                             """Values:

Values are taken from euBusinessGraph NACE RDF concept scheme .Template: nace:([A-Z]|[0-9]{2}|[0-9]{2}\\.[0-9]{1,2}). 
Rules:
● Providers must use exact codes of the specified form (dot separators, no extra spaces).
○ Or we could use a more uniform code (e.g. [A-Z]\\d{2,5}) to make submission easier, but we will need to do some segmenting on output
● Providers should drop eventual NACE National Extensions trailing digits (see Section 2.1.1.11.2.3)
● If providers find difficulties mapping to NACE, or need national levels, we should discuss this.""" ;
                rdfs:label "Economic Activity" ;
                skos:definition "Economic activity of the organization (NACE code)" ;
                skos:scopeNote "Recorded using a controlled vocabulary: EC NACE 2. More detailed national classifications could also useful (e.g. IT ATECO, UK SIC, BG NKID) but are not supported for now." .


###  http://www.w3.org/ns/regorg#orgStatus
rov:orgStatus rdf:type owl:ObjectProperty ;
              schema:domainIncludes rov:RegisteredOrganization ;
              schema:rangeIncludes skos:ConceptScheme ;
              rdfs:comment "A Best Practice for recording status levels is to use the relevant jurisdiction's terms and to encode these in a SKOS Concept Scheme. [rov:]." ;
              rdfs:label "Status" ;
              skos:definition "Flag that identifies whether a company is active or not [ebg:]. The operational and/or legal registration status of the entity [lei:]." ;
              skos:example "'Actively trading' vs 'Dormant' vs 'Unregistered' could be considered the 3 main divisions of Status." ,
                           "'Normal Activity': does appear to have cross-border usefulness and this should be used in preference to terms like 'trading' or 'operating' [rov:]." ,
                           "'insolvent', 'bankrupt', 'in receivership': likely to mean slightly different things with different legal implications in different jurisdictions [rov:]." ;
              skos:scopeNote "There is no globally accepted list of company states. For Inactive, some look at hard evidence (the company has been deregistered), others at a long period of inactivity (dormant). Because of this, a user cannot assume that Active and Inactive are opposites." .


###  http://www.w3.org/ns/regorg#orgType
rov:orgType rdf:type owl:ObjectProperty ;
            schema:domainIncludes rov:RegisteredOrganization ;
            schema:rangeIncludes skos:Concept ;
            rdfs:comment """Values:

Values are taken from code lists of data providers. Code lists of euBusinessGraph data providers were collected and published in the project repository .
Alternatively, a free text \"Type Text\" is used.""" ;
            rdfs:label "Type" ;
            skos:definition "Company Type (Legal Form of the entity)" ;
            skos:scopeNote "Each jurisdiction will have a limited set of recognized company types and these should be expressed in a consistent manner in a SKOS Concept Scheme [rov:] The types may form a hierarchy, but each company can have maximum one value. E.g. for Italy: Società Di Capitale > Società a responsabilità limitata [ebg:]" .


###  http://www.w3.org/ns/regorg#registration
rov:registration rdf:type owl:ObjectProperty ;
                 schema:domainIncludes rov:RegisteredOrganization ;
                 schema:rangeIncludes adms:Identifier ;
                 rdfs:label "official registration" ;
                 skos:definition "Identifier that holds the official company registration in its jurisdiction of registration.  It establishes the legal existence of the company." ;
                 skos:example """Companies House in the United Kingdom
Registro Imprese in Italy""" ;
                 skos:scopeNote """This property holds redundant information that is captured through the registration property. This is done for compatibility with the Registered Organization vocabulary.
In some cases, we may not have info about the official registration, though \"it is questionable whether a description of a registered organization without this property and an associated Identifier class will be of any value\" [rov:]""" .


#################################################################
#    Data properties
#################################################################

###  http://data.businessgraph.io/ontology#exclusionNote
ebg:exclusionNote rdf:type owl:DatatypeProperty ;
                  schema:domainIncludes skos:Concept ;
                  schema:rangeIncludes rdf:langString ;
                  rdfs:comment "Exclusion note of a NACE classification concept" ;
                  rdfs:isDefinedBy <http://data.businessgraph.io/ontology#> ;
                  rdfs:label "Exclusion note" .


###  http://data.businessgraph.io/ontology#identifierWebResource
ebg:identifierWebResource rdf:type owl:DatatypeProperty ;
                          schema:domainIncludes ebg:IdentifierSystem ;
                          schema:rangeIncludes xsd:string ;
                          rdfs:isDefinedBy <http://data.businessgraph.io/ontology#> ;
                          rdfs:label "Identifier Web Resource" ;
                          skos:definition "Web resource(s) associated with an identifier system that specifies templates to build URLs for all identifiers in the system." ;
                          skos:example """Web resource(s) associated with an identifier system that specifies templates to build URLs for all identifiers in the system.
For OCORP, the templates:
• \"https://opencorporates.com/companies/{}\", 
• \"https://opencorporates.com/companies/{}.xml\",
•  \"https://opencorporates.com/companies/{}.json\",
• https://opencorporates.com/companies/{}.rdf
and the identifier value return company information in \"text/html\", \"application/xml\", \"application/json\" and \"application/rdf+xml\"  respectively.""" .


###  http://data.businessgraph.io/ontology#isEnumerated
ebg:isEnumerated rdf:type owl:DatatypeProperty ;
                 schema:domainIncludes ebg:IdentifierSystem ;
                 schema:rangeIncludes xsd:boolean ;
                 rdfs:isDefinedBy <http://data.businessgraph.io/ontology#> ;
                 rdfs:label "has enumerated identifiers" ;
                 skos:definition "whether the system has an Issuer and issued identifiers are kept in a database (register)" ;
                 skos:example """• Every official register is enumerated
• Websites are not enumerated""" .


###  http://data.businessgraph.io/ontology#isImmutable
ebg:isImmutable rdf:type owl:DatatypeProperty ;
                schema:domainIncludes ebg:IdentifierSystem ;
                schema:rangeIncludes xsd:boolean ;
                rdfs:isDefinedBy <http://data.businessgraph.io/ontology#> ;
                rdfs:label "has immutable identifiers" ;
                skos:definition "whether identifiers can change" ;
                skos:example "Some registers encode additional information within the identifier (e.g., some identifiers encode the economic sector of the company). In these cases the identifier changes when the extra information that is encoded changes (see “Dumb vs. Intelligent Identifiers” in Section 3.1.2.5)." .


###  http://data.businessgraph.io/ontology#isOfficial
ebg:isOfficial rdf:type owl:DatatypeProperty ;
               schema:domainIncludes ebg:IdentifierSystem ;
               schema:rangeIncludes xsd:boolean ;
               rdfs:isDefinedBy <http://data.businessgraph.io/ontology#> ;
               rdfs:label "is official in jurisdiction" ;
               skos:definition "Whether the system is considered the official one in all jurisdictions in which it applies." ;
               skos:example """• False for Website, Twitter, Facebook in that they don't have any official status
• True for UK company house, the official register for the “GB” jurisdiction
• False for GLEI, since it is not the official register for any of the world’s jurisdictions
• False for SDATI identifiers since the SDATI system is not official in Italy.""" .


###  http://data.businessgraph.io/ontology#isPersistent
ebg:isPersistent rdf:type owl:DatatypeProperty ;
                 schema:domainIncludes ebg:IdentifierSystem ;
                 schema:rangeIncludes xsd:boolean ;
                 rdfs:isDefinedBy <http://data.businessgraph.io/ontology#> ;
                 rdfs:label "has persistent identifiers" ;
                 skos:definition "whether identifiers can be removed from the register" ;
                 skos:example "Some registers “remove” identifiers when the object they relate to is no longer active(see “Persistent Identifiers” in Section 3.1.2.8)." .


###  http://data.businessgraph.io/ontology#isPublic
ebg:isPublic rdf:type owl:DatatypeProperty ;
             schema:domainIncludes ebg:IdentifierSystem ;
             schema:rangeIncludes xsd:boolean ;
             rdfs:isDefinedBy <http://data.businessgraph.io/ontology#> ;
             rdfs:label "is public" ;
             skos:definition "whether identifiers from the system are available for public use: consulting, search or download." ;
             skos:example """• Italian (IT) company identifiers are public. Even though they are not published openly, they are available for a fee, and then can be used freely.
• DUNS identifiers are not public, even though there are limited lookup services (e.g., https://www.dnb.com/duns-number/lookup.html). Dun and Bradstreet does not allow their use en-masse.""" ;
             skos:scopeNote "Most public systems (but not all) will have some Publishers, and preferably some web resources." .


###  http://data.businessgraph.io/ontology#isPubliclyTraded
ebg:isPubliclyTraded rdf:type owl:DatatypeProperty ;
                     schema:domainIncludes rov:RegisteredOrganization ;
                     schema:rangeIncludes xsd:boolean ;
                     rdfs:isDefinedBy <http://data.businessgraph.io/ontology#> ;
                     rdfs:label "is publicly traded" ;
                     skos:definition "Whether the company is publicly traded (listed at a stock exchange) [ebg:]." .


###  http://data.businessgraph.io/ontology#isSingleValued
ebg:isSingleValued rdf:type owl:DatatypeProperty ;
                   schema:domainIncludes ebg:IdentifierSystem ;
                   schema:rangeIncludes xsd:boolean ;
                   rdfs:isDefinedBy <http://data.businessgraph.io/ontology#> ;
                   rdfs:label "is single-valued" ;
                   skos:definition "Whether each entity has only one identifier in the system" ;
                   skos:example """• Company IDs are unique in most national registers 
• Stock exchange tickers are unique to each exchange (but a company can buy the ticker of another, i.e. the identity changes over time)
• Person names are not unique since they are highly ambiguous
• Websites are not unique since a website can be shared by several related companies""" ;
                   skos:scopeNote """Similar to:
• owl:FunctionalProperty 
• Wikidata Single Value constraint""" .


###  http://data.businessgraph.io/ontology#isStartup
ebg:isStartup rdf:type owl:DatatypeProperty ;
              schema:domainIncludes rov:RegisteredOrganization ;
              schema:rangeIncludes xsd:boolean ;
              rdfs:isDefinedBy <http://data.businessgraph.io/ontology#> ;
              rdfs:label "is startup" ;
              skos:definition "Whether the company is a startup [ebg:]" ;
              skos:example """Pitch, sectors and business model of the startup and innovative SMEs registered in the special section of the Business Register
http://startup.registroimprese.it/""" .


###  http://data.businessgraph.io/ontology#isStateOwned
ebg:isStateOwned rdf:type owl:DatatypeProperty ;
                 schema:domainIncludes rov:RegisteredOrganization ;
                 schema:rangeIncludes xsd:boolean ;
                 rdfs:isDefinedBy <http://data.businessgraph.io/ontology#> ;
                 rdfs:label "is state owned" ;
                 skos:definition "Whether this organisation is owned by the government, a government agency, community, city or other public entity." ;
                 skos:example "False for Spaziodati (a private company)." ,
                              "True Autonomous Province of Trento (local government)." ,
                              "True for the Norwegian company Statkraft (Norwegian state-owned company)." ;
                 skos:scopeNote "In many cases it's not possible to compute this attribute without access to the shareholder register, so it may be missing." .


###  http://data.businessgraph.io/ontology#isUnique
ebg:isUnique rdf:type owl:DatatypeProperty ;
             schema:domainIncludes ebg:IdentifierSystem ;
             schema:rangeIncludes xsd:boolean ;
             rdfs:isDefinedBy <http://data.businessgraph.io/ontology#> ;
             rdfs:label "has unique identifiers" ;
             skos:definition "Whether each identifier in the system relates to only one entity" ;
             skos:example """• Company IDs are unique in most national registers 
• Stock exchange tickers are unique to each exchange (but a company can buy the ticker of another, i.e. the identity changes over time)
• Person names are not unique since they are highly ambiguous
• Websites are not unique since a website can be shared by several related companies""" ;
             skos:scopeNote """Similar to:
• owl:InverseFunctionalProperty 
• Wikidata Distinct Values constraint""" .


###  http://data.businessgraph.io/ontology#level
ebg:level rdf:type owl:DatatypeProperty ;
          schema:domainIncludes skos:Concept ;
          schema:rangeIncludes xsd:integer ;
          rdfs:comment "Hierarchical level of a thesaurus concept" ;
          rdfs:isDefinedBy <http://data.businessgraph.io/ontology#> ;
          rdfs:label "Level" .


###  http://data.businessgraph.io/ontology#order
ebg:order rdf:type owl:DatatypeProperty ;
          schema:domainIncludes skos:Concept ;
          schema:rangeIncludes xsd:integer ;
          rdfs:comment "Global order of a thesaurus concept respecting the hierarchical structure (depth-first traversal)" ;
          rdfs:isDefinedBy <http://data.businessgraph.io/ontology#> ;
          rdfs:label "Order" .


###  http://data.businessgraph.io/ontology#orgActivityText
ebg:orgActivityText rdf:type owl:DatatypeProperty ;
                    schema:domainIncludes rov:RegisteredOrganization ;
                    schema:rangeIncludes rdf:langString ;
                    rdfs:isDefinedBy <http://data.businessgraph.io/ontology#> ;
                    rdfs:label "economic activity text" ;
                    skos:definition "Economic activity of the organization (free text)" ;
                    skos:scopeNote """Such field is widely used in some countries (e.g. BG) and may include much richer info, e.g.:
● NACE = 72.19 Scientific research and development in the field of natural, medical, agricultural and technical sciences, without biotechnology
● Free text = Development, exploration and production of opto-electronic systems for analogue and digital holographic recording, interferometric measurement of mechanical characteristics and biological objects at micro and macro level, refractometers, light-sensitive materials for holographic recording, blueprints of museum exhibits, artworks and collection surveys, production of holographic illustrations for students, albums, advertising, souvenirs and others, design and manufacture of holographic optical elements with a wide spectrum of applications, marketing and sale of holographic products, consulting, training and promotion of holographic methods and technologies, mediation, brokerage, and any other activity not prohibited by Bulgarian legislation.""" .


###  http://data.businessgraph.io/ontology#orgStatusText
ebg:orgStatusText rdf:type owl:DatatypeProperty ;
                  schema:domainIncludes rov:RegisteredOrganization ;
                  schema:rangeIncludes rdf:langString ;
                  rdfs:comment """● Include valid language tag (see [iana:] for list)
● If both Status and Status Text are present, they must express compatible values (Status Text will be a finer-granularity value)""" ;
                  rdfs:isDefinedBy <http://data.businessgraph.io/ontology#> ;
                  rdfs:label "status text" ;
                  skos:definition "Company status as it comes from the original register." ;
                  skos:example "Dissolved"@en ,
                               "En Liquidacion"@es ,
                               "Inactive"@en ,
                               "Revoked"@en ,
                               "Situation Normale"@fr ,
                               "Πτώχευση"@el .


###  http://data.businessgraph.io/ontology#orgTypeText
ebg:orgTypeText rdf:type owl:DatatypeProperty ;
                schema:domainIncludes rov:RegisteredOrganization ;
                schema:rangeIncludes rdf:langString ;
                rdfs:comment """Include valid language tag (see [iana:] for list)
If Type is also present, it must express the same value as Type Text.""" ;
                rdfs:isDefinedBy <http://data.businessgraph.io/ontology#> ;
                rdfs:label "type text" ;
                skos:definition "Company Type (Legal Form of the entity) given in the form of free text." ;
                skos:example "Private Limited Company"@en ,
                             "Società a responsabilità limitata"@it ,
                             "Дружество с ограничена отговорност"@bg ;
                skos:scopeNote "Because of the difficulties of standardizing Type lookup, we include a free text field." .


###  http://data.businessgraph.io/ontology#ralCode
ebg:ralCode rdf:type owl:DatatypeProperty ;
            schema:domainIncludes ebg:IdentifierSystem ;
            schema:rangeIncludes xsd:string ;
            rdfs:isDefinedBy <http://data.businessgraph.io/ontology#> ;
            rdfs:label "identifier system RAL code" ;
            skos:definition "GLEI RAL code for the identifier system." ;
            skos:scopeNote "Used only for official registers." .


###  http://data.businessgraph.io/ontology#replacementPattern
ebg:replacementPattern rdf:type owl:DatatypeProperty ;
                       schema:domainIncludes ebg:IdentifierSystem ;
                       schema:rangeIncludes xsd:string ;
                       rdfs:isDefinedBy <http://data.businessgraph.io/ontology#> ;
                       rdfs:label "Replacement Pattern" ;
                       skos:definition "Pattern to use together with the Validation Regex to normalise identifier values by removing optional decorations" ;
                       skos:example "\"$1$2$3\" can be used together with the validationRegex \"(\\d{2})-?(\\d{3})-?(\\d{4})\" to extract the pure digits from a DUNS number spelled with optional dashes (e.g. \"36-032-1459\" -> \"360321459\")" .


###  http://data.businessgraph.io/ontology#validationRegex
ebg:validationRegex rdf:type owl:DatatypeProperty ;
                    schema:domainIncludes ebg:IdentifierSystem ;
                    schema:rangeIncludes xsd:string ;
                    rdfs:isDefinedBy <http://data.businessgraph.io/ontology#> ;
                    rdfs:label "Validation Regex" ;
                    skos:definition "Regular expression for validating identifier values within the system" ;
                    skos:example """• \"([A-Z]{2})/(\\d+)\" is a regex for the EU Value Added Tax (VIES) register, which consists of a member state code followed by slash and a national numeric identifier
• \"\\d{9}\" is a simple regex for validating DUNS numbers
• \"(\\d{2})-?(\\d{3})-?(\\d{4})\" is a regex for validating DUNS numbers that may include optional dashes in the indicated positions (e.g. \"36-032-1459\")""" .


###  http://data.businessgraph.io/ontology#validationRule
ebg:validationRule rdf:type owl:DatatypeProperty ;
                   schema:domainIncludes ebg:IdentifierSystem ;
                   schema:rangeIncludes xsd:anyURI ;
                   rdfs:isDefinedBy <http://data.businessgraph.io/ontology#> ;
                   rdfs:label "Validation Rule" ;
                   skos:definition "URL providing human or machine-readable rule(s) for validating identifiers in the system" ;
                   skos:example """• http://bsv-bg.com/контролни-цифри-ползвани-в-българия/ describes the BG EIK checksum algorithm in HTML
• http://www.nsi.bg/sites/default/files/konkursi/RGP_OPAK_2014_Annex_6.pdf describes the BG EIK checksum algorithm in PDF. It is by an official source, but is less convenient""" ;
                   skos:scopeNote "Can be in the form of webpage, PDF document, RDF shape, etc. Multiple values about the same validation rule are ok." .


###  http://data.businessgraph.io/ontology#webResource
ebg:webResource rdf:type owl:DatatypeProperty ;
                schema:domainIncludes ebg:IdentifierSystem ;
                schema:rangeIncludes xsd:string ;
                rdfs:isDefinedBy <http://data.businessgraph.io/ontology#> ;
                rdfs:label "Identifier System Web Resource" ;
                skos:definition "Web resource(s) associated with an identifier system." ;
                skos:example """For BG TR:
• https://brra.bg is the homepage.
• http://opendata.government.bg/dataset/tbprobckn-pernctbp is the open data download endpoint.
For BE Banque-Carrefour des Entreprises, https://kbopub.economie.fgov.be/kbopub/zoeknummerform.html is the search URL.""" .


###  http://dbpedia.org/ontology/jurisdiction
dbo:jurisdiction rdf:type owl:DatatypeProperty ;
                 schema:domainIncludes ebg:IdentifierSystem ,
                                       rov:RegisteredOrganization ;
                 schema:rangeIncludes xsd:string ;
                 rdfs:label "Jurisdiction" ,
                            "identifier system jurisdiction" ;
                 skos:definition "Jurisdiction in which the company is registered. For Europe, this is a country, even for Germany that has 166 separate registers (see Registration Authorities List).  Many jurisdictions register foreign companies that are incorporated and fully owned in another country. EBG collects all registrations from each register and doesn't attempt to match foreign companies across jurisdictions." ,
                                 "Jurisdiction to which the identifier system applies." ;
                 skos:example "BG has many types, including a number of European companies." ,
                              """Consider the following cases:
• Website, Twitter, Facebook don't apply to any particular jurisdiction in that they don't have any official status
• UK company number applies to jurisdiction \"GB\"
• GLEI applies to the \"INT\" (world-wide) jurisdiction""" ,
                              "NO has type NUF 'Norskregistrert utenlandsk foretak'." ,
                              """“IT”, “FR”
Values are ISO 3166 country codes""" ;
                 skos:scopeNote "If we know the official legal ID of the company, the jurisdiction code and legal ID are used to form the company URI" .


###  http://purl.org/dc/terms/creator
dct:creator rdf:type owl:DatatypeProperty .


###  http://purl.org/dc/terms/issued
dct:issued rdf:type owl:DatatypeProperty ;
           schema:domainIncludes adms:Identifier ;
           schema:rangeIncludes xsd:date ;
           rdfs:label "identifier has start" ;
           skos:definition "When was the identifier issued." ;
           skos:scopeNote "This may or may not be the same as the incorporation date of the company. Even for the official registration, the two dates may differ, depending on business rules." .


###  http://rdfdata.eionet.europa.eu/ramon/ontology/code
ramon:code rdf:type owl:DatatypeProperty ;
           schema:domainIncludes ebg:LAURegion ,
                                 ramon:NUTSRegion ;
           schema:rangeIncludes xsd:string ;
           rdfs:comment "NUTS/LAU Code of an administrative region" ;
           rdfs:label "Code" .


###  http://rdfdata.eionet.europa.eu/ramon/ontology/level
ramon:level rdf:type owl:DatatypeProperty ;
            schema:domainIncludes ebg:LAURegion ,
                                  ramon:NUTSRegion ;
            schema:rangeIncludes xsd:integer ;
            rdfs:comment "Level of an administrative region: NUTS1..3=1..3, LAU1..2=4..5" ;
            rdfs:label "Level" .


###  http://rdfdata.eionet.europa.eu/ramon/ontology/name
ramon:name rdf:type owl:DatatypeProperty ;
           schema:domainIncludes ebg:LAURegion ,
                                 ramon:NUTSRegion ;
           schema:rangeIncludes rdfs:langString ;
           rdfs:comment "Name of an administrative region or settlement" ;
           rdfs:label "Name" .


###  http://schema.org/author
schema:author rdf:type owl:DatatypeProperty ;
              schema:domainIncludes ebg:IdentifierSystem ;
              schema:rangeIncludes xsd:anyURI ;
              rdfs:label "Identifier System Author" ;
              skos:definition "Agent who specified the rules and organisation of the system" ;
              skos:example """• W3C specified web URL rules 
• GLEIF specified GLEI
• Dun and Bradstreet specified DUNS numbers""" .


###  http://schema.org/availableLanguages
schema:availableLanguages rdf:type owl:DatatypeProperty ;
                          schema:domainIncludes rov:RegisteredOrganization ;
                          schema:rangeIncludes xsd:string ;
                          rdfs:label "web languages" ;
                          skos:definition "Languages used in web resources related to the organisation (e.g., corporate websites, social network accounts, etc.)." ;
                          skos:example "Values from ISO 639-1 code list, optionally followed by the country code (as for zh-CN)." ;
                          skos:scopeNote "Currently this data is provided by SDATI, for matching company entities only." .


###  http://schema.org/dissolutionDate
schema:dissolutionDate rdf:type owl:DatatypeProperty ;
                       schema:domainIncludes rov:RegisteredOrganization ;
                       schema:rangeIncludes xsd:date ;
                       rdfs:label "dissolution date" ;
                       skos:definition "Date entity was dissolved or removed from register." ;
                       skos:example "\"2014-03-22\"" .


###  http://schema.org/email
schema:email rdf:type owl:DatatypeProperty ;
             schema:domainIncludes rov:RegisteredOrganization ;
             schema:rangeIncludes rdfs:Literal ;
             rdfs:label "certified email address" ;
             skos:definition "Email that is officially registered and with the same validity as certified (snail) mail." ;
             skos:example <mailto:elettorale@pec.comune.trento.it> ;
             skos:scopeNote "euBusinessGraph does not record other company emails, so there is no need to distinguish between different types." .


###  http://schema.org/expires
schema:expires rdf:type owl:DatatypeProperty ;
               schema:domainIncludes adms:Identifier ;
               schema:rangeIncludes xsd:date ;
               rdfs:label "identifier has end" ;
               skos:definition "Date when the identifier expires" ;
               skos:scopeNote "This may or may not be the same as the dissolution date of the company. Even when it is about the official registration, the two dates may differ, depending on business rules." .


###  http://schema.org/foundingDate
schema:foundingDate rdf:type owl:DatatypeProperty ;
                    schema:domainIncludes rov:RegisteredOrganization ;
                    schema:rangeIncludes xsd:date ;
                    rdfs:label "incorporation date" ;
                    skos:definition "Date legal entity was created." ;
                    skos:example "\"2010-11-18\"" .


###  http://schema.org/latitude
schema:latitude rdf:type owl:DatatypeProperty ;
                schema:domainIncludes schema:GeoCoordinates ;
                schema:rangeIncludes xsd:decimal ;
                rdfs:comment """● Coordinates must be expressed in the WGS 84 system
● If no coordinates available, do not make a schema:GeoCoordinates node""" ;
                rdfs:label "latitude" ;
                skos:example "(“51.477811\", \"-0.001475”)" .


###  http://schema.org/license
schema:license rdf:type owl:DatatypeProperty ;
               schema:domainIncludes ebg:IdentifierSystem ;
               schema:rangeIncludes xsd:anyURI ;
               rdfs:label "identifier system license" ;
               skos:definition "License that applies to the system" ;
               skos:scopeNote "If possible, use established license URLs, e.g. from https://creativecommons.org/ or http://rightsstatements.org/" .


###  http://schema.org/longitude
schema:longitude rdf:type owl:DatatypeProperty ;
                 schema:domainIncludes schema:GeoCoordinates ;
                 schema:rangeIncludes xsd:decimal ;
                 rdfs:comment """● Coordinates must be expressed in the WGS 84 system
● If no coordinates available, do not make a schema:GeoCoordinates node""" ;
                 rdfs:label "longitude" ;
                 skos:example "(“51.477811\", \"-0.001475”)" .


###  http://schema.org/publisher
schema:publisher rdf:type owl:DatatypeProperty ;
                 schema:domainIncludes ebg:IdentifierSystem ;
                 schema:rangeIncludes xsd:anyURI ;
                 rdfs:label "Identifier System Publisher" ;
                 skos:definition "Agent that publishes the identifier database (register) in some form (i.e., printed form, online)" ;
                 skos:example """• GLEIF publishes the GLEI openly, with a full dump that is updated regularly, which has spurned re-publishers such as http://openleis.com/ and http://glei.info.
• Companies House and BRC publish the UK and NO registers openly.
• DUNS numbers are not openly published.""" ;
                 skos:scopeNote "Different functions and distributions can be considered (e.g. search or other query, per-company web resources, full download). Often but not always the issuer is also publisher." .


###  http://schema.org/sameAs
schema:sameAs rdf:type owl:DatatypeProperty .


###  http://schema.org/url
schema:url rdf:type owl:DatatypeProperty ;
           rdfs:subPropertyOf schema:url .


###  http://www.w3.org/2004/02/skos/core#altLabel
skos:altLabel rdf:type owl:DatatypeProperty ;
              schema:domainIncludes rov:RegisteredOrganization ;
              schema:rangeIncludes rdf:langString ,
                                   xsd:string ;
              rdfs:comment """Do not emit such name if it is equal to the legal name [ebg:]. 
Do not use this property to record translations of the primary legal name [rov:]. 
Provide a valid language tag if possible (see [iana:] for a list).
Don't allow leading, trailing and two consecutive spaces.""" ;
              rdfs:label "Trade name" ;
              skos:definition "Informal/popular name of the company (also called Trading As) [ebg:]" ;
              skos:example """\"PROGIENE 2.000 I PROFESSIONISTI DELL'IGIENE SRL\"@it
\"OpenCorporates\"@en
cf. to the first two examples of Legal Name""" ,
                           "OpenCorporates"@en ,
                           "PROGIENE 2.000 I PROFESSIONISTI DELL'IGIENE SRL"@it ;
              skos:scopeNote "Sometimes (e.g., when the legal name is very long) people refer to a company using a different, informal version [ebg:]. Some jurisdictions recognize concepts such as a trading name or alternative forms of a legal entity's name [rov:]." .


###  http://www.w3.org/2004/02/skos/core#notation
skos:notation rdf:type owl:DatatypeProperty ;
              schema:domainIncludes ebg:IdentifierSystem ,
                                    adms:Identifier ;
              schema:rangeIncludes rdfs:Literal ,
                                   xsd:string ;
              rdfs:comment "Should not include leading, trailing and consecutive spaces, to facilitate exact match." ;
              rdfs:label "identifier system code" ,
                         "identifier value" ;
              skos:definition "Literal value of the identifier." ,
                              "Short mnemonic code for the identifier system, used in its URL. Also used in identifier URLs that are part of the system." ;
              skos:scopeNote """Issued locally by EBG.
For identifier systems published by the sole or preferred official register in a jurisdiction, we use the jurisdiction code (e.g. \"BG\", \"GB\"). For others, if the identifier system has no explicit name, we use a short mnemonic code of the publisher: upper-case for company registers (e.g. \"OCORP\", \"SDATI\", \"RAL\", \"EU\", \"BRIS\"), mixed-case for social network registers (e.g. \"Twitter\", \"Facebook\").""" ,
                             "Should not include leading, trailing and consecutive spaces, to facilitate exact match." ,
                             """adms:Identifier recommends that this value should be \"datatyped with the identifier scheme (including the version number if appropriate)\". However, we decided not to do this because:
● One cannot search by exact literal value unless one also knows the datatype URL
● Currently we do not plan to maintain different identifier system versions""" .


###  http://www.w3.org/2004/02/skos/core#prefLabel
skos:prefLabel rdf:type owl:DatatypeProperty ;
               schema:domainIncludes ebg:IdentifierSystem ,
                                     rov:RegisteredOrganization ;
               schema:rangeIncludes rdf:langString ,
                                    rdfs:Literal ,
                                    xsd:string ;
               rdfs:label "identifier system name" ,
                          "preferred name" ;
               skos:definition "A single preferred name of a company or register (preferably English)." ,
                               "The name of the identifier system" ;
               skos:scopeNote "Used as a display name of the company or register. For companies we usually pick one of the Registered Names (English if present, else at random). For registers, we use a commonly used English name." .


###  http://www.w3.org/ns/locn#addressArea
locn:addressArea rdf:type owl:DatatypeProperty ;
                 schema:domainIncludes locn:Address ;
                 schema:rangeIncludes rdf:langString ,
                                      xsd:string ;
                 rdfs:label "neighbourhood/quarter" ;
                 skos:definition "Part of a city, village or neighborhood." ;
                 skos:scopeNote "Not likely to appear, but we have Coordinate Resolution corresponding to this field." .


###  http://www.w3.org/ns/locn#fullAddress
locn:fullAddress rdf:type owl:DatatypeProperty ;
                 schema:domainIncludes locn:Address ;
                 schema:rangeIncludes rdf:langString ,
                                      xsd:string ;
                 rdfs:label "full address" ;
                 skos:definition "Full address, free text." ;
                 skos:example "Aston House, Cornwall Avenue, London N3 1LF, UK" ,
                              "Via Belenzani 19, 38122, Trento" .


###  http://www.w3.org/ns/locn#locatorDesignator
locn:locatorDesignator rdf:type owl:DatatypeProperty ;
                       schema:domainIncludes locn:Address ;
                       schema:rangeIncludes xsd:string ;
                       rdfs:label "street number" ;
                       skos:definition "Street number and/or building name." ;
                       skos:example "47A" ,
                                    "Polygraphia Office Center, floor 4" ;
                       skos:scopeNote "Not likely to appear separately, but we have Coordinate resolution corresponding to this field." .


###  http://www.w3.org/ns/locn#poBox
locn:poBox rdf:type owl:DatatypeProperty ;
           schema:domainIncludes locn:Address ;
           schema:rangeIncludes xsd:string ;
           rdfs:label "postal office box" ;
           skos:definition "Some addresses are associated with a PO box instead of a street address." .


###  http://www.w3.org/ns/locn#postCode
locn:postCode rdf:type owl:DatatypeProperty ;
              schema:domainIncludes locn:Address ;
              schema:rangeIncludes xsd:string ;
              rdfs:label "Postal code" ;
              skos:definition "Postal code of the address." ;
              skos:scopeNote "If possible, a European postal code should correspond to the fixed values given in NUTS Downloads, so we can correlate it to a NUTS region." .


###  http://www.w3.org/ns/locn#postName
locn:postName rdf:type owl:DatatypeProperty ;
              schema:domainIncludes locn:Address ;
              schema:rangeIncludes rdf:langString ,
                                   xsd:string ;
              rdfs:comment """● Provide a language tag if possible
● If both ebg:adminUnitL6 and locn:postName are specified, they should correspond to each other""" ;
              rdfs:label "locality/city/settlement" ;
              skos:definition "Locality/City/Settlement of the address, free text." ;
              skos:example "Trento"@it ,
                           "Тренто"@bg .


###  http://www.w3.org/ns/locn#throughfare
locn:throughfare rdf:type owl:DatatypeProperty ;
                 schema:domainIncludes locn:Address ;
                 schema:rangeIncludes rdf:langString ,
                                      xsd:string ;
                 rdfs:label "street address" ;
                 skos:definition "Street name (and optionally number)." ;
                 skos:example "Polygraphia Office Center, floor 4 \\n 47A Tsarigradsko Shosse" ,
                              "Via Belenzani 19" ;
                 skos:scopeNote "It is ok if the street number is also here, because many systems do not enter the number separately. There may be several concatenated lines, separated with newlines (\\n)" .


###  http://www.w3.org/ns/regorg#legalName
rov:legalName rdf:type owl:DatatypeProperty ;
              schema:domainIncludes rov:RegisteredOrganization ;
              schema:rangeIncludes rdf:langString ;
              rdfs:comment "Provide a legal language tag (see [iana:] for a list) if possible. Don't allow leading, trailing and two consecutive spaces" ;
              rdfs:label "legal name" ;
              skos:definition "The legal name of the business, i.e. official name of the company [ebg:]" ;
              skos:example "CHRINON LTD" ,
                           "Ontotext"@en ,
                           "PROGIENE 2.000 I PROFESSIONISTI DELL'IGIENE S.R.L. ENUNCIABILE ANCHE: PROGIENE 2.000 S.R.L."@it ,
                           "Онтотекст"@bg ;
              skos:scopeNote "A business may have more than one legal name, particularly in jurisdictions with more than one official language (e.g. Belgium). Some registries also treat a transliterated name as official (e.g. Онтотекст vs Ontotext) [ebg:]" .


#################################################################
#    Classes
#################################################################

###  http://data.businessgraph.io/ontology#IdentifierSystem
ebg:IdentifierSystem rdf:type owl:Class ;
                     rdfs:label "Identifier System" ;
                     skos:definition "A system managed by a publisher (e.g., a register or agency) that is used to issue identifiers to companies." ;
                     skos:scopeNote """Many registers keep several identifier systems, e.g. http://www.registryagency.bg keeps the systems used by:
● The Trade Register http://brra.bg for companies, 
● The Bulstat Register http://www.bulstat.bg/ for other entities""" .


###  http://data.businessgraph.io/ontology#LAURegion
ebg:LAURegion rdf:type owl:Class ;
              dct:source <http://ec.europa.eu/eurostat/web/nuts/national-structures-eu> ,
                         <http://ec.europa.eu/eurostat/web/nuts/correspondence-tables/national-structures-non-eu> ;
              rdfs:comment "Local Administrative Unit" ;
              rdfs:isDefinedBy <http://data.businessgraph.io/ontology#> ;
              rdfs:label "LAU Region" ;
              skos:example """---- LAU1:
BG: Общини (Obshtini)
CH: Bezirke Districts Disretti
CY: Επαρχίες (Eparchies)
CZ: Okresy
DE: Verwaltungs- gemeinschaften
DK: Kommuner
EE: Maakond
EL: Δήμοι, Κοινότητες (Demoi, Koinotites)
FI: Seutukunnat / Ekonomiska regioner
FR: Cantons de rattachement
HU: Statisztikai kistérségek
IE: Counties, Cities
IS: Landsvædi
LI: Landschaften
LT: Savivaldybės
LU: Cantons
ME: Општине (Opštine)
MK: Општини (Opštini)
MT: Distretti
NO: Økonomiske regioner
PL: Powiaty i miasta na prawach powiatu
PT: Concelhos - Munícipios
SI: Upravne enote
SK: Okresy
TR: Ilceler
UK: Lower tier authorities (districts) or individual unitary authorities;  Individual unitary authorities or LECs (or parts thereof); Districts""" ,
                           """---- LAU2:
AL: Bashki / Komunë
AT: Gemeinden
BE: Gemeenten / Communes
BG: Населени места (Naseleni mesta)
CH: Gemeinden Communes Comuni
CY: Δήμοι, Κοινότητες (Dimoi, koinotites)
CZ: Obce
DE: Gemeinden
DK: Sogne
EE: Linn, vald
EL: Δημοτικές / Τοπικές Κοινότητες (Dimotikes / Topikes Koinotites - Municipal  / Local Communes)
ES: Municipios
FI: Kunnat / Kommuner
FR: Communes
HR: Gradovi i općine
HU: Települések
IE: Electoral Districts
IS: Sveitarfélög
IT: Comuni
LI: Gemeinden
LT: Seniūnijos
LU: Communes
LV: Republikas pilsētas, novadi
ME: Насеља (Naselja)
MK: Населени места (Naseleni mesta)
MT: Kunsilli
NL: Gemeenten
NO: Kommuner
PL: Gminy
PT: Freguesias
RO: Comuni + Municipiu + Orase
SE: Kommuner
SI: Občine
SK: Obce
TR: Köy
UK: Wards (or parts thereof)""" .


###  http://rdfdata.eionet.europa.eu/ramon/ontology/NUTSRegion
ramon:NUTSRegion rdf:type owl:Class ;
                 rdfs:label "NUTS Region" .


###  http://rdfs.org/ns/void#Dataset
void:Dataset rdf:type owl:Class .


###  http://schema.org/GeoCoordinates
schema:GeoCoordinates rdf:type owl:Class ;
                      rdfs:label "Geographic Coordinates" ;
                      skos:definition "Geographic coordinates" .


###  http://schema.org/Organization
schema:Organization rdf:type owl:Class .


###  http://schema.org/Person
schema:Person rdf:type owl:Class .


###  http://www.w3.org/2004/02/skos/core#Concept
skos:Concept rdf:type owl:Class .


###  http://www.w3.org/2004/02/skos/core#ConceptScheme
skos:ConceptScheme rdf:type owl:Class .


###  http://www.w3.org/ns/adms#Identifier
adms:Identifier rdf:type owl:Class ;
                rdfs:label "Identifier" ;
                skos:definition "Identifier of a company according to some identifier system." .


###  http://www.w3.org/ns/locn#Address
locn:Address rdf:type owl:Class ;
             rdfs:comment "Every data provider should strive to provide NUTS3 for each address. This can be done in cooperation, using the techniques described in Address Calculations above." ;
             rdfs:label "Address" ;
             skos:definition "Mailing or physical address of the company" ;
             skos:scopeNote "When used for company, should be linked as registered address (one) or other address (multiple)." .


###  http://www.w3.org/ns/org#Site
org:Site rdf:type owl:Class ;
         rdfs:comment "Every data provider should strive to provide NUTS3 for each address. This can be done in cooperation, using the techniques described in Address Calculations above." ;
         rdfs:label "Address" ;
         skos:definition "Mailing or physical address of the company" ;
         skos:scopeNote "When used for company, should be linked as registered address (one) or other address (multiple)." .


###  http://www.w3.org/ns/regorg#RegisteredOrganization
rov:RegisteredOrganization rdf:type owl:Class ;
                           rdfs:label "Company" ;
                           skos:definition "An organization that gains legal entity status by the act of registration. Compare to org:FormalOrganization that applies to any legal entity, including those created by other legal means. Registered organizations are distinct from the broader concept of organizations, groups or, in some jurisdictions, sole traders. Many organizations exist that are not legal entities yet to the outside world they have staff, hierarchies, locations etc. Other organizations exist that are an umbrella for several legal entities (universities are often good examples of this) [rov:].  A legal person or structure that is organized under the laws of any jurisdiction [lei-elf:]." ;
                           skos:example "All entities listed on an exchange." ,
                                        "All entities that issue equity, debt or other securities for other capital structures." ,
                                        "All entities that trade stock or debt, investment vehicles, including mutual funds, pension funds and alternative investment vehicles constituted as corporate entities or collective investment agreements (including umbrella funds as well as funds under an umbrella structure, hedge funds, private equity funds, etc.)." ,
                                        "All entities under the purview of a financial regulator and their affiliates, subsidiaries and holding companies." ,
                                        "All financial intermediaries." ,
                                        "Banks and finance companies." ,
                                        "Counterparties to financial transactions." ;
                           skos:scopeNote "Registered organizations are the main entities that euBusinessGraph works with (the project is not concerned with unregistered informal groups). The borderline between public organizations and commercial companies is not always clear-cut (a company may be partially owned by government, and e.g.  Public-Private-Partnerships are a prime example), so the project may deal with some organizations that are not companies. But for brevity and convenience we often call them Companies. [ebg:]" .


#################################################################
#    Individuals
#################################################################

###  http://businessgraph.io
<http://businessgraph.io> rdf:type owl:NamedIndividual .


###  http://ontotext.com
<http://ontotext.com> rdf:type owl:NamedIndividual .


###  http://data.businessgraph.io/lau/
lau: rdf:type owl:NamedIndividual ,
              void:Dataset ;
     dct:creator <http://businessgraph.io> ;
     dct:issued "2017-07-28"^^xsd:date ;
     dct:created "2017-07-28"^^xsd:date ;
     dct:publisher <http://businessgraph.io> ;
     dct:source <http://ec.europa.eu/eurostat/web/nuts/local-administrative-units> ;
     rdfs:comment "Local Administrative Units" ;
     rdfs:isDefinedBy <http://data.businessgraph.io/ontology#> ;
     rdfs:label "LAU Regions" .


###  http://data.businessgraph.io/nace/
nace: rdf:type owl:NamedIndividual ,
               skos:ConceptScheme ;
      dct:creator <http://businessgraph.io> ;
      dct:issued "2017-07-28"^^xsd:date ;
      dct:created "2017-07-28"^^xsd:date ;
      dct:publisher <http://businessgraph.io> ;
      dct:source <http://ec.europa.eu/eurostat/ramon/nomenclatures/index.cfm?TargetUrl=LST_CLS_DLD&StrNom=NACE_REV2&StrLanguageCode=EN&StrLayoutCode=HIERARCHIC#> ;
      rdfs:comment "Statistical Classification of Economic Activities in the European Community, Rev. 2 (2008)" ;
      rdfs:isDefinedBy <http://data.businessgraph.io/ontology#> ;
      rdfs:label "NACE 2 classification" .


###  http://data.businessgraph.io/ontology#
<http://data.businessgraph.io/ontology#> rdf:type owl:NamedIndividual ;
                                         dct:creator <http://businessgraph.io> ,
                                                     <http://ontotext.com> ,
                                                     <mailto:vladimir.alexiev@ontotext.com> .


###  http://data.businessgraph.io/resolution/
<http://data.businessgraph.io/resolution/> rdf:type owl:NamedIndividual ,
                                                    skos:ConceptScheme ;
                                           dct:creator <http://businessgraph.io> ;
                                           dct:publisher <http://businessgraph.io> ;
                                           rdfs:comment "Resolution of a geographic coordinate location: from continent (least precise) to individual house number (most precise)" ;
                                           rdfs:isDefinedBy <http://data.businessgraph.io/ontology#> ;
                                           rdfs:label "Geo Coordinate Resolution" .


###  http://data.businessgraph.io/status/
<http://data.businessgraph.io/status/> rdf:type owl:NamedIndividual ,
                                                skos:ConceptScheme ;
                                       dct:creator <http://businessgraph.io> ;
                                       dct:publisher <http://businessgraph.io> ;
                                       rdfs:comment "Company status, e.g. active, inactive. Unfortunately different providers use different definitions" ;
                                       rdfs:isDefinedBy <http://data.businessgraph.io/ontology#> ;
                                       rdfs:label "Company status" .


###  http://data.businessgraph.io/type/
<http://data.businessgraph.io/type/> rdf:type owl:NamedIndividual ,
                                              skos:ConceptScheme ;
                                     dct:creator <http://businessgraph.io> ;
                                     dct:publisher <http://businessgraph.io> ;
                                     rdfs:comment "Company type (legal form) per jurisdiction" ;
                                     rdfs:isDefinedBy <http://data.businessgraph.io/ontology#> ;
                                     rdfs:label "Company type" .


###  mailto:vladimir.alexiev@ontotext.com
<mailto:vladimir.alexiev@ontotext.com> rdf:type owl:NamedIndividual .


#################################################################
#    Annotations
#################################################################

dct:creator schema:rangeIncludes xsd:anyURI ;
            skos:scopeNote "In many countries there is a single registry although in others, such as Spain and Germany, multiple registries exist. [rov:]" ;
            rdfs:label "identifier issuer" ;
            schema:domainIncludes ebg:IdentifierSystem ;
            rdfs:label "Identifier System Issuer" ;
            skos:example """• Web URLs are not issued by any central agency and there is no register to consult.
• Companies House is the issuer for the official UK identifier system.
• Dun and Bradstreet issues DUNS numbers.
• GLEI Foundation (GLEIF) issues identifiers for the world-wide GLEI register (through its Local Operating Units, LOU).""" ;
            skos:scopeNote """Many agencies keep several registries. E.g., http://www.registryagency.bg  keeps:
• Trade Register http://brra.bg for companies
• Bulstat Register http://www.bulstat.bg/ for other entities""" ;
            skos:definition "Agent that issues identifiers and then keeps them in a database (register)" ,
                            "Agency that issued the identifier, and register that holds it." ;
            schema:domainIncludes adms:Identifier .


schema:sameAs rdfs:label "Wikipedia page" ;
              schema:domainIncludes rov:RegisteredOrganization ;
              schema:rangeIncludes xsd:anyURI ;
              skos:example <https://it.wikipedia.org/wiki/Trento> ;
              skos:definition "Wikipedia page pertaining to the company." .


schema:url schema:domainIncludes ebg:IdentifierSystem ;
           rdfs:label "identifier system website" ;
           schema:rangeIncludes xsd:anyURI ;
           skos:definition "Various websites of the identifier system and/or its associated issuer and register, e.g. home page, search, download." ;
           rdfs:label "website" ;
           schema:domainIncludes rov:RegisteredOrganization ;
           skos:scopeNote "To be more specific on what the URL returns, Web Resource should be used (see Section 2.3.1.1.4). Not for per-company or validation rule URLs (see Section 2.3.1.1.3)." ;
           skos:example <http://www.comune.trento.it> ;
           skos:definition "Website pertaining to the company" .


###  Generated by the OWL API (version 4.2.8.20170104-2310) https://github.com/owlcs/owlapi
