@base            <http://data.businessgraph.io/>.
@prefix ebg:     <http://data.businessgraph.io/ontology#> .
@prefix acrt:    <https://privatealpha.com/ontology/certification/1#> .
@prefix adms:    <http://www.w3.org/ns/adms#>.
@prefix dbo:     <http://dbpedia.org/ontology/>.
@prefix dc:      <http://purl.org/dc/elements/1.1/>.
@prefix dct:     <http://purl.org/dc/terms/> .
@prefix foaf:    <http://xmlns.com/foaf/0.1/> .
@prefix locn:    <http://www.w3.org/ns/locn#>.
@prefix nuts:    <http://nuts.geovocab.org/id/>.
@prefix org:     <http://www.w3.org/ns/org#>.
@prefix owl:     <http://www.w3.org/2002/07/owl#> .
@prefix person:  <http://www.w3.org/ns/person#>.
@prefix rdf:     <http://www.w3.org/1999/02/22-rdf-syntax-ns#> .
@prefix rdfs:    <http://www.w3.org/2000/01/rdf-schema#> .
@prefix rov:     <http://www.w3.org/ns/regorg#>.
@prefix schema:  <http://schema.org/> .
@prefix sdatke:  <http://ontologies.spaziodati.eu/atoka-ebg#> .
@prefix sioc:    <http://rdfs.org/sioc/ns#> .
@prefix skos:    <http://www.w3.org/2004/02/skos/core#> .
@prefix void:    <http://rdfs.org/ns/void#> .
@prefix xsd:     <http://www.w3.org/2001/XMLSchema#> .


<https://spaziodati.eu/> a schema:Organization;
  schema:name "SpazioDati";
  skos:notation "SDATI".

<dataset/SDATI> a void:Dataset ;
  dct:description "euBusinessGraph only provides info about jurisdictions and fields in this dataset. Contact the publisher for commercial information." ;
  dct:title "SpazioDati full dataset" ;
  dct:type <dataset/type/provider> ;
  dct:publisher <https://spaziodati.eu/en/> ;
  void:subset <dataset/SDATI/GB>, <dataset/SDATI/IT>, <dataset/SDATI/EBG> .

<dataset/SDATI/EBG> a void:Dataset ;
  dct:title "SpazioDati dataset provided to EBG" ;
  dct:publisher <https://spaziodati.eu/> ;
  dct:type <dataset/type/provided-to-EBG> ;
  dct:license <https://atoka.io/en/terms-use/> ;
  void:subset <dataset/SDATI/EBG/IT>, <dataset/SDATI/EBG/GB> .

## Extra classes and properties ---------------------------------------------------------------------------------------
dbo:updated a owl:DatatypeProperty ;
  schema:rangeIncludes xsd:date ;
  skos:definition "The last update date of a resource." ;
  rdfs:label "last updated" .

dbo:score a owl:DatatypeProperty ;
  schema:rangeIncludes xsd:double ;
  skos:definition "Score or points of something." ;
  rdfs:label "score value" .

dbo:rating a owl:DatatypeProperty ;
  schema:rangeIncludes xsd:double ;
  skos:definition "An evaluation or assessment of something, in terms of quality, quantity, or some combination of both." ;
  rdfs:label "rating value" .

sdatke:percentileRank a owl:DatatypeProperty ;
  schema:rangeIncludes xsd:double ;
  skos:definition "The percentage of scores in a frequency distribution that are equal to or lower than a score." ;
  rdfs:label "percentile rank" .

#### Root fields
#### Atoka Indicators
sdatke:AtokaInnovationScore a rdfs:Class ;
  rdfs:isDefinedBy sdatke: ;
  skos:definition "A score given to the company based on the content of its website that measures the innovation factors of a company." ;
  skos:scopeNote <https://developers.atoka.io/v2/glossary.html#innovationScore> ;
  rdfs:label "Atoka Innovation Score" .
dbo:updated schema:domainIncludes sdatke:AtokaInnovationScore .
dbo:percentileRank schema:domainIncludes sdatke:AtokaInnovationScore .

sdatke:atokaInnovationScore a owl:ObjectProperty ;
  rdfs:isDefinedBy sdatke: ;
  rdfs:label "Atoka innovation score" ;
  schema:domainIncludes rov:RegisteredOrganization ;
  schema:rangeIncludes sdatke:AtokaInnovationScore ;
  skos:definition "The Atoka Innovation Score of a Registered Organisation." .

sdatke:AtokaInnovationScoreBySector a rdfs:Class ;
  rdfs:isDefinedBy sdatke: ;
  skos:definition "A score given to the company based on the content of its website that measures the innovation factors of a company within its prevalent economic sector." ;
  skos:scopeNote <https://developers.atoka.io/v2/glossary.html#innovationCategoryScore> ;
  rdfs:label "Atoka Innovation Score by sector" .
dbo:updated schema:domainIncludes sdatke:AtokaInnovationScoreBySector .
dbo:percentileRank schema:domainIncludes sdatke:AtokaInnovationScoreBySector .

sdatke:atokaInnovationScoreBySector a owl:ObjectProperty ;
  rdfs:isDefinedBy sdatke: ;
  rdfs:label "Atoka innovation score by sector" ;
  schema:domainIncludes rov:RegisteredOrganization ;
  schema:rangeIncludes sdatke:AtokaInnovationScoreBySector ;
  skos:definition "The Atoka Innovation Score of a Registered Organisation in its prevalent economic sector." .

sdatke:IstatIDE a rdfs:Class ;
  rdfs:isDefinedBy sdatke: ;
  skos:definition "A score comparing the state of degradation of buildings in an urban area with the national average value." ;
  skos:scopeNote <https://developers.atoka.io/v2/glossary.html#territorialScoreIDE> ;
  rdfs:label "Istat Building Degradation Index" .
dbo:updated schema:domainIncludes sdatke:IstatIDE .
dbo:score schema:domainIncludes sdatke:IstatIDE .

sdatke:istatIDE a owl:ObjectProperty ;
  rdfs:isDefinedBy sdatke: ;
  rdfs:label "Istat building degradation index" ;
  schema:domainIncludes rov:RegisteredOrganization ;
  schema:rangeIncludes sdatke:AtokaInnovationScoreBySector ;
  skos:definition "The Istat Building Degradation Index of a Registered Organisation's headquarters area." .

sdatke:IstatIDS a rdfs:Class ;
  rdfs:isDefinedBy sdatke: ;
  skos:definition "A score measuring unemployment rate, scholarisation and the average age of the population in an urban area." ;
  skos:scopeNote <https://developers.atoka.io/v2/glossary.html#territorialScoreIDS> ;
  rdfs:label "Istat Social Distress Index" .
dbo:updated schema:domainIncludes sdatke:IstatIDS .
dbo:score schema:domainIncludes sdatke:IstatIDS .

sdatke:istatIDS a owl:ObjectProperty ;
  rdfs:isDefinedBy sdatke: ;
  rdfs:label "Istat social distress index" ;
  schema:domainIncludes rov:RegisteredOrganization ;
  schema:rangeIncludes sdatke:AtokaInnovationScoreBySector ;
  skos:definition "The Istat Social Distress Index of a Registered Organisation's headquarters area." .

sdatke:AtokaWebCentrality a rdfs:Class ;
  rdfs:isDefinedBy sdatke: ;
  skos:definition "A score that measures how central the webpage of that company is in the Corporate Web." ;
  skos:scopeNote <https://developers.atoka.io/v2/glossary.html#webCentralityScore> ;
  rdfs:label "Atoka Web Centrality" .
dbo:updated schema:domainIncludes sdatke:AtokaWebCentrality .
dbo:percentileRank schema:domainIncludes sdatke:AtokaWebCentrality .

sdatke:atokaWebCentrality a owl:ObjectProperty ;
  rdfs:isDefinedBy sdatke: ;
  rdfs:label "Atoka web centrality" ;
  schema:domainIncludes rov:RegisteredOrganization ;
  schema:rangeIncludes sdatke:AtokaWebCentrality ;
  skos:definition "The Atoka Web Centrality of a Registered Organisation." .

sdatke:AtokaWebCentralityBySector a rdfs:Class ;
  rdfs:isDefinedBy sdatke: ;
  skos:definition "A score that measures how central the webpage of that company is in the Corporate Web, within its prevalent economic sector." ;
  skos:scopeNote <https://developers.atoka.io/v2/glossary.html#webCentralityCategoryScore> ;
  rdfs:label "Atoka Web Centrality by sector" .
dbo:updated schema:domainIncludes sdatke:AtokaWebCentralityBySector .
dbo:percentileRank schema:domainIncludes sdatke:AtokaWebCentralityBySector .

sdatke:atokaWebCentralityBySector a owl:ObjectProperty ;
  rdfs:isDefinedBy sdatke: ;
  rdfs:label "Atoka web centrality by sector" ;
  schema:domainIncludes rov:RegisteredOrganization ;
  schema:rangeIncludes sdatke:AtokaWebCentralityBySector ;
  skos:definition "The Atoka Innovation Score of a Registered Organisation in its prevalent economic sector." .

#### Balance Sheets
sdatke:BalanceSheet a rdfs:Class ;
  rdfs:isDefinedBy sdatke: ;
  rdfs:label "Balance Sheet" ;
  skos:definition "A statement of the assets, liabilities, and capital of a business or other organization at a particular point in time, detailing the balance of income and expenditure over the preceding period." .
  
dbo:assets a owl:DatatypeProperty ;
  schema:domainIncludes sdatke:BalanceSheet, rov:RegisteredOrganization ;
  schema:rangeIncludes xsd:double ;
  skos:definition "Anything tangible or intangible that is capable of being owned or controlled to produce value and that is held to have positive economic value." ;
  rdfs:label "assets" .

sdatke:capitalStock a owl:DatatypeProperty ;
  rdfs:isDefinedBy sdatke: ;
  schema:domainIncludes sdatke:BalanceSheet, rov:RegisteredOrganization ;
  schema:rangeIncludes xsd:double ;
  skos:definition "The nominal (or authorised) capital that the company is authorised to issue to shareholders." ;
  rdfs:label "capital stock" .

sdatke:costs a owl:DatatypeProperty ;
  rdfs:isDefinedBy sdatke: ;
  schema:domainIncludes sdatke:BalanceSheet ;
  schema:rangeIncludes xsd:double ;
  skos:definition "The sum of purchases, personnel costs and charges for services and third-party goods, from which the variations in raw materials are detracted." ;
  rdfs:label "costs" .

sdatke:ebitda a owl:DatatypeProperty ;
  rdfs:isDefinedBy sdatke: ;
  schema:domainIncludes sdatke:BalanceSheet ;
  schema:rangeIncludes xsd:double ;
  skos:definition "Earnings Before Interest, taxes, depreciation and amortization." ;
  rdfs:label "ebitda" .

sdatke:grossOperatingMargin a owl:DatatypeProperty ;
  rdfs:isDefinedBy sdatke: ;
  schema:domainIncludes sdatke:BalanceSheet ;
  schema:rangeIncludes xsd:double ;
  skos:definition "Profit from selling goods or services in a particular period after costs directly related to producing them are subtracted." ;
  rdfs:label "gross operating margin" .

sdatke:netFinancialPosition a owl:DatatypeProperty ;
  rdfs:isDefinedBy sdatke: ;
  schema:domainIncludes sdatke:BalanceSheet ;
  schema:rangeIncludes xsd:double ;
  skos:definition "Financial liabilities minus cash and cash equivalents." ;
  rdfs:label "net financial position" .

sdatke:costOfSales a owl:DatatypeProperty ;
  rdfs:isDefinedBy sdatke: ;
  schema:domainIncludes sdatke:BalanceSheet ;
  schema:rangeIncludes xsd:double ;
  skos:definition "For a manufacturer is the cost of its finished goods in its beginning inventory plus the cost of goods manufactured during the accounting period minus the cost of finished goods in ending inventory.",
    "For a retailer is the cost of merchandise in its beginning inventory plus the net cost of merchandise purchased during the accounting period minus the cost of merchandise in its ending inventory." ;
  rdfs:label "cost of sales" .

sdatke:operatingProfit a owl:DatatypeProperty ;
  rdfs:isDefinedBy sdatke: ;
  schema:domainIncludes sdatke:BalanceSheet ;
  schema:rangeIncludes xsd:double ;
  skos:definition "A profit from business operations (gross profit minus operating expenses) before deduction of interest and taxes." ;
  rdfs:label "operating profit" .

sdatke:purchases a owl:DatatypeProperty ;
  rdfs:isDefinedBy sdatke: ;
  schema:domainIncludes sdatke:BalanceSheet ;
  schema:rangeIncludes xsd:double ;
  skos:definition "A general ledger account in which is recorded the inventory purchases of a business." ;
  rdfs:label "purchases" .

sdatke:inventoryChangeInRawMaterials a owl:DatatypeProperty ;
  rdfs:isDefinedBy sdatke: ;
  schema:domainIncludes sdatke:BalanceSheet ;
  schema:rangeIncludes xsd:double ;
  skos:definition "The difference between the inventory totals regarding raw materials for the last reporting period and the current reporting period." ;
  rdfs:label "inventory change in raw materials" .

dbo:revenue a owl:DatatypeProperty ;
  schema:domainIncludes sdatke:BalanceSheet, rov:RegisteredOrganization ;
  schema:rangeIncludes xsd:double ;
  skos:definition "The amount of money that a company actually receives during a specific period, including discounts and deductions for returned merchandise." ;
  rdfs:label "revenue" .

sdatke:revenueTrend a owl:DatatypeProperty ;
  rdfs:isDefinedBy sdatke: ;
  schema:domainIncludes sdatke:BalanceSheet ;
  schema:rangeIncludes xsd:double ;
  skos:definition "Percentage of increase of revenue since the last report." ;
  rdfs:label "revenue trend" .

sdatke:costOfMaterials a owl:DatatypeProperty ;
  rdfs:isDefinedBy sdatke: ;
  schema:domainIncludes sdatke:BalanceSheet ;
  schema:rangeIncludes xsd:double ;
  skos:definition "Percentage of increase of revenue since the last report." ;
  rdfs:label "revenue trend" .

sdatke:leasesAndRentalExpenses a owl:DatatypeProperty ;
  rdfs:isDefinedBy sdatke: ;
  schema:domainIncludes sdatke:BalanceSheet ;
  schema:rangeIncludes xsd:double ;
  skos:definition "Total expenses for lease and rental of third-party goods and services." ;
  rdfs:label "leases and rental expenses" .

sdatke:personnelCosts a owl:DatatypeProperty ;
  rdfs:isDefinedBy sdatke: ;
  schema:domainIncludes sdatke:BalanceSheet ;
  schema:rangeIncludes xsd:double ;
  skos:definition "Wages and salaries and employer's social security costs." ;
  rdfs:label "personnel costs" .

dbo:closingDate a owl:DatatypeProperty ;
  schema:domainIncludes sdatke:BalanceSheet ;
  schema:rangeIncludes xsd:date ;
  skos:definition "Balance sheet closing date." ;
  rdfs:label "closing date" .

sdatke:balanceSheet a owl:ObjectProperty ;
  rdfs:isDefinedBy sdatke: ;
  rdfs:label "balance sheet" ;
  schema:domainIncludes rov:RegisteredOrganization ;
  schema:rangeIncludes sdatke:BalanceSheet ;
  skos:definition "Balance Sheet report of a Registered Organisation." .

#### Base fields
sdatke:AGCMLegalityRating a rdfs:Class ;
  rdfs:isDefinedBy sdatke: ;
  skos:definition "Measure of compliance with legality protocols, transparent traceability systems and certified compliance checks." ;
  skos:scopeNote <https://en.agcm.it/en/scope-of-activity/legality-rating/> ;
  rdfs:label "AGCM Legality Rating" .

schema:expires a owl:DatatypeProperty ;
  schema:domainIncludes sdatke:AGCMLegalityRating ;
  schema:rangeIncludes xsd:date ;
  skos:definition "The AGCM Legality Rating expiration date" ;
  rdfs:label "expiration date" .

dbo:rating schema:domainIncludes sdatke:AGCMLegalityRating ;
  schema:rangeIncludes xsd:string .

sdatke:agcmLegalityRating a owl:ObjectProperty ;
  rdfs:isDefinedBy sdatke: ;
  rdfs:label "AGCM legality rating" ;
  schema:domainIncludes rov:RegisteredOrganization ;
  schema:rangeIncludes sdatke:AGCMLegalityRating ;
  skos:definition "The AGCM Legality Rating for a Registered Organisation." .


sdatke:businessDescription a owl:DatatypeProperty ;
  rdfs:isDefinedBy sdatke: ;
  rdfs:label "business description" ;
  schema:domainIncludes rov:RegisteredOrganization ;
  schema:rangeIncludes rdf:langString ;
  skos:definition "Description of the main business activity of the company." .


sdatke:italianPublicSectorOrganizationCode a owl:DatatypeProperty ;
  rdfs:isDefinedBy sdatke: ;
  rdfs:label "italian PSO code" ;
  schema:domainIncludes rov:RegisteredOrganization ;
  schema:rangeIncludes rdf:string ;
  skos:definition "Identifier issued by the Italian government for public sector organizations." ;
  skos:scopeNone <https://developers.atoka.io/v2/glossary.html#govtypes> .

sdatke:italianPublicSectorOrganizationType a owl:DatatypeProperty ;
  rdfs:isDefinedBy sdatke: ;
  rdfs:label "type of italian PSO" ;
  schema:domainIncludes rov:RegisteredOrganization ;
  schema:rangeIncludes rdf:string ;
  skos:definition "The type of Italian public sector organization." ;
  skos:scopeNone <https://developers.atoka.io/v2/glossary.html#govtypes> .

#### Certifications
acrt:Certification a owl:Class ;
  skos:definition """Represents the abstract notion of certification, of an agent, by another agent,
that the first agent possesses some property or set of properties implied by the certification,
potentially within some spatiotemporal scope.""" ;
  skos:scopeNote <https://privatealpha.com/ontology/certification/1#Certification> ;
  rdfs:label "Certification" .

acrt:has-certification a owl:ObjectProperty ;
  rdfs:label "certification" ;
  schema:domainIncludes rov:RegisteredOrganization ;
  schema:rangeIncludes acrt:Certification ;
  skos:definition "This property specifies that a Registered Organization has a given Certification." .


#### Contact Phone
sdatke:ContactPhone a rdfs:Class ;
  rdfs:isDefinedBy sdatke: ;
  skos:definition "Contact phone of a given type." ;
  rdfs:label "Contact Phone" .

foaf:phone a owl:DatatypeProperty ;
  schema:domainIncludes sdatke:ContactPhone ;
  schema:rangeIncludes xsd:string ;
  skos:definition "Number for the Contact Phone." ;
  rdfs:label "number" .

sdatke:contactPhone a owl:ObjectProperty ;
  rdfs:isDefinedBy sdatke: ;
  schema:domainIncludes org:Site ;
  schema:rangeIncludes sdatke:ContactPhone ;
  skos:definition "Contact Phone of a Site." ;
  rdfs:label "phone" .

#### Contact Email
sdatke:ContactEmail a rdfs:Class ;
  rdfs:isDefinedBy sdatke: ;
  skos:definition "An email contact of a given type." ;
  rdfs:label "Contact Email" .

schema:email a owl:DatatypeProperty ;
  schema:domainIncludes sdatke:ContactEmail ;
  schema:rangeIncludes rdf:Resource ;
  skos:definition "Email address for the Contact Email." ;
  rdfs:label "email address" .

sdatke:contactEmail a owl:ObjectProperty ;
  rdfs:isDefinedBy sdatke: ;
  schema:domainIncludes rov:RegisteredOrganization ;
  schema:rangeIncludes sdatke:ContactEmail ;
  skos:definition "A Contact Email of a Registered Organisation." ;
  rdfs:label "email address" .

sdatke:contactType a owl:DatatypeProperty ;
  rdfs:isDefinedBy sdatke: ;
  schema:domainIncludes sdatke:ContactEmail, sdatke:ContactPhone ;
  schema:rangeIncludes rdf:langString ;
  skos:definition "Type of contact" ;
  skos:scopeNote "Most frequent values are \"administration\", \"info\", \"management\", \"marketing\", \"purchases\", \"sales\", \"support\", \"technician\", \"personal\", \"other\"." ;
  rdfs:label "contact type" .

sdatke:faxNumber a owl:DatatypeProperty ;
  schema:domainIncludes rov:RegisteredOrganization ;
  schema:rangeIncludes xsd:string ;
  skos:definition "Fax number associated to a company." ;
  rdfs:label "fax number" .

#### Employee Count Report
sdatke:EmployeeCountReport a rdfs:Class ;
  rdfs:isDefinedBy sdatke: ;
  rdfs:label "Employee Count Report" ;
  skos:definition "A report of the number of employees in an organisation at a given date." .
  
sdatke:employeeCount a owl:DatatypeProperty ;
  rdfs:isDefinedBy sdatke: ;
  schema:domainIncludes sdatke:EmployeeCountReport ;
  schema:rangeIncludes xsd:nonNegativeInteger ;
  skos:definition "Number of employees in an organisation." ;
  rdfs:label "employee count" .

dct:dateSubmitted a owl:DatatypeProperty ;
  schema:domainIncludes sdatke:EmployeeCountReport ;
  schema:rangeIncludes xsd:date ;
  skos:definition "Employee count report submission date." ;
  rdfs:label "date submitted" .

sdatke:employeeCountReport a owl:ObjectProperty ;
  rdfs:isDefinedBy sdatke: ;
  rdfs:label "employee count report" ;
  schema:domainIncludes rov:RegisteredOrganization ;
  schema:rangeIncludes sdatke:EmployeeCountReport ;
  skos:definition "The number of employees of a Registered Organisation at a given point in time." .

#### Related Entities
sdatke:hasEntity a owl:ObjectProperty ;
  rdfs:isDefinedBy sdatke: ;
  rdfs:label "related entity" ;
  schema:domainIncludes rov:RegisteredOrganization ;
  schema:rangeIncludes rdf:Resource ;
  skos:definition "Relation of an Entity to a Registered Organisation." .

#### Shares (Shareholders and Owned Shares)
sdatke:Share a rdfs:Class ;
  rdfs:isDefinedBy sdatke: ;
  rdfs:label "Share Ownership" ;
  skos:definition "Ownership of company shares." .

sdatke:ownershipType a owl:DatatypeProperty ;
  rdfs:isDefinedBy sdatke: ;
  rdfs:label "ownership type" ;
  schema:domainIncludes sdatke:Share ;
  schema:rangeIncludes xsd:string ;
  skos:definition "Type of share ownership (free text)." .

dbo:ratio a owl:DatatypeProperty ;
  rdfs:label "amount" ;
  schema:domainIncludes sdatke:Share ;
  schema:rangeIncludes xsd:float ;
  skos:definition "Ratio of this share ownership to total shares." .

dbo:owner a owl:ObjectProperty ;
  rdfs:label "owned by" ;
  schema:domainIncludes sdatke:Share ;
  schema:rangeIncludes rov:RegisteredOrganization, person:Person ;
  skos:definition "Ownership of company shares by a company or a person." .

dbo:owns a owl:ObjectProperty ;
  rdfs:label "owned shares" ;
  schema:domainIncludes rov:RegisteredOrganization, person:Person ;
  schema:rangeIncludes sdatke:Share ;
  skos:definition "Shares owned by the company." .

sdatke:share a owl:ObjectProperty ;
  rdfs:isDefinedBy sdatke: ;
  rdfs:label "shares" ;
  schema:domainIncludes rov:RegisteredOrganization ;
  schema:rangeIncludes sdatke:Share ;
  skos:definition "Share of the company owned by a person or another company." .

#### Web technologies
sdatke:analyticsTechUsed a owl:DatatypeProperty ;
  rdfs:isDefinedBy sdatke: ;
  rdfs:label "analytics technology used" ;
  schema:domainIncludes rov:RegisteredOrganization ;
  schema:rangeIncludes xsd:string ;
  skos:definition "Analytics technology used by the company on its websites." .

sdatke:smartphoneAppUsed a owl:DatatypeProperty ;
  rdfs:isDefinedBy sdatke: ;
  rdfs:label "smartphone application used" ;
  schema:domainIncludes rov:RegisteredOrganization ;
  schema:rangeIncludes rdf:Resource ;
  skos:definition "Link to the store page of the smartphone application used by the company on its websites." .

sdatke:blogTechUsed a owl:DatatypeProperty ;
  rdfs:isDefinedBy sdatke: ;
  rdfs:label "blogging technology used" ;
  schema:domainIncludes rov:RegisteredOrganization ;
  schema:rangeIncludes xsd:string ;
  skos:definition "Name of the blog-related technology used by the company on its websites." .

sdatke:cmsTechUsed a owl:DatatypeProperty ;
  rdfs:isDefinedBy sdatke: ;
  rdfs:label "CMS technology used" ;
  schema:domainIncludes rov:RegisteredOrganization ;
  schema:rangeIncludes xsd:string ;
  skos:definition "Name of the CMS-related technology used by the company on its websites." .

sdatke:eCommerceTechUsed a owl:DatatypeProperty ;
  rdfs:isDefinedBy sdatke: ;
  rdfs:label "E-commerce technology used" ;
  schema:domainIncludes rov:RegisteredOrganization ;
  schema:rangeIncludes xsd:string ;
  skos:definition "Name of the E-commerce -related technology used by the company on its websites." .

sdatke:marketingToolUsed a owl:DatatypeProperty ;
  rdfs:isDefinedBy sdatke: ;
  rdfs:label "marketing tool used" ;
  schema:domainIncludes rov:RegisteredOrganization ;
  schema:rangeIncludes xsd:string ;
  skos:definition "Name of the marketing tool used by the company on its websites." .

sdatke:paymentsPlatformUsed a owl:DatatypeProperty ;
  rdfs:isDefinedBy sdatke: ;
  rdfs:label "payments platform used" ;
  schema:domainIncludes rov:RegisteredOrganization ;
  schema:rangeIncludes xsd:string ;
  skos:definition "Name of the payments platform used by the company on its websites." .

dbo:logo a owl:ObjectProperty ;
  rdfs:label "logo" ;
  schema:domainIncludes rov:RegisteredOrganization ;
  schema:rangeIncludes rdf:Resource ;
  skos:definition "Logo image associated to the company." .

sdatke:isStartup a owl:DatatypeProperty;
  rdfs:isDefinedBy ebg: ;
  rdfs:label "is startup" ;
  schema:domainIncludes rov:RegisteredOrganization ;
  schema:rangeIncludes xsd:boolean;
  skos:definition "Whether the company is a startup [ebg:]";
  skos:example "A special section of the IT Business Register http://startup.registroimprese.it/ includes pitch, sectors and business model of startups and innovative SMEs".

## --------------------------------------------------------------------------------------------------------------------

<dataset/SDATI/GB> a void:Dataset;
  dct:title "SpazioDati full dataset of GB companies" ;
  dct:type <dataset/type/partition> ;
  dct:spatial "GB" ;
  void:entities 4276471 ;
  void:classPartition <dataset/SDATI/GB/address>, <dataset/SDATI/GB/person>, <dataset/SDATI/GB/membership>;
  void:property
    dct:creator,
    dct:isPartOf,
    org:member,
    org:memberDuring,
    org:organization,
    org:role,
    org:siteAddress,
    rov:legalName,
    schema:availableLanguage,
    schema:url,
    # root fields
    rov:orgStatus,
    dbo:jurisdiction,
    org:hasRegisteredSite,
    locn:adminUnitL1,
    locn:adminUnitL2,
    ebg:adminUnitL3,
    ebg:adminUnitL4,
    ebg:adminUnitL5,
    ebg:adminUnitL6,
    locn:postName,
    locn:postCode,
    locn:thoroughfare,
    schema:geo,
    schema:latitude,
    schema:longitude,
    ebg:geoResolution,
    locn:locatorDesignator,
    skos:prefLabel,
    # atokaindicators
    # balance sheets
    dbo:assets,
    sdatke:capitalStock,
    dbo:revenue,
    sdatke:balanceSheet,
    # base
    skos:altLabel,
    rov:orgActivity,
    rov:orgActivityText,
    sdatke:businessDescription,
    rov:registration,
    ebg:foundingYear,
    schema:foundingDate,
    rov:orgType,
    ebg:orgTypeText,
    rov:orgType,
    rov:orgTypeText,
    rov:legalName,
    schema:email,
    adms:identifier,
    # certifications
    # contacts
    sdatke:contactPhone,
    sdatke:contactEmail,
    # economics
    ebg:isPubliclyTraded,
    # related entities
    sdatke:hasEntity,
    # locations
    org:hasSite,
    # shares
    # web technologies
    sdatke:analyticsTechUsed,
    sdatke:smartphoneAppUsed,
    sdatke:blogTechUsed,
    sdatke:cmsTechUsed,
    sdatke:eCommerceTechUsed,
    sdatke:marketingToolUsed,
    sdatke:paymentsPlatformUsed,
    dbo:logo,
    sioc:feed ;
  dct:license <https://atoka.io/en/terms-use/>;
  dct:source <https://spaziodati.eu/en/>, <https://atoka.io/en/>.

<dataset/SDATI/GB/address>    a void:Dataset; dct:type <dataset/type/partition>; void:class locn:Address;   void:entities 4417147.
<dataset/SDATI/GB/person>     a void:Dataset; dct:type <dataset/type/partition>; void:class person:Person;  void:entities 6900513.
<dataset/SDATI/GB/membership> a void:Dataset; dct:type <dataset/type/partition>; void:class org:Membership; void:entities 8531141.

<dataset/SDATI/IT> a void:Dataset;
  dct:title "SpazioDati full dataset of IT companies";
  dct:type <dataset/type/partition>;
  dct:spatial "IT";
  void:entities 6067546;
  void:classPartition <dataset/SDATI/IT/address>, <dataset/SDATI/IT/person>, <dataset/SDATI/IT/membership>;
  void:property
    dct:creator,
    dct:isPartOf,
    org:member,
    org:memberDuring,
    org:organization,
    org:role,
    org:siteAddress,
    rov:legalName,
    schema:availableLanguage,
    schema:url,
    # root fields
    rov:orgStatus,
    dbo:jurisdiction,
    org:hasRegisteredSite,
    locn:adminUnitL1,
    locn:adminUnitL2,
    ebg:adminUnitL3,
    ebg:adminUnitL4,
    ebg:adminUnitL5,
    ebg:adminUnitL6,
    locn:postName,
    locn:postCode,
    locn:thoroughfare,
    schema:geo,
    schema:latitude,
    schema:longitude,
    ebg:geoResolution,
    locn:locatorDesignator,
    skos:prefLabel,
    # atokaindicators
    sdatke:atokaInnovationScore,
    sdatke:atokaInnovationScoreBySector,
    sdatke:istatIDE,
    sdatke:istatIDS,
    sdatke:atokaWebCentrality,
    sdatke:atokaWebCentralityBySector,
    sdatke:agcmLegalityRating,
    # balance sheets
    dbo:assets,
    sdatke:capitalStock,
    dbo:revenue,
    sdatke:balanceSheet,
    # base
    sdatke:agcmLegalityRating,
    skos:altLabel,
    rov:orgActivity,
    rov:orgActivityText,
    sdatke:businessDescription,
    rov:registration,
    ebg:foundingYear,
    schema:foundingDate,
    ebg:isStateOwned,
    sdatke:italianPublicSectorOrganizationCode,
    sdatke:italianPublicSectorOrganizationType,
    rov:orgType,
    ebg:orgTypeText,
    rov:orgType,
    rov:orgTypeText,
    rov:legalName,
    schema:email,
    ebg:isStartup,
    adms:identifier,
    # certifications
    acrt:has-certification,
    # contacts
    sdatke:contactPhone,
    sdatke:contactEmail,
    sdatke:faxNumber,
    # economics
    sdatke:employeeCountReport,
    ebg:isPubliclyTraded,
    # related entities
    sdatke:hasEntity,
    # locations
    org:hasSite,
    # shares
    sdatke:share,
    dbo:owns,
    # web technologies
    sdatke:analyticsTechUsed,
    sdatke:smartphoneAppUsed,
    sdatke:blogTechUsed,
    sdatke:cmsTechUsed,
    sdatke:eCommerceTechUsed,
    sdatke:marketingToolUsed,
    sdatke:paymentsPlatformUsed,
    dbo:logo,
    sioc:feed ;
  dct:license <https://atoka.io/en/terms-use/> ;
  dct:source <https://spaziodati.eu/en/>, <https://atoka.io/en/> .

<dataset/SDATI/IT/address>    a void:Dataset; dct:type <dataset/type/partition>; void:class locn:Address;   void:entities 12107304.
<dataset/SDATI/IT/person>     a void:Dataset; dct:type <dataset/type/partition>; void:class person:Person;  void:entities 14589257.
<dataset/SDATI/IT/membership> a void:Dataset; dct:type <dataset/type/partition>; void:class org:Membership; void:entities 17647023.

<https://spaziodati.eu/en/> a ebg:WebResource;
  schema:url <https://spaziodati.eu/en/>;
  schema:name "SpazioDati: home page"@en;
  dc:format "text/html";
  schema:inLanguage "en".

<https://atoka.io/en/> a ebg:WebResource;
  schema:url <https://atoka.io/en/>;
  schema:name "Atoka: All of the italian and british companies in a unique database"@en;
  dc:format "text/html";
  schema:inLanguage "en".
