<rdf:RDF
    xmlns:ngeo="http://geovocab.org/geometry#"
    xmlns:dbo="http://dbpedia.org/ontology/"
    xmlns:locn="http://www.w3.org/ns/locn#"
    xmlns:ramon="http://rdfdata.eionet.europa.eu/ramon/ontology/"
    xmlns:dct="http://purl.org/dc/terms/"
    xmlns:dc="http://purl.org/dc/elements/1.1/"
    xmlns:adms="http://www.w3.org/ns/adms#"
    xmlns:puml="http://plantuml.com/ontology#"
    xmlns:skos="http://www.w3.org/2004/02/skos/core#"
    xmlns:vann="http://purl.org/vocab/vann/"
    xmlns:org="http://www.w3.org/ns/org#"
    xmlns:ebg="http://data.businessgraph.io/ontology#"
    xmlns:xsd="http://www.w3.org/2001/XMLSchema#"
    xmlns:rdf="http://www.w3.org/1999/02/22-rdf-syntax-ns#"
    xmlns:ebg-comp="http://data.businessgraph.io/company/"
    xmlns:schema="http://schema.org/"
    xmlns:rdfs="http://www.w3.org/2000/01/rdf-schema#"
    xmlns:rov="http://www.w3.org/ns/regorg#"
    xmlns:spatial="http://geovocab.org/spatial#"
    xmlns:void="http://rdfs.org/ns/void#"
    xmlns:nuts="http://nuts.geovocab.org/id/"
    xmlns:time="http://www.w3.org/2006/time#"
    xmlns:owl="http://www.w3.org/2002/07/owl#"
    xmlns:sioc="http://rdfs.org/sioc/ns#"
    xmlns:nace="http://data.businessgraph.io/nace/"
    xmlns:ebg-id="http://data.businessgraph.io/identifier/"
    xmlns:lau="http://data.businessgraph.io/lau/"
    xmlns:person="http://www.w3.org/ns/person#"
    xmlns:foaf="http://xmlns.com/foaf/0.1/" > 
  <rdf:Description rdf:about="http://www.w3.org/2001/XMLSchema#string">
    <rdfs:label>String</rdfs:label>
    <rdf:type rdf:resource="http://www.w3.org/2000/01/rdf-schema#Datatype"/>
  </rdf:Description>
  <rdf:Description rdf:about="http://data.businessgraph.io/dataset/free-available">
    <skos:prefLabel>Freely available</skos:prefLabel>
    <skos:inScheme rdf:resource="http://data.businessgraph.io/dataset/"/>
    <rdfs:isDefinedBy rdf:resource="http://data.businessgraph.io/ontology#"/>
    <rdf:type rdf:resource="http://www.w3.org/2004/02/skos/core#Concept"/>
  </rdf:Description>
  <rdf:Description rdf:about="http://data.businessgraph.io/ontology#exclusionNote">
    <ebg:order rdf:datatype="http://www.w3.org/2001/XMLSchema#integer">108</ebg:order>
    <schema:rangeIncludes rdf:resource="http://www.w3.org/1999/02/22-rdf-syntax-ns#langString"/>
    <schema:domainIncludes rdf:resource="http://www.w3.org/2004/02/skos/core#Concept"/>
    <rdfs:comment>Exclusion note of a NACE classification concept</rdfs:comment>
    <rdfs:label>exclusion note</rdfs:label>
    <rdfs:isDefinedBy rdf:resource="http://data.businessgraph.io/ontology#"/>
    <rdf:type rdf:resource="http://www.w3.org/2002/07/owl#DatatypeProperty"/>
  </rdf:Description>
  <rdf:Description rdf:about="http://data.businessgraph.io/lau/">
    <rdfs:comment>Local Administrative Units</rdfs:comment>
    <dct:creator rdf:resource="http://businessgraph.io"/>
    <rdf:type rdf:resource="http://rdfs.org/ns/void#Dataset"/>
    <dct:issued rdf:datatype="http://www.w3.org/2001/XMLSchema#date">2017-07-28</dct:issued>
    <rdfs:isDefinedBy rdf:resource="http://data.businessgraph.io/ontology#"/>
    <rdfs:label>LAU Regions</rdfs:label>
    <dct:license rdf:resource="https://opendatacommons.org/licenses/by/"/>
    <dct:publisher rdf:resource="http://businessgraph.io"/>
    <dct:created rdf:datatype="http://www.w3.org/2001/XMLSchema#date">2017-07-28</dct:created>
    <dct:source rdf:resource="http://ec.europa.eu/eurostat/web/nuts/local-administrative-units"/>
  </rdf:Description>
  <rdf:Description rdf:about="http://data.businessgraph.io/ontology#isOfficial">
    <skos:example>False for SDATI identifiers since the SDATI system is not official in Italy.</skos:example>
    <rdfs:isDefinedBy rdf:resource="http://data.businessgraph.io/ontology#"/>
    <skos:example>False for GLEI, since it is not the official register for any of the world's jurisdictions</skos:example>
    <schema:rangeIncludes rdf:resource="http://www.w3.org/2001/XMLSchema#boolean"/>
    <skos:example>True for UK Company House identifiers, the official register for the GB jurisdiction</skos:example>
    <skos:example>False for Website, Twitter, Facebook in that they don't have any official status</skos:example>
    <schema:domainIncludes rdf:resource="http://data.businessgraph.io/ontology#IdentifierSystem"/>
    <skos:definition>Whether the system is considered the official one in all jurisdictions in which it applies.</skos:definition>
    <rdf:type rdf:resource="http://www.w3.org/2002/07/owl#DatatypeProperty"/>
    <ebg:order rdf:datatype="http://www.w3.org/2001/XMLSchema#integer">59</ebg:order>
    <rdfs:label>is official in jurisdiction</rdfs:label>
  </rdf:Description>
  <rdf:Description rdf:about="http://www.w3.org/ns/adms#Identifier">
    <skos:scopeNote>The identifier value is recorded in skos:notation and the issuer/register in dct:creator.</skos:scopeNote>
    <skos:definition>Identifier of an entity (company, person) according to some identifier system.</skos:definition>
    <rdfs:label>Identifier</rdfs:label>
    <rdf:type rdf:resource="http://www.w3.org/2000/01/rdf-schema#Class"/>
  </rdf:Description>
  <rdf:Description rdf:about="http://data.businessgraph.io/ontology#adminUnitL4">
    <ebg:order rdf:datatype="http://www.w3.org/2001/XMLSchema#integer">32</ebg:order>
    <skos:example>nuts:ITC20 Aosta</skos:example>
    <skos:example>nuts:ITH31 Verona</skos:example>
    <skos:definition>NUTS3 (Province) of the address.</skos:definition>
    <rdfs:label>admin unit level 4</rdfs:label>
    <rdfs:isDefinedBy rdf:resource="http://data.businessgraph.io/ontology#"/>
    <schema:rangeIncludes rdf:resource="http://rdfdata.eionet.europa.eu/ramon/ontology/NUTSRegion"/>
    <schema:domainIncludes rdf:resource="http://www.w3.org/ns/locn#Address"/>
    <rdf:type rdf:resource="http://www.w3.org/2002/07/owl#ObjectProperty"/>
  </rdf:Description>
  <rdf:Description rdf:about="http://data.businessgraph.io/type/">
    <dct:publisher rdf:resource="http://businessgraph.io"/>
    <dct:creator rdf:resource="http://businessgraph.io"/>
    <rdfs:comment>Company type (legal form) per jurisdiction</rdfs:comment>
    <rdfs:label>Company type</rdfs:label>
    <rdfs:isDefinedBy rdf:resource="http://data.businessgraph.io/ontology#"/>
    <rdf:type rdf:resource="http://www.w3.org/2004/02/skos/core#ConceptScheme"/>
  </rdf:Description>
  <rdf:Description rdf:about="http://schema.org/geo">
    <ebg:order rdf:datatype="http://www.w3.org/2001/XMLSchema#integer">41</ebg:order>
    <skos:scopeNote>If data is integrated from several providers, we may end up with multiple coordinate pairs in that node, which will need to be resolved into one.</skos:scopeNote>
    <skos:definition>Geographic coordinates, eg of a geo-located address.</skos:definition>
    <rdfs:label>geographic coordinates</rdfs:label>
    <schema:rangeIncludes rdf:resource="http://schema.org/GeoCoordinates"/>
    <schema:domainIncludes rdf:resource="http://www.w3.org/ns/locn#Address"/>
    <rdf:type rdf:resource="http://www.w3.org/2002/07/owl#ObjectProperty"/>
  </rdf:Description>
  <rdf:Description rdf:about="http://data.businessgraph.io/ontology#dissolutionYear">
    <ebg:order rdf:datatype="http://www.w3.org/2001/XMLSchema#integer">16</ebg:order>
    <skos:scopeNote>Used for faceting.</skos:scopeNote>
    <skos:definition>Year the organization was dissolved or deregistered, as integer.</skos:definition>
    <rdfs:label>dissolution year</rdfs:label>
    <schema:rangeIncludes rdf:resource="http://www.w3.org/2001/XMLSchema#integer"/>
    <schema:domainIncludes rdf:resource="http://www.w3.org/ns/regorg#RegisteredOrganization"/>
    <rdf:type rdf:resource="http://www.w3.org/2002/07/owl#DatatypeProperty"/>
  </rdf:Description>
  <rdf:Description rdf:about="http://www.w3.org/ns/org#hasSite">
    <ebg:order rdf:datatype="http://www.w3.org/2001/XMLSchema#integer">24</ebg:order>
    <skos:definition>Other address/location associated to an organisation.</skos:definition>
    <skos:scopeNote>org:hasSite leads to a node with types org:Site &amp; locn:Address that has self-link org:siteAddress. org:hasRegisteredSite is declared a sub-property of org:hasSite, so querying by org:hasSite will obtain all addresses.</skos:scopeNote>
    <rdfs:label>site/address</rdfs:label>
    <schema:rangeIncludes rdf:resource="http://www.w3.org/ns/org#Site"/>
    <schema:domainIncludes rdf:resource="http://www.w3.org/ns/regorg#RegisteredOrganization"/>
    <rdf:type rdf:resource="http://www.w3.org/2002/07/owl#ObjectProperty"/>
  </rdf:Description>
  <rdf:Description rdf:about="http://data.businessgraph.io/ontology#urlTemplate">
    <skos:example>For OCORP, 'https://opencorporates.com/companies/{}.rdf'  returns company data with MIME type 'application/rdf+xml'</skos:example>
    <schema:rangeIncludes rdf:resource="http://www.w3.org/2001/XMLSchema#string"/>
    <skos:example>For OCORP, 'https://opencorporates.com/companies/{}.json' returns company data with MIME type 'application/json'</skos:example>
    <skos:example>For the EU Value Added Tax (VIES) register, "http://ec.europa.eu/taxation_customs/vies/vatResponse.html?memberStateCode=$1&amp;number=$2" with MIME type "text/html" shows a web page for an identifier that can be parsed with ebg:validationRegex "([A-Z]{2})/(\d+)". Here $1 is the member state code, and $2 is the national company id</skos:example>
    <schema:domainIncludes rdf:resource="http://data.businessgraph.io/ontology#IdentifierWebResource"/>
    <skos:definition>URL template of an identifier web resource.&#xD;
If it has a placeholder {}, substitute the identifier value there.&#xD;
If it has placeholders like $1, $2… substitute the groups extracted by ebg:validationRegex</skos:definition>
    <skos:example>For BR, "http://data.brreg.no/enhetsregisteret/enhet/{}" with either "application/xml" or "application/json" returns the respective MIME type using Content Negotiation</skos:example>
    <rdf:type rdf:resource="http://www.w3.org/2002/07/owl#DatatypeProperty"/>
    <skos:example>For BE Banque-Carrefour des Entreprises, "https://kbopub.economie.fgov.be/kbopub/toonondernemingps.html?ondernemingsnummer={}" with MIME type "text/html" shows a web page for the company.</skos:example>
    <skos:example>For OCORP, 'https://opencorporates.com/companies/{}.xml'  returns company data with MIME type 'application/xml'</skos:example>
    <ebg:order rdf:datatype="http://www.w3.org/2001/XMLSchema#integer">69</ebg:order>
    <skos:example>For OCORP, 'https://opencorporates.com/companies/{}'      returns company data with MIME type 'text/html'</skos:example>
    <rdfs:label>URL template</rdfs:label>
    <rdfs:isDefinedBy rdf:resource="http://data.businessgraph.io/ontology#"/>
  </rdf:Description>
  <rdf:Description rdf:about="http://www.w3.org/ns/regorg#orgStatus">
    <skos:scopeNote>A Best Practice for recording status levels is to use the relevant jurisdiction's terms and to encode these in a SKOS Concept Scheme [rov:].</skos:scopeNote>
    <skos:example>'Actively trading' vs 'Dormant' vs 'Unregistered' could be considered the 3 main divisions of Status.</skos:example>
    <rdf:type rdf:resource="http://www.w3.org/2002/07/owl#ObjectProperty"/>
    <rdfs:label>status</rdfs:label>
    <skos:scopeNote>There is no globally accepted list of company states. For Inactive, some look at hard evidence (the company has been deregistered), others at a long period of inactivity (dormant). Because of this, a user cannot assume that Active and Inactive are opposites.</skos:scopeNote>
    <ebg:order rdf:datatype="http://www.w3.org/2001/XMLSchema#integer">8</ebg:order>
    <skos:definition>Flag that identifies whether a company is active or not [ebg:]. The operational and/or legal registration status of the entity [lei:].</skos:definition>
    <skos:example>'Normal Activity': does appear to have cross-border usefulness and this should be used in preference to terms like 'trading' or 'operating' [rov:].</skos:example>
    <schema:domainIncludes rdf:resource="http://www.w3.org/ns/regorg#RegisteredOrganization"/>
    <skos:example>'insolvent', 'bankrupt', 'in receivership': likely to mean slightly different things with different legal implications in different jurisdictions [rov:].</skos:example>
  </rdf:Description>
  <rdf:Description rdf:about="http://schema.org/inLanguage">
    <ebg:order rdf:datatype="http://www.w3.org/2001/XMLSchema#integer">68</ebg:order>
    <skos:scopeNote>Use a valid [iana:] language code from the IETF BCP 47 standard</skos:scopeNote>
    <skos:definition>Language of the web resource</skos:definition>
    <rdfs:label>language</rdfs:label>
    <rdf:type rdf:resource="http://www.w3.org/2002/07/owl#DatatypeProperty"/>
  </rdf:Description>
  <rdf:Description rdf:about="http://data.businessgraph.io/ontology#orgStatusText">
    <rdf:type rdf:resource="http://www.w3.org/2002/07/owl#DatatypeProperty"/>
    <schema:domainIncludes rdf:resource="http://www.w3.org/ns/regorg#RegisteredOrganization"/>
    <skos:example xml:lang="el">Πτώχευση</skos:example>
    <skos:example xml:lang="en">Dissolved</skos:example>
    <skos:definition>Company status as it comes from the original register (free text).</skos:definition>
    <skos:example xml:lang="en">Revoked</skos:example>
    <rdfs:isDefinedBy rdf:resource="http://data.businessgraph.io/ontology#"/>
    <ebg:order rdf:datatype="http://www.w3.org/2001/XMLSchema#integer">9</ebg:order>
    <skos:example xml:lang="fr">Situation Normale</skos:example>
    <rdfs:label>status text</rdfs:label>
    <skos:scopeNote>Include valid language tag (see [iana:] for list).</skos:scopeNote>
    <skos:scopeNote>If both Status and Status Text are present, they must express compatible values (Status Text may be a finer-granularity value).</skos:scopeNote>
    <skos:example xml:lang="es">En Liquidacion</skos:example>
    <schema:rangeIncludes rdf:resource="http://www.w3.org/1999/02/22-rdf-syntax-ns#langString"/>
    <skos:example xml:lang="en">Inactive</skos:example>
  </rdf:Description>
  <rdf:Description rdf:about="http://data.businessgraph.io/ontology#level">
    <ebg:order rdf:datatype="http://www.w3.org/2001/XMLSchema#integer">109</ebg:order>
    <schema:rangeIncludes rdf:resource="http://www.w3.org/2001/XMLSchema#integer"/>
    <schema:domainIncludes rdf:resource="http://www.w3.org/2004/02/skos/core#Concept"/>
    <rdfs:comment>Hierarchical level of a thesaurus concept</rdfs:comment>
    <rdfs:label>concept level</rdfs:label>
    <rdfs:isDefinedBy rdf:resource="http://data.businessgraph.io/ontology#"/>
    <rdf:type rdf:resource="http://www.w3.org/2002/07/owl#DatatypeProperty"/>
  </rdf:Description>
  <rdf:Description rdf:about="http://www.w3.org/ns/locn#Address">
    <skos:scopeNote>Every data provider should strive to provide NUTS3 for each address. This can be done in cooperation, using the techniques described in Address Calculations above.</skos:scopeNote>
    <skos:scopeNote>Should be linked as registered address (one) or other address (multiple).</skos:scopeNote>
    <skos:definition>Mailing or physical address of a company</skos:definition>
    <rdfs:label>Address</rdfs:label>
    <rdf:type rdf:resource="http://www.w3.org/2000/01/rdf-schema#Class"/>
  </rdf:Description>
  <rdf:Description rdf:about="http://rdfdata.eionet.europa.eu/ramon/ontology/NUTSRegion">
    <rdfs:label>NUTS Region</rdfs:label>
    <rdf:type rdf:resource="http://www.w3.org/2000/01/rdf-schema#Class"/>
  </rdf:Description>
  <rdf:Description rdf:about="http://data.businessgraph.io/ontology#LAURegion">
    <skos:example>LAU2 BG: Населени места (Naseleni mesta)</skos:example>
    <skos:example>LAU2 ME: Насеља (Naselja)</skos:example>
    <skos:example>LAU1 CH: Bezirke Districts Distretti</skos:example>
    <skos:example>LAU1 DK: Kommuner</skos:example>
    <skos:example>LAU1 CY: Επαρχίες (Eparchies)</skos:example>
    <dct:source rdf:resource="http://ec.europa.eu/eurostat/web/nuts/correspondence-tables/national-structures-non-eu"/>
    <skos:example>LAU1 CZ: Okresy</skos:example>
    <skos:example>LAU1 TR: Ilceler</skos:example>
    <skos:example>LAU1 SI: Upravne enote</skos:example>
    <skos:example>LAU2 TR: Köy</skos:example>
    <skos:example>LAU2 SE: Kommuner</skos:example>
    <skos:example>LAU1 LT: Savivaldybės</skos:example>
    <skos:example>LAU1 MK: Општини (Opštini)</skos:example>
    <skos:example>LAU2 IS: Sveitarfélög</skos:example>
    <skos:example>LAU2 FR: Communes</skos:example>
    <skos:example>LAU2 NL: Gemeenten</skos:example>
    <skos:example>LAU2 AL: Bashki / Komunë</skos:example>
    <skos:example>LAU2 LU: Communes</skos:example>
    <skos:example>LAU1 UK: Lower tier authorities (districts) or individual unitary authorities;  Individual unitary authorities or LECs (or parts thereof); Districts</skos:example>
    <skos:example>LAU1 IS: Landsvædi</skos:example>
    <skos:example>LAU2 PT: Freguesias</skos:example>
    <rdf:type rdf:resource="http://www.w3.org/2000/01/rdf-schema#Class"/>
    <skos:example>LAU1 EE: Maakond</skos:example>
    <skos:example>LAU2 LV: Republikas pilsētas, novadi</skos:example>
    <skos:example>LAU1 ME: Општине (Opštine)</skos:example>
    <skos:example>LAU2 SK: Obce</skos:example>
    <skos:example>LAU2 EE: Linn, vald</skos:example>
    <skos:example>LAU1 FR: Cantons de rattachement</skos:example>
    <dct:source rdf:resource="http://ec.europa.eu/eurostat/web/nuts/national-structures-eu"/>
    <skos:example>LAU1 NO: Økonomiske regioner</skos:example>
    <skos:example>LAU2 ES: Municipios</skos:example>
    <skos:example>LAU2 BE: Gemeenten / Communes</skos:example>
    <skos:example>LAU1 DE: Verwaltungs- gemeinschaften</skos:example>
    <skos:example>LAU2 LI: Gemeinden</skos:example>
    <skos:example>LAU2 FI: Kunnat / Kommuner</skos:example>
    <skos:example>LAU1 BG: Общини (Obshtini)</skos:example>
    <skos:example>LAU2 CY: Δήμοι, Κοινότητες (Dimoi, koinotites)</skos:example>
    <skos:example>LAU2 RO: Comuni + Municipiu + Orase</skos:example>
    <skos:example>LAU2 SI: Občine</skos:example>
    <skos:example>LAU1 HU: Statisztikai kistérségek</skos:example>
    <skos:example>LAU2 IE: Electoral Districts</skos:example>
    <skos:example>LAU2 EL: Δημοτικές / Τοπικές Κοινότητες (Dimotikes / Topikes Koinotites - Municipal  / Local Communes)</skos:example>
    <skos:example>LAU2 UK: Wards (or parts thereof)</skos:example>
    <rdfs:isDefinedBy rdf:resource="http://data.businessgraph.io/ontology#"/>
    <skos:example>LAU2 MK: Населени места (Naseleni mesta)</skos:example>
    <skos:example>LAU2 CZ: Obce</skos:example>
    <skos:example>LAU1 LI: Landschaften</skos:example>
    <skos:example>LAU2 DK: Sogne</skos:example>
    <skos:example>LAU2 IT: Comuni</skos:example>
    <skos:example>LAU1 MT: Distretti</skos:example>
    <skos:example>LAU2 HR: Gradovi i općine</skos:example>
    <skos:example>LAU2 LT: Seniūnijos</skos:example>
    <skos:example>LAU2 CH: Gemeinden Communes Comuni</skos:example>
    <rdfs:comment>Local Administrative Unit</rdfs:comment>
    <skos:example>LAU1 PL: Powiaty i miasta na prawach powiatu</skos:example>
    <rdfs:label>LAU Region</rdfs:label>
    <skos:example>LAU1 LU: Cantons</skos:example>
    <skos:example>LAU1 FI: Seutukunnat / Ekonomiska regioner</skos:example>
    <skos:example>LAU2 AT: Gemeinden</skos:example>
    <skos:example>LAU1 IE: Counties, Cities</skos:example>
    <skos:example>LAU2 NO: Kommuner</skos:example>
    <skos:example>LAU2 PL: Gminy</skos:example>
    <skos:example>LAU2 MT: Kunsilli</skos:example>
    <skos:example>LAU2 DE: Gemeinden</skos:example>
    <skos:example>LAU1 EL: Δήμοι, Κοινότητες (Demoi, Koinotites)</skos:example>
    <skos:example>LAU1 PT: Concelhos - Munícipios</skos:example>
    <skos:example>LAU2 HU: Települések</skos:example>
    <skos:example>LAU1 SK: Okresy</skos:example>
  </rdf:Description>
  <rdf:Description rdf:about="http://dbpedia.org/ontology/jurisdiction">
    <skos:example>BG has many types, including a number of European companies.</skos:example>
    <skos:example>NO has type NUF 'Norskregistrert utenlandsk foretak'.</skos:example>
    <skos:scopeNote>For Europe, this is a country, even for Germany that has 166 separate registers (see Registration Authorities List).  Many jurisdictions register foreign companies that are incorporated and fully owned in another country. EBG collects all registrations from each register and doesn't attempt to match foreign companies across jurisdictions.</skos:scopeNote>
    <skos:definition>Jurisdiction in which the company is registered or to which the identifier system applies.</skos:definition>
    <schema:rangeIncludes rdf:resource="http://www.w3.org/2001/XMLSchema#string"/>
    <rdfs:label>jurisdiction</rdfs:label>
    <schema:domainIncludes rdf:resource="http://www.w3.org/ns/regorg#RegisteredOrganization"/>
    <ebg:order rdf:datatype="http://www.w3.org/2001/XMLSchema#integer">22</ebg:order>
    <schema:domainIncludes rdf:resource="http://data.businessgraph.io/ontology#IdentifierSystem"/>
    <rdf:type rdf:resource="http://www.w3.org/2002/07/owl#DatatypeProperty"/>
    <skos:scopeNote>If we know the official legal ID of the company, the jurisdiction code and official ID are used to form the company URL.</skos:scopeNote>
  </rdf:Description>
  <rdf:Description rdf:about="http://data.businessgraph.io/ontology#adminUnitL3">
    <ebg:order rdf:datatype="http://www.w3.org/2001/XMLSchema#integer">31</ebg:order>
    <schema:domainIncludes rdf:resource="http://www.w3.org/ns/locn#Address"/>
    <schema:rangeIncludes rdf:resource="http://rdfdata.eionet.europa.eu/ramon/ontology/NUTSRegion"/>
    <skos:example>nuts:ITC2 Valle d'Aosta/Vallée d'Aoste</skos:example>
    <rdf:type rdf:resource="http://www.w3.org/2002/07/owl#ObjectProperty"/>
    <skos:scopeNote>Use a valid NUTS region. Eg Trentino-Alto Adige/Sudtirol (taken from the Geonames hierarchy above) is not a NUTS region.</skos:scopeNote>
    <skos:example>nuts:ITH2 Provincia Autonoma di Trento</skos:example>
    <skos:definition>NUTS2 (administrative region) of the address.</skos:definition>
    <rdfs:label>admin unit level 3</rdfs:label>
    <rdfs:isDefinedBy rdf:resource="http://data.businessgraph.io/ontology#"/>
  </rdf:Description>
  <rdf:Description rdf:about="http://schema.org/dissolutionDate">
    <skos:example rdf:datatype="http://www.w3.org/2001/XMLSchema#date">2010-11-18</skos:example>
    <schema:rangeIncludes rdf:resource="http://www.w3.org/2001/XMLSchema#gYearMonth"/>
    <rdf:type rdf:resource="http://www.w3.org/2002/07/owl#DatatypeProperty"/>
    <schema:rangeIncludes rdf:resource="http://www.w3.org/2001/XMLSchema#date"/>
    <ebg:order rdf:datatype="http://www.w3.org/2001/XMLSchema#integer">15</ebg:order>
    <schema:rangeIncludes rdf:resource="http://www.w3.org/2001/XMLSchema#gYear"/>
    <skos:scopeNote>Should have a valid XSD datatype.</skos:scopeNote>
    <schema:domainIncludes rdf:resource="http://www.w3.org/ns/regorg#RegisteredOrganization"/>
    <rdfs:label>dissolution date</rdfs:label>
    <skos:example rdf:datatype="http://www.w3.org/2001/XMLSchema#gYearMonth">2010-11</skos:example>
    <skos:example rdf:datatype="http://www.w3.org/2001/XMLSchema#gYear">2010</skos:example>
    <skos:definition>Date when the organization was dissolved or removed from register.</skos:definition>
  </rdf:Description>
  <rdf:Description rdf:about="http://www.w3.org/ns/org#hasRegisteredSite">
    <ebg:order rdf:datatype="http://www.w3.org/2001/XMLSchema#integer">23</ebg:order>
    <skos:scopeNote>org:hasRegisteredSite leads to a node with types org:Site and locn:Address that has self-link org:siteAddress.</skos:scopeNote>
    <skos:definition>Public legal address where legal papers can be served.</skos:definition>
    <rdfs:label>registered site/address</rdfs:label>
    <schema:rangeIncludes rdf:resource="http://www.w3.org/ns/locn#Address"/>
    <schema:domainIncludes rdf:resource="http://www.w3.org/ns/regorg#RegisteredOrganization"/>
    <rdf:type rdf:resource="http://www.w3.org/2002/07/owl#ObjectProperty"/>
  </rdf:Description>
  <rdf:Description rdf:about="http://www.w3.org/ns/locn#postName">
    <rdfs:label>post name (locality/city/settlement)</rdfs:label>
    <schema:domainIncludes rdf:resource="http://www.w3.org/ns/locn#Address"/>
    <schema:rangeIncludes rdf:resource="http://www.w3.org/1999/02/22-rdf-syntax-ns#langString"/>
    <schema:rangeIncludes rdf:resource="http://www.w3.org/2001/XMLSchema#string"/>
    <ebg:order rdf:datatype="http://www.w3.org/2001/XMLSchema#integer">35</ebg:order>
    <skos:scopeNote>Provide a language tag if possible. If both ebg:adminUnitL6 and locn:postName are specified, they should correspond to each other.</skos:scopeNote>
    <rdf:type rdf:resource="http://www.w3.org/2002/07/owl#DatatypeProperty"/>
    <skos:definition>Locality/City/Settlement of the address, free text.</skos:definition>
    <skos:example xml:lang="bg">Тренто</skos:example>
    <skos:example xml:lang="it">Trento</skos:example>
  </rdf:Description>
  <rdf:Description rdf:about="http://www.w3.org/ns/locn#addressArea">
    <ebg:order rdf:datatype="http://www.w3.org/2001/XMLSchema#integer">36</ebg:order>
    <skos:scopeNote>Not likely to appear, but we have Coordinate resolution corresponding to this field.</skos:scopeNote>
    <skos:definition>Part of a city, village or neighborhood.</skos:definition>
    <rdfs:label>address area (neighbourhood/quarter)</rdfs:label>
    <schema:rangeIncludes rdf:resource="http://www.w3.org/1999/02/22-rdf-syntax-ns#langString"/>
    <schema:rangeIncludes rdf:resource="http://www.w3.org/2001/XMLSchema#string"/>
    <schema:domainIncludes rdf:resource="http://www.w3.org/ns/locn#Address"/>
    <rdf:type rdf:resource="http://www.w3.org/2002/07/owl#DatatypeProperty"/>
  </rdf:Description>
  <rdf:Description rdf:about="http://data.businessgraph.io/ontology#foundingYear">
    <ebg:order rdf:datatype="http://www.w3.org/2001/XMLSchema#integer">14</ebg:order>
    <skos:scopeNote>Used for faceting.</skos:scopeNote>
    <skos:definition>Year the organization was created, as integer.</skos:definition>
    <rdfs:label>founding year</rdfs:label>
    <schema:rangeIncludes rdf:resource="http://www.w3.org/2001/XMLSchema#integer"/>
    <schema:domainIncludes rdf:resource="http://www.w3.org/ns/regorg#RegisteredOrganization"/>
    <rdf:type rdf:resource="http://www.w3.org/2002/07/owl#DatatypeProperty"/>
  </rdf:Description>
  <rdf:Description rdf:about="http://data.businessgraph.io/dataset/partition">
    <skos:scopeNote>Used to describe dataset statistics. Not downloadable separately.</skos:scopeNote>
    <skos:prefLabel>Partition</skos:prefLabel>
    <skos:inScheme rdf:resource="http://data.businessgraph.io/dataset/"/>
    <rdfs:isDefinedBy rdf:resource="http://data.businessgraph.io/ontology#"/>
    <rdf:type rdf:resource="http://www.w3.org/2004/02/skos/core#Concept"/>
  </rdf:Description>
  <rdf:Description rdf:about="http://data.businessgraph.io/ontology#">
    <dct:publisher rdf:resource="http://businessgraph.io"/>
    <dct:created rdf:datatype="http://www.w3.org/2001/XMLSchema#date">2017-07-11</dct:created>
    <rdfs:seeAlso rdf:resource="https://docs.google.com/document/d/1dhMOTlIOC6dOK_jksJRX0CB-GIRoiYY6fWtCnZArUhU/edit"/>
    <dct:type rdf:resource="http://purl.org/adms/assettype/Ontology"/>
    <dct:creator rdf:resource="mailto:vladimir.alexiev@ontotext.com"/>
    <foaf:homepage rdf:resource="http://businessgraph.io"/>
    <owl:versionInfo>1.0</owl:versionInfo>
    <rdfs:comment>The euBusinessGraph (`ebg:`) ontology represents companies, type/status/economic classification, addresses, identifiers, (and soon) directors and CEOs, dataset offerings.&#xD;
&#xD;
It uses `schema:domain/rangeIncludes` (which are polymorphic) to describe which properties are applicable to a class, &#xD;
rather than `rdfs:domain/rainge` (which are monomorphic) to prescribe what classes must be applied to each node using a property.&#xD;
We find that this enables more flexible reuse and combination of different ontologies.&#xD;
We reuse the following ontologies and nomenclatures, and extend them where appropriate with classes and properties:&#xD;
- W3C Org, W3C RegOrg (basic company data), &#xD;
- W3C Time (officer membership), &#xD;
- W3C Locn (addresses),&#xD;
- schema.org (domain/rangeIncludes and various properties)&#xD;
- DBpedia ontology (jurisdiction)&#xD;
- NGEO and Spatial (NUTS administrative divisions)&#xD;
- ADMS (identifiers), &#xD;
- FOAF, SIOC (blog posts),&#xD;
- RAMON, SKOS (NACE economic classifications and various nomenclatures),&#xD;
- VOID (dataset descriptions).&#xD;
This is only a reference. See more detail in the [EBG Semantic Model](https://docs.google.com/document/d/1dhMOTlIOC6dOK_jksJRX0CB-GIRoiYY6fWtCnZArUhU/edit) google document, which includes an informative description of classes and properties, gives examples and data provider rules, and provides more schema and instance diagrams.&#xD;
&#xD;
A couple of illustrations follow.&#xD;
&#xD;
#### Company&#xD;
![](https://raw.githubusercontent.com/euBusinessGraph/eubg-data/master/model/images/company.png)&#xD;
&#xD;
#### Identifier System&#xD;
![](https://raw.githubusercontent.com/euBusinessGraph/eubg-data/master/model/images/Identifiers-ORM.png)&#xD;
&#xD;
#### Dataset Descriptions&#xD;
Dataset Hierarchy&#xD;
&#xD;
![](https://raw.githubusercontent.com/euBusinessGraph/eubg-data/master/model/images/dataset-hierarchy.png)&#xD;
&#xD;
Dataset Metadata Details&#xD;
&#xD;
![](https://raw.githubusercontent.com/euBusinessGraph/eubg-data/master/model/images/dataset-details.png)&#xD;
&#xD;
Dataset Sources&#xD;
&#xD;
![](https://raw.githubusercontent.com/euBusinessGraph/eubg-data/master/model/images/dataset-sources.png)&#xD;
&#xD;
Dataset Statistics&#xD;
&#xD;
![](https://raw.githubusercontent.com/euBusinessGraph/eubg-data/master/model/images/dataset-stats.png)&#xD;
&#xD;
#### Officers&#xD;
In development. Below are 5 examples from 2 datasets (OCORP GB and ONTO BG). See [officers.md](https://github.com/euBusinessGraph/eubg-data/blob/master/model/officers.md) for some notes.&#xD;
&#xD;
![](https://raw.githubusercontent.com/euBusinessGraph/eubg-data/master/model/images/officers.png)&#xD;
&#xD;
</rdfs:comment>
    <dct:modified rdf:datatype="http://www.w3.org/2001/XMLSchema#date">2018-02-21</dct:modified>
    <dct:title>euBusinessGraph ontology</dct:title>
    <dct:creator rdf:resource="http://businessgraph.io"/>
    <rdf:type rdf:resource="http://www.w3.org/2002/07/owl#Ontology"/>
    <dct:creator rdf:resource="http://ontotext.com"/>
    <vann:preferredNamespacePrefix>ebg</vann:preferredNamespacePrefix>
    <vann:preferredNamespaceUri>http://data.businessgraph.io/ontology#</vann:preferredNamespaceUri>
    <dct:status rdf:resource="http://purl.org/adms/status/UnderDevelopment"/>
  </rdf:Description>
  <rdf:Description rdf:about="http://data.businessgraph.io/ontology#validationRule">
    <rdfs:isDefinedBy rdf:resource="http://data.businessgraph.io/ontology#"/>
    <rdfs:label>validation rule</rdfs:label>
    <skos:scopeNote>Can be in the form of webpage, PDF document, RDF shape, etc. Multiple values about the same validation rule are ok.</skos:scopeNote>
    <skos:definition>URL providing human or machine-readable rule(s) for validating identifiers in the system</skos:definition>
    <schema:domainIncludes rdf:resource="http://data.businessgraph.io/ontology#IdentifierSystem"/>
    <skos:example>http://bsv-bg.com/контролни-цифри-ползвани-в-българия/ describes the BG EIK checksum algorithm in HTML</skos:example>
    <ebg:order rdf:datatype="http://www.w3.org/2001/XMLSchema#integer">60</ebg:order>
    <skos:example>http://www.nsi.bg/sites/default/files/konkursi/RGP_OPAK_2014_Annex_6.pdf describes the BG EIK checksum algorithm in PDF. It is by an official source, but is less convenient</skos:example>
    <schema:rangeIncludes rdf:resource="http://www.w3.org/1999/02/22-rdf-syntax-ns#Resource"/>
    <rdf:type rdf:resource="http://www.w3.org/2002/07/owl#ObjectProperty"/>
  </rdf:Description>
  <rdf:Description rdf:about="http://data.businessgraph.io/resolution/">
    <dct:publisher rdf:resource="http://businessgraph.io"/>
    <dct:creator rdf:resource="http://businessgraph.io"/>
    <rdfs:comment>Resolution of a geographic coordinate location: from continent (least precise) to individual house number (most precise)</rdfs:comment>
    <rdfs:label>Geo Coordinate Resolution</rdfs:label>
    <rdfs:isDefinedBy rdf:resource="http://data.businessgraph.io/ontology#"/>
    <rdf:type rdf:resource="http://www.w3.org/2004/02/skos/core#ConceptScheme"/>
  </rdf:Description>
  <rdf:Description rdf:about="http://data.businessgraph.io/ontology#adminUnitL6">
    <ebg:order rdf:datatype="http://www.w3.org/2001/XMLSchema#integer">34</ebg:order>
    <skos:definition>LAU2 (Municipality/Commune/Settlement) of the address.</skos:definition>
    <rdfs:isDefinedBy rdf:resource="http://data.businessgraph.io/ontology#"/>
    <skos:scopeNote>Some countries (e.g. Bulgaria) use both LAU1 and LAU2 levels. Others (e.g. Italy) use only LAU2.</skos:scopeNote>
    <rdfs:label>admin unit level 6</rdfs:label>
    <schema:rangeIncludes rdf:resource="http://data.businessgraph.io/ontology#LAURegion"/>
    <schema:domainIncludes rdf:resource="http://www.w3.org/ns/locn#Address"/>
    <rdf:type rdf:resource="http://www.w3.org/2002/07/owl#ObjectProperty"/>
  </rdf:Description>
  <rdf:Description rdf:about="http://purl.org/dc/terms/isPartOf">
    <ebg:order rdf:datatype="http://www.w3.org/2001/XMLSchema#integer">71</ebg:order>
    <skos:definition>The Identifier System this identifier is part of</skos:definition>
    <schema:rangeIncludes rdf:resource="http://data.businessgraph.io/ontology#IdentifierSystem"/>
    <schema:domainIncludes rdf:resource="http://www.w3.org/ns/adms#Identifier"/>
    <rdfs:label>is part of</rdfs:label>
    <rdf:type rdf:resource="http://www.w3.org/2002/07/owl#ObjectProperty"/>
  </rdf:Description>
  <rdf:Description rdf:about="http://www.w3.org/ns/locn#adminUnitL2">
    <ebg:order rdf:datatype="http://www.w3.org/2001/XMLSchema#integer">30</ebg:order>
    <skos:example>nuts:ITC NORD-OVEST (Nord-est).</skos:example>
    <skos:definition>NUTS1 (Macroregion) of the address.</skos:definition>
    <rdfs:label>admin unit level 2</rdfs:label>
    <schema:rangeIncludes rdf:resource="http://rdfdata.eionet.europa.eu/ramon/ontology/NUTSRegion"/>
    <schema:domainIncludes rdf:resource="http://www.w3.org/ns/locn#Address"/>
    <rdf:type rdf:resource="http://www.w3.org/2002/07/owl#ObjectProperty"/>
  </rdf:Description>
  <rdf:Description rdf:about="http://www.w3.org/ns/person#Person">
    <skos:definition>An officer is a natural person (as opposed to a legal person) [person:] that has a high-level management role in a Company (e.g., the CEO, treasurer and chief financial officer). Despite their high status, they typically serve at the will of the corporate directors, who can fire or replace them. Officers can also be shareholders and directors but don't necessarily have to be. They have the authority to act on behalf of the corporation, including contract authority.</skos:definition>
    <rdfs:label>Officer</rdfs:label>
    <rdf:type rdf:resource="http://www.w3.org/2000/01/rdf-schema#Class"/>
  </rdf:Description>
  <rdf:Description rdf:about="http://schema.org/author">
    <schema:domainIncludes rdf:resource="http://data.businessgraph.io/ontology#IdentifierSystem"/>
    <rdfs:label>author</rdfs:label>
    <ebg:order rdf:datatype="http://www.w3.org/2001/XMLSchema#integer">45</ebg:order>
    <skos:definition>Agent who specified the rules and organization of the identifier system</skos:definition>
    <skos:example>W3C or TimBL specified web URLs</skos:example>
    <rdf:type rdf:resource="http://www.w3.org/2002/07/owl#ObjectProperty"/>
    <schema:rangeIncludes rdf:resource="http://schema.org/Person"/>
    <skos:example>W3C specified web URL rules</skos:example>
    <skos:definition>Agent who specified the rules and organisation of an Identifier System</skos:definition>
    <skos:example>Dun and Bradstreet specified DUNS numbers</skos:example>
    <schema:rangeIncludes rdf:resource="http://schema.org/Organization"/>
    <skos:example>GLEIF specified GLEI</skos:example>
    <skos:example>GLEIF specified LEI structure and rules, then formalied it as ISO 17442:2012 Financial services -- Legal Entity Identifier (LEI)</skos:example>
  </rdf:Description>
  <rdf:Description rdf:about="http://data.businessgraph.io/ontology#IdentifierWebResource">
    <skos:scopeNote>This class has ebg:urlTemplate, and the same general properties as Web Resource: name, MIME type, language</skos:scopeNote>
    <skos:definition>URL template complemented with name, language and MIME type(s) to specify what the URL is about. Substitute the identifier value into the template</skos:definition>
    <rdfs:label>Identifier Web Resource</rdfs:label>
    <rdfs:isDefinedBy rdf:resource="http://data.businessgraph.io/ontology#"/>
    <rdf:type rdf:resource="http://www.w3.org/2000/01/rdf-schema#Class"/>
  </rdf:Description>
  <rdf:Description rdf:about="http://rdfdata.eionet.europa.eu/ramon/ontology/code">
    <ebg:order rdf:datatype="http://www.w3.org/2001/XMLSchema#integer">111</ebg:order>
    <schema:rangeIncludes rdf:resource="http://www.w3.org/2001/XMLSchema#string"/>
    <schema:domainIncludes rdf:resource="http://data.businessgraph.io/ontology#LAURegion"/>
    <schema:domainIncludes rdf:resource="http://rdfdata.eionet.europa.eu/ramon/ontology/NUTSRegion"/>
    <rdfs:comment>NUTS/LAU Code of an administrative region</rdfs:comment>
    <rdfs:label>code</rdfs:label>
    <rdf:type rdf:resource="http://www.w3.org/2002/07/owl#DatatypeProperty"/>
  </rdf:Description>
  <rdf:Description rdf:about="http://www.w3.org/ns/org#siteAddress">
    <ebg:order rdf:datatype="http://www.w3.org/2001/XMLSchema#integer">27</ebg:order>
    <skos:scopeNote>EBG doesn't need the distinction between org:Site and locn:Address, so we use one node having both types, and a self-link org:siteAddress</skos:scopeNote>
    <schema:rangeIncludes rdf:resource="http://www.w3.org/ns/locn#Address"/>
    <schema:domainIncludes rdf:resource="http://www.w3.org/ns/org#Site"/>
    <rdfs:label>site's address</rdfs:label>
    <rdf:type rdf:resource="http://www.w3.org/2002/07/owl#ObjectProperty"/>
  </rdf:Description>
  <rdf:Description rdf:about="http://www.w3.org/2004/02/skos/core#altLabel">
    <skos:definition>Informal/popular name of the company (also called Trading As) [ebg:]. Sometimes (e.g., when the legal name is very long) people refer to a company using a different, informal version [ebg:]. Some jurisdictions recognize concepts such as a trading name or alternative forms of a legal entity's name [rov:].</skos:definition>
    <skos:scopeNote>Don't allow leading, trailing and two consecutive spaces.</skos:scopeNote>
    <rdf:type rdf:resource="http://www.w3.org/2002/07/owl#DatatypeProperty"/>
    <skos:scopeNote>Provide a valid language tag if possible (see [iana:] for a list).</skos:scopeNote>
    <skos:scopeNote>Do not use this property to record translations of the primary legal name [rov:].</skos:scopeNote>
    <ebg:order rdf:datatype="http://www.w3.org/2001/XMLSchema#integer">2</ebg:order>
    <schema:domainIncludes rdf:resource="http://www.w3.org/ns/regorg#RegisteredOrganization"/>
    <skos:scopeNote>Do not emit such name if it's equal to the legal name [ebg:]. </skos:scopeNote>
    <rdfs:label>alt label (trade name)</rdfs:label>
    <skos:example xml:lang="en">OpenCorporates</skos:example>
    <schema:rangeIncludes rdf:resource="http://www.w3.org/1999/02/22-rdf-syntax-ns#langString"/>
    <skos:example xml:lang="it">PROGIENE 2.000 I PROFESSIONISTI DELL'IGIENE SRL</skos:example>
    <schema:rangeIncludes rdf:resource="http://www.w3.org/2001/XMLSchema#string"/>
  </rdf:Description>
  <rdf:Description rdf:about="http://data.businessgraph.io/nace/">
    <rdfs:isDefinedBy rdf:resource="http://data.businessgraph.io/ontology#"/>
    <dct:license rdf:resource="https://opendatacommons.org/licenses/by/"/>
    <rdf:type rdf:resource="http://www.w3.org/2004/02/skos/core#ConceptScheme"/>
    <dct:creator rdf:resource="http://businessgraph.io"/>
    <dct:issued rdf:datatype="http://www.w3.org/2001/XMLSchema#date">2017-07-28</dct:issued>
    <rdfs:comment>Statistical Classification of Economic Activities in the European Community, Rev. 2 (2008)</rdfs:comment>
    <dct:source rdf:resource="http://ec.europa.eu/eurostat/ramon/nomenclatures/index.cfm?TargetUrl=LST_CLS_DLD&amp;StrNom=NACE_REV2&amp;StrLanguageCode=EN&amp;StrLayoutCode=HIERARCHIC#"/>
    <dct:created rdf:datatype="http://www.w3.org/2001/XMLSchema#date">2017-07-28</dct:created>
    <dct:publisher rdf:resource="http://businessgraph.io"/>
    <rdfs:label>NACE 2 classification</rdfs:label>
  </rdf:Description>
  <rdf:Description rdf:about="http://data.businessgraph.io/ontology#isPubliclyTraded">
    <ebg:order rdf:datatype="http://www.w3.org/2001/XMLSchema#integer">7</ebg:order>
    <skos:definition>Whether the company is publicly traded (listed at a stock exchange) [ebg:].</skos:definition>
    <rdfs:label>is publicly traded</rdfs:label>
    <schema:rangeIncludes rdf:resource="http://www.w3.org/2001/XMLSchema#boolean"/>
    <schema:domainIncludes rdf:resource="http://www.w3.org/ns/regorg#RegisteredOrganization"/>
    <rdfs:isDefinedBy rdf:resource="http://data.businessgraph.io/ontology#"/>
    <rdf:type rdf:resource="http://www.w3.org/2002/07/owl#DatatypeProperty"/>
  </rdf:Description>
  <rdf:Description rdf:about="http://schema.org/publisher">
    <skos:example>GLEIF publishes the GLEI openly, with a full dump that is updated regularly, which has spurned re-publishers such as http://openleis.com/ and http://glei.info.</skos:example>
    <schema:rangeIncludes rdf:resource="http://schema.org/Person"/>
    <ebg:order rdf:datatype="http://www.w3.org/2001/XMLSchema#integer">47</ebg:order>
    <schema:rangeIncludes rdf:resource="http://schema.org/Organization"/>
    <rdf:type rdf:resource="http://www.w3.org/2002/07/owl#DatatypeProperty"/>
    <skos:scopeNote>Different functions and distributions can be considered (e.g. search or other query, per-company web resources, full download). Often but not always the issuer is also the publisher.</skos:scopeNote>
    <rdfs:label>identifier system publisher</rdfs:label>
    <skos:example>Companies House and BRC publish the UK and NO registers openly.</skos:example>
    <skos:definition>Agent that publishes an identifier database (register) in some form (i.e., printed form, online)</skos:definition>
    <schema:domainIncludes rdf:resource="http://data.businessgraph.io/ontology#IdentifierSystem"/>
    <skos:example>DUNS numbers are not openly published.</skos:example>
  </rdf:Description>
  <rdf:Description rdf:about="http://www.w3.org/1999/02/22-rdf-syntax-ns#langString">
    <rdfs:label>Language-Tagged String</rdfs:label>
    <rdf:type rdf:resource="http://www.w3.org/2000/01/rdf-schema#Datatype"/>
  </rdf:Description>
  <rdf:Description rdf:about="http://schema.org/longitude">
    <ebg:order rdf:datatype="http://www.w3.org/2001/XMLSchema#integer">43</ebg:order>
    <skos:scopeNote>If no coordinates are available, do not make a schema:GeoCoordinates node.</skos:scopeNote>
    <skos:scopeNote>Coordinates must be expressed in the WGS 84 system.</skos:scopeNote>
    <rdfs:label>longitude</rdfs:label>
    <schema:rangeIncludes rdf:resource="http://www.w3.org/2001/XMLSchema#decimal"/>
    <schema:domainIncludes rdf:resource="http://schema.org/GeoCoordinates"/>
    <rdf:type rdf:resource="http://www.w3.org/2002/07/owl#DatatypeProperty"/>
  </rdf:Description>
  <rdf:Description rdf:about="http://schema.org/url">
    <schema:domainIncludes rdf:resource="http://data.businessgraph.io/ontology#WebResource"/>
    <skos:definition>Website pertaining to the company or URL of a web resource</skos:definition>
    <skos:example>For system BG TR, &lt;https://brra.bg&gt; with language "bg" and MIME type "text/html" is the homepage</skos:example>
    <skos:example rdf:resource="http://www.comune.trento.it"/>
    <skos:example>For system BE Banque-Carrefour des Entreprises, &lt;https://kbopub.economie.fgov.be/kbopub/zoeknummerform.html&gt; with MIME type "application/x-search" is the search URL</skos:example>
    <rdfs:label>website</rdfs:label>
    <ebg:order rdf:datatype="http://www.w3.org/2001/XMLSchema#integer">18</ebg:order>
    <rdf:type rdf:resource="http://www.w3.org/2002/07/owl#ObjectProperty"/>
    <schema:domainIncludes rdf:resource="http://www.w3.org/ns/regorg#RegisteredOrganization"/>
    <skos:example>For system BG TR, &lt;http://opendata.government.bg/dataset/tbprobckn-pernctbp&gt; with language "bg" and MIME type "application/xml" is open data download in XML</skos:example>
    <schema:rangeIncludes rdf:resource="http://www.w3.org/1999/02/22-rdf-syntax-ns#Resource"/>
  </rdf:Description>
  <rdf:Description rdf:about="http://www.w3.org/2004/02/skos/core#prefLabel">
    <ebg:order rdf:datatype="http://www.w3.org/2001/XMLSchema#integer">1</ebg:order>
    <skos:scopeNote>Used as a display name of the company or identifier system. For companies we usually pick one of the Registered Names (English if present, else at random). For identifier systems, we use a commonly used English name.</skos:scopeNote>
    <skos:definition>A single preferred name of a company or identifier system (preferably English).</skos:definition>
    <rdfs:label>preferred name</rdfs:label>
    <schema:rangeIncludes rdf:resource="http://www.w3.org/2001/XMLSchema#string"/>
    <schema:rangeIncludes rdf:resource="http://www.w3.org/1999/02/22-rdf-syntax-ns#langString"/>
    <schema:domainIncludes rdf:resource="http://www.w3.org/ns/regorg#RegisteredOrganization"/>
    <schema:domainIncludes rdf:resource="http://data.businessgraph.io/ontology#IdentifierSystem"/>
    <rdf:type rdf:resource="http://www.w3.org/2002/07/owl#DatatypeProperty"/>
  </rdf:Description>
  <rdf:Description rdf:about="http://data.businessgraph.io/ontology#adminUnitL5">
    <ebg:order rdf:datatype="http://www.w3.org/2001/XMLSchema#integer">33</ebg:order>
    <skos:definition>LAU1 (Municipality/Commune/Settlement) of the address.</skos:definition>
    <rdfs:label>admin unit level 5</rdfs:label>
    <skos:scopeNote>Some countries (e.g. Bulgaria) use both LAU1 and LAU2 levels. Others (e.g. Italy) use only LAU2.</skos:scopeNote>
    <rdfs:isDefinedBy rdf:resource="http://data.businessgraph.io/ontology#"/>
    <schema:rangeIncludes rdf:resource="http://data.businessgraph.io/ontology#LAURegion"/>
    <schema:domainIncludes rdf:resource="http://www.w3.org/ns/locn#Address"/>
    <rdf:type rdf:resource="http://www.w3.org/2002/07/owl#ObjectProperty"/>
  </rdf:Description>
  <rdf:Description rdf:about="http://schema.org/availableLanguage">
    <schema:domainIncludes rdf:resource="http://www.w3.org/ns/regorg#RegisteredOrganization"/>
    <rdfs:label>language</rdfs:label>
    <skos:example>en</skos:example>
    <skos:scopeNote>Deduced from languages appearing in web resources related to the organisation (e.g. corporate websites, social network accounts, etc.).</skos:scopeNote>
    <schema:rangeIncludes rdf:resource="http://www.w3.org/2001/XMLSchema#string"/>
    <skos:example>it</skos:example>
    <skos:scopeNote>The value should be from the [iana:] list: ISO 639-1 codes, optionally followed by region of use.</skos:scopeNote>
    <skos:example>zh-CN</skos:example>
    <skos:scopeNote>Currently this data is provided by SDATI, for matching company entities only.</skos:scopeNote>
    <skos:definition>Languages used by the organization.</skos:definition>
    <ebg:order rdf:datatype="http://www.w3.org/2001/XMLSchema#integer">17</ebg:order>
    <rdf:type rdf:resource="http://www.w3.org/2002/07/owl#DatatypeProperty"/>
  </rdf:Description>
  <rdf:Description rdf:about="http://www.w3.org/ns/locn#adminUnitL1">
    <ebg:order rdf:datatype="http://www.w3.org/2001/XMLSchema#integer">29</ebg:order>
    <skos:example>nuts:IT (Italy).</skos:example>
    <skos:definition>Country of the address</skos:definition>
    <rdfs:label>admin unit level 1</rdfs:label>
    <schema:rangeIncludes rdf:resource="http://rdfdata.eionet.europa.eu/ramon/ontology/NUTSRegion"/>
    <schema:domainIncludes rdf:resource="http://www.w3.org/ns/locn#Address"/>
    <rdf:type rdf:resource="http://www.w3.org/2002/07/owl#ObjectProperty"/>
  </rdf:Description>
  <rdf:Description rdf:about="http://data.businessgraph.io/ontology#validationRegex">
    <rdfs:isDefinedBy rdf:resource="http://data.businessgraph.io/ontology#"/>
    <skos:example>"\d{9}" is a simple regex for validating DUNS numbers</skos:example>
    <rdf:type rdf:resource="http://www.w3.org/2002/07/owl#DatatypeProperty"/>
    <skos:definition>Regular expression for validating identifier values within the system</skos:definition>
    <skos:example>"([A-Z]{2})/(\d+)" is a regex for the EU Value Added Tax (VIES) register, which consists of a member state code followed by slash and a national numeric identifier</skos:example>
    <skos:example>"(\d{2})-?(\d{3})-?(\d{4})" is a regex for validating DUNS numbers that may include optional dashes in the indicated positions (e.g. "36-032-1459")</skos:example>
    <schema:rangeIncludes rdf:resource="http://www.w3.org/2001/XMLSchema#string"/>
    <schema:domainIncludes rdf:resource="http://data.businessgraph.io/ontology#IdentifierSystem"/>
    <rdfs:label>validation regex</rdfs:label>
    <ebg:order rdf:datatype="http://www.w3.org/2001/XMLSchema#integer">61</ebg:order>
  </rdf:Description>
  <rdf:Description rdf:about="http://www.w3.org/ns/org#Site">
    <skos:scopeNote>EBG doesn't need the distinction between org:Site and locn:Address, so we use one node having both types, and a self link org:siteAddress</skos:scopeNote>
    <skos:definition xml:lang="en">An office or other premise at which the organization is located.&#xD;
Many organizations are spread across multiple sites and many sites will host multiple locations.&#xD;
In most cases a Site will be a physical location. However, we don't exclude the possibility of non-physical sites such as a virtual office with an associated post box and phone reception service [org:]</skos:definition>
    <rdfs:label>Site</rdfs:label>
    <rdf:type rdf:resource="http://www.w3.org/2000/01/rdf-schema#Class"/>
  </rdf:Description>
  <rdf:Description rdf:about="http://www.w3.org/2004/02/skos/core#ConceptScheme">
    <rdfs:label>Concept Scheme</rdfs:label>
    <rdf:type rdf:resource="http://www.w3.org/2000/01/rdf-schema#Class"/>
  </rdf:Description>
  <rdf:Description rdf:about="http://www.w3.org/ns/org#Membership">
    <skos:scopeNote>it is acceptable to use the same Membership node for several officers, if they had exactly the same role and membership interval (e.g. in many countries the Board is appointed and discharged at the same interval, namely between AGMs of the company)</skos:scopeNote>
    <skos:definition>represents the relation between an organisation and a member of that organisation.</skos:definition>
    <rdfs:label>Membership</rdfs:label>
    <rdf:type rdf:resource="http://www.w3.org/2000/01/rdf-schema#Class"/>
  </rdf:Description>
  <rdf:Description rdf:about="http://purl.org/dc/elements/1.1/format">
    <skos:example>For a Description document supporting the OpenSearch standard, use &lt;http://a9.com/-/spec/opensearch/1.1/&gt;</skos:example>
    <schema:domainIncludes rdf:resource="http://data.businessgraph.io/ontology#IdentifierWebResource"/>
    <schema:rangeIncludes rdf:resource="http://www.w3.org/2001/XMLSchema#string"/>
    <ebg:order rdf:datatype="http://www.w3.org/2001/XMLSchema#integer">67</ebg:order>
    <skos:definition>MIME type of the resource. If several are provided, the server must provide all these resource types using Content Negotiation</skos:definition>
    <rdfs:label>MIME Type</rdfs:label>
    <skos:example>For a search page, use the custom type "application/x-search"</skos:example>
    <skos:example>application/rdf+xml</skos:example>
    <skos:example>application/xml</skos:example>
    <skos:example>text/turtle</skos:example>
    <skos:example>text/tab-separated-values</skos:example>
    <schema:rangeIncludes rdf:resource="http://www.w3.org/1999/02/22-rdf-syntax-ns#Resource"/>
    <skos:example>text/html</skos:example>
    <rdf:type rdf:resource="http://www.w3.org/2002/07/owl#DatatypeProperty"/>
    <schema:domainIncludes rdf:resource="http://data.businessgraph.io/ontology#WebResource"/>
    <skos:example>text/csv</skos:example>
  </rdf:Description>
  <rdf:Description rdf:about="http://www.w3.org/ns/adms#identifier">
    <skos:example>Indirect: BG GUID 617f4edf8c154f4296efdf146513de21, which corresponds to official id 204060254 and can be used to reach the official register page for that company</skos:example>
    <skos:example>Multiple: bank license, insurance license, license to trade dual-use goods (arms), Twitter account, Facebook account.</skos:example>
    <skos:example>Direct: EU VAT number (in those jurisdictions where it is used as the primary company identifier), BRIS id, OCORP id.</skos:example>
    <skos:example>Indirect: GLEI LEI, SDATI Atoka ID.</skos:example>
    <rdfs:label>identifier</rdfs:label>
    <schema:domainIncludes rdf:resource="http://www.w3.org/ns/regorg#RegisteredOrganization"/>
    <skos:scopeNote>For Identifier Systems, we use codes issued by euBusinessGraph.&#xD;
For official Identifier Systems (country registers), we use the jurisdiction code (e.g. 'BG', 'GB').&#xD;
For other identifier systems, we use a short mnemonic code:&#xD;
- upper-case for company registers (e.g. 'OCORP', 'SDATI', 'RAL', 'EU', 'BRIS'),&#xD;
- mixed-case for social network registers (eg 'Twitter', 'Facebook').&#xD;
This code is used as the last URL part for identifiers issued in that system.</skos:scopeNote>
    <ebg:order rdf:datatype="http://www.w3.org/2001/XMLSchema#integer">26</ebg:order>
    <skos:definition>An identifier of a Company (the official identifier is rov:registration) or Identifier System / Register</skos:definition>
    <rdf:type rdf:resource="http://www.w3.org/2002/07/owl#ObjectProperty"/>
    <schema:rangeIncludes rdf:resource="http://www.w3.org/ns/adms#Identifier"/>
    <schema:domainIncludes rdf:resource="http://data.businessgraph.io/ontology#IdentifierSystem"/>
    <skos:scopeNote>This includes, but is not limited to:&#xD;
- Direct: Identifier in some aggregated dataset, where the official ID is part of the aggregation ID.&#xD;
- Indirect: Identifier in some aggregated dataset or for a website, where the aggregation ID bears no resemblance to the official ID&#xD;
- Multiple: Identifier that has a many-to-many relation with the company, i.e., a company may have several identifiers of the same kind, and the same identifier can be used by several companies.</skos:scopeNote>
  </rdf:Description>
  <rdf:Description rdf:about="http://schema.org/sameAs">
    <ebg:order rdf:datatype="http://www.w3.org/2001/XMLSchema#integer">19</ebg:order>
    <skos:example rdf:resource="https://it.wikipedia.org/wiki/Trento"/>
    <skos:definition>Wikipedia page pertaining to the company.</skos:definition>
    <rdfs:label>wikipedia page</rdfs:label>
    <schema:rangeIncludes rdf:resource="http://www.w3.org/1999/02/22-rdf-syntax-ns#Resource"/>
    <schema:domainIncludes rdf:resource="http://www.w3.org/ns/regorg#RegisteredOrganization"/>
    <rdf:type rdf:resource="http://www.w3.org/2002/07/owl#ObjectProperty"/>
  </rdf:Description>
  <rdf:Description rdf:about="http://www.w3.org/2001/XMLSchema#gYearMonth">
    <rdfs:label>Year-Month</rdfs:label>
    <rdf:type rdf:resource="http://www.w3.org/2000/01/rdf-schema#Datatype"/>
  </rdf:Description>
  <rdf:Description rdf:about="http://data.businessgraph.io/ontology#order">
    <ebg:order rdf:datatype="http://www.w3.org/2001/XMLSchema#integer">110</ebg:order>
    <schema:rangeIncludes rdf:resource="http://www.w3.org/2001/XMLSchema#integer"/>
    <schema:domainIncludes rdf:resource="http://www.w3.org/2004/02/skos/core#Concept"/>
    <rdfs:comment>Global order of a thesaurus concept respecting the hierarchical structure (depth-first traversal)</rdfs:comment>
    <rdfs:label>order</rdfs:label>
    <rdfs:isDefinedBy rdf:resource="http://data.businessgraph.io/ontology#"/>
    <rdf:type rdf:resource="http://www.w3.org/2002/07/owl#DatatypeProperty"/>
  </rdf:Description>
  <rdf:Description rdf:about="http://data.businessgraph.io/ontology#isUnique">
    <skos:example>Person names are not unique since they are highly ambiguous</skos:example>
    <skos:definition>Whether each identifier in the system relates to only one entity</skos:definition>
    <rdf:type rdf:resource="http://www.w3.org/2002/07/owl#DatatypeProperty"/>
    <schema:domainIncludes rdf:resource="http://data.businessgraph.io/ontology#IdentifierSystem"/>
    <rdfs:isDefinedBy rdf:resource="http://data.businessgraph.io/ontology#"/>
    <skos:example>Stock exchange tickers are unique to each exchange (but a company can buy the ticker of another, i.e. the identity may change over time)</skos:example>
    <skos:scopeNote>Similar to: owl:InverseFunctionalProperty, and Wikidata Distinct Values constraint</skos:scopeNote>
    <ebg:order rdf:datatype="http://www.w3.org/2001/XMLSchema#integer">52</ebg:order>
    <skos:example>Company IDs are unique in most national registers: one ID cannot identify two companies</skos:example>
    <skos:example>Websites are not unique since a website can be shared by several related companies</skos:example>
    <rdfs:label>has unique identifiers</rdfs:label>
    <schema:rangeIncludes rdf:resource="http://www.w3.org/2001/XMLSchema#boolean"/>
  </rdf:Description>
  <rdf:Description rdf:about="http://www.w3.org/2004/02/skos/core#Concept">
    <rdfs:label>Concept</rdfs:label>
    <rdf:type rdf:resource="http://www.w3.org/2000/01/rdf-schema#Class"/>
  </rdf:Description>
  <rdf:Description rdf:about="http://schema.org/email">
    <ebg:order rdf:datatype="http://www.w3.org/2001/XMLSchema#integer">20</ebg:order>
    <skos:example rdf:resource="mailto:elettorale@pec.comune.trento.it"/>
    <skos:defintion>Email that is officially registered and with the same validity as certified (snail) mail.</skos:defintion>
    <rdfs:label>certified email address</rdfs:label>
    <skos:scopeNote>The value should be a mailto: URL.</skos:scopeNote>
    <skos:scopeNote>euBusinessGraph does not record other company emails, so there is no need to distinguish between different kinds</skos:scopeNote>
    <schema:rangeIncludes rdf:resource="http://www.w3.org/1999/02/22-rdf-syntax-ns#Resource"/>
    <schema:domainIncludes rdf:resource="http://www.w3.org/ns/regorg#RegisteredOrganization"/>
    <rdf:type rdf:resource="http://www.w3.org/2002/07/owl#ObjectProperty"/>
  </rdf:Description>
  <rdf:Description rdf:about="http://www.w3.org/ns/org#organization">
    <ebg:order rdf:datatype="http://www.w3.org/2001/XMLSchema#integer">103</ebg:order>
    <skos:definition>Points to the company the membership is about</skos:definition>
    <rdfs:label>company</rdfs:label>
    <schema:rangeIncludes rdf:resource="http://www.w3.org/ns/org#Organization"/>
    <schema:domainIncludes rdf:resource="http://www.w3.org/ns/org#Membership"/>
    <rdf:type rdf:resource="http://www.w3.org/2002/07/owl#ObjectProperty"/>
  </rdf:Description>
  <rdf:Description rdf:about="http://schema.org/foundingDate">
    <skos:example rdf:datatype="http://www.w3.org/2001/XMLSchema#date">2010-11-18</skos:example>
    <schema:rangeIncludes rdf:resource="http://www.w3.org/2001/XMLSchema#gYearMonth"/>
    <skos:scopeNote>Should have a valid XSD datatype.</skos:scopeNote>
    <skos:example rdf:datatype="http://www.w3.org/2001/XMLSchema#gYearMonth">2010-11</skos:example>
    <rdf:type rdf:resource="http://www.w3.org/2002/07/owl#DatatypeProperty"/>
    <schema:rangeIncludes rdf:resource="http://www.w3.org/2001/XMLSchema#gYear"/>
    <schema:domainIncludes rdf:resource="http://www.w3.org/ns/regorg#RegisteredOrganization"/>
    <ebg:order rdf:datatype="http://www.w3.org/2001/XMLSchema#integer">13</ebg:order>
    <schema:rangeIncludes rdf:resource="http://www.w3.org/2001/XMLSchema#date"/>
    <skos:definition>Date when the organization was created.</skos:definition>
    <rdfs:label>founding date</rdfs:label>
    <skos:example rdf:datatype="http://www.w3.org/2001/XMLSchema#gYear">2010</skos:example>
  </rdf:Description>
  <rdf:Description rdf:about="http://data.businessgraph.io/ontology#replacementPattern">
    <ebg:order rdf:datatype="http://www.w3.org/2001/XMLSchema#integer">62</ebg:order>
    <skos:example>"$1$2$3" can be used together with the validationRegex "(\d{2})-?(\d{3})-?(\d{4})" to extract the pure digits from a DUNS number spelled with optional dashes (e.g. "36-032-1459" -&gt; "360321459")</skos:example>
    <skos:definition>Pattern to use together with the Validation Regex to normalise identifier values by removing optional decorations</skos:definition>
    <schema:rangeIncludes rdf:resource="http://www.w3.org/2001/XMLSchema#string"/>
    <schema:domainIncludes rdf:resource="http://data.businessgraph.io/ontology#IdentifierSystem"/>
    <rdfs:label>replacement pattern</rdfs:label>
    <rdfs:isDefinedBy rdf:resource="http://data.businessgraph.io/ontology#"/>
    <rdf:type rdf:resource="http://www.w3.org/2002/07/owl#DatatypeProperty"/>
  </rdf:Description>
  <rdf:Description rdf:about="http://rdfs.org/sioc/ns#feed">
    <ebg:order rdf:datatype="http://www.w3.org/2001/XMLSchema#integer">21</ebg:order>
    <skos:example rdf:resource="http://www.comune.ancona.gov.it/ankonline/anconaentrate/feed/"/>
    <skos:definition>RSS/Atom feed pertaining to the company.</skos:definition>
    <rdfs:label>news/blog feed</rdfs:label>
    <schema:rangeIncludes rdf:resource="http://www.w3.org/1999/02/22-rdf-syntax-ns#Resource"/>
    <schema:domainIncludes rdf:resource="http://www.w3.org/ns/regorg#RegisteredOrganization"/>
    <rdf:type rdf:resource="http://www.w3.org/2002/07/owl#ObjectProperty"/>
  </rdf:Description>
  <rdf:Description rdf:about="http://schema.org/latitude">
    <ebg:order rdf:datatype="http://www.w3.org/2001/XMLSchema#integer">42</ebg:order>
    <skos:scopeNote>If no coordinates are available, do not make a schema:GeoCoordinates node.</skos:scopeNote>
    <skos:scopeNote>Coordinates must be expressed in the WGS 84 system.</skos:scopeNote>
    <rdfs:label>latitude</rdfs:label>
    <schema:rangeIncludes rdf:resource="http://www.w3.org/2001/XMLSchema#decimal"/>
    <schema:domainIncludes rdf:resource="http://schema.org/GeoCoordinates"/>
    <rdf:type rdf:resource="http://www.w3.org/2002/07/owl#DatatypeProperty"/>
  </rdf:Description>
  <rdf:Description rdf:about="http://data.businessgraph.io/dataset/paid-advertised">
    <skos:prefLabel>Paid (advertised only)</skos:prefLabel>
    <skos:inScheme rdf:resource="http://data.businessgraph.io/dataset/"/>
    <rdfs:isDefinedBy rdf:resource="http://data.businessgraph.io/ontology#"/>
    <rdf:type rdf:resource="http://www.w3.org/2004/02/skos/core#Concept"/>
  </rdf:Description>
  <rdf:Description rdf:about="http://data.businessgraph.io/ontology#orgActivityText">
    <skos:example>NACE = 72.19 Scientific research and development in the field of natural, medical, agricultural and technical sciences, without biotechnology</skos:example>
    <skos:example>Free text = Development, exploration and production of opto-electronic systems for analogue and digital holographic recording, interferometric measurement of mechanical characteristics and biological objects at micro and macro level, refractometers, light-sensitive materials for holographic recording, blueprints of museum exhibits, artworks and collection surveys, production of holographic illustrations for students, albums, advertising, souvenirs and others, design and manufacture of holographic optical elements with a wide spectrum of applications, marketing and sale of holographic products, consulting, training and promotion of holographic methods and technologies, mediation, brokerage, and **any other activity not prohibited** by Bulgarian legislation.</skos:example>
    <skos:definition>Economic activity of the organization (free text)</skos:definition>
    <rdf:type rdf:resource="http://www.w3.org/2002/07/owl#DatatypeProperty"/>
    <rdfs:isDefinedBy rdf:resource="http://data.businessgraph.io/ontology#"/>
    <schema:rangeIncludes rdf:resource="http://www.w3.org/1999/02/22-rdf-syntax-ns#langString"/>
    <schema:domainIncludes rdf:resource="http://www.w3.org/ns/regorg#RegisteredOrganization"/>
    <skos:scopeNote>Such field is widely used in some countries (e.g. BG) and may include much richer info than rov:orgActivity</skos:scopeNote>
    <ebg:order rdf:datatype="http://www.w3.org/2001/XMLSchema#integer">11</ebg:order>
    <rdfs:label>economic activity text</rdfs:label>
  </rdf:Description>
  <rdf:Description rdf:about="http://www.w3.org/2001/XMLSchema#gYear">
    <rdfs:label>Year</rdfs:label>
    <rdf:type rdf:resource="http://www.w3.org/2000/01/rdf-schema#Datatype"/>
  </rdf:Description>
  <rdf:Description rdf:about="http://www.w3.org/ns/regorg#registration">
    <ebg:order rdf:datatype="http://www.w3.org/2001/XMLSchema#integer">25</ebg:order>
    <skos:scopeNote>In some cases we may not have info about the official registration, though "it is questionable whether a description of a registered organization without this property and an associated Identifier class will be of any value" [rov:]</skos:scopeNote>
    <skos:scopeNote>This is a sub-property of adms:identifier, and should be an adms:Identifier pointing to an official ebg:IdentifierSystem. So it holds redundant information, but this is done for compatibility with the Registered Organization vocabulary.</skos:scopeNote>
    <skos:definition>Identifier that holds the official company registration in its jurisdiction of registration. It establishes the legal existence of the company.</skos:definition>
    <rdfs:label>official registration</rdfs:label>
    <schema:rangeIncludes rdf:resource="http://www.w3.org/ns/adms#Identifier"/>
    <schema:domainIncludes rdf:resource="http://www.w3.org/ns/regorg#RegisteredOrganization"/>
    <rdf:type rdf:resource="http://www.w3.org/2002/07/owl#ObjectProperty"/>
  </rdf:Description>
  <rdf:Description rdf:about="http://www.w3.org/ns/locn#locatorDesignator">
    <ebg:order rdf:datatype="http://www.w3.org/2001/XMLSchema#integer">38</ebg:order>
    <skos:example>Polygraphia Office Center, floor 4</skos:example>
    <skos:example>47A</skos:example>
    <skos:definition>Street number and/or building name.</skos:definition>
    <rdfs:label>locator designator (street number)</rdfs:label>
    <skos:scopeNote>Not likely to appear separately, but we have Coordinate resolution corresponding to this field.</skos:scopeNote>
    <schema:rangeIncludes rdf:resource="http://www.w3.org/2001/XMLSchema#string"/>
    <schema:domainIncludes rdf:resource="http://www.w3.org/ns/locn#Address"/>
    <rdf:type rdf:resource="http://www.w3.org/2002/07/owl#DatatypeProperty"/>
  </rdf:Description>
  <rdf:Description rdf:about="http://purl.org/dc/terms/issued">
    <ebg:order rdf:datatype="http://www.w3.org/2001/XMLSchema#integer">73</ebg:order>
    <skos:scopeNote>This may or may not be the same as the Incorporation Date of the company. Even for the official registration, the two dates may differ, depending on business rules.</skos:scopeNote>
    <skos:definition>When was the identifier was issued (start date).</skos:definition>
    <rdfs:label>issued on</rdfs:label>
    <schema:rangeIncludes rdf:resource="http://www.w3.org/2001/XMLSchema#date"/>
    <schema:domainIncludes rdf:resource="http://www.w3.org/ns/adms#Identifier"/>
    <rdf:type rdf:resource="http://www.w3.org/2002/07/owl#DatatypeProperty"/>
  </rdf:Description>
  <rdf:Description rdf:about="http://rdfdata.eionet.europa.eu/ramon/ontology/name">
    <ebg:order rdf:datatype="http://www.w3.org/2001/XMLSchema#integer">113</ebg:order>
    <schema:rangeIncludes rdf:resource="http://www.w3.org/1999/02/22-rdf-syntax-ns#langString"/>
    <schema:domainIncludes rdf:resource="http://data.businessgraph.io/ontology#LAURegion"/>
    <schema:domainIncludes rdf:resource="http://rdfdata.eionet.europa.eu/ramon/ontology/NUTSRegion"/>
    <rdfs:comment>Name of an administrative region or settlement</rdfs:comment>
    <rdfs:label>admin region name</rdfs:label>
    <rdf:type rdf:resource="http://www.w3.org/2002/07/owl#DatatypeProperty"/>
  </rdf:Description>
  <rdf:Description rdf:about="http://www.w3.org/ns/locn#poBox">
    <ebg:order rdf:datatype="http://www.w3.org/2001/XMLSchema#integer">40</ebg:order>
    <skos:definition>Some addresses are associated with a PO box instead of a street address.</skos:definition>
    <rdfs:label>post office box</rdfs:label>
    <schema:rangeIncludes rdf:resource="http://www.w3.org/2001/XMLSchema#string"/>
    <schema:domainIncludes rdf:resource="http://www.w3.org/ns/locn#Address"/>
    <rdf:type rdf:resource="http://www.w3.org/2002/07/owl#DatatypeProperty"/>
  </rdf:Description>
  <rdf:Description rdf:about="http://data.businessgraph.io/ontology#orgActivityTransitive">
    <ebg:order rdf:datatype="http://www.w3.org/2001/XMLSchema#integer">12</ebg:order>
    <skos:scopeNote>Transive closure of rov:orgActivity along the skos:broader hierarchy</skos:scopeNote>
    <skos:definition>Economic activity of the organization (all hierarchical NACE codes)</skos:definition>
    <rdfs:label>economic activity transitive</rdfs:label>
    <schema:rangeIncludes rdf:resource="http://www.w3.org/2004/02/skos/core#Concept"/>
    <schema:domainIncludes rdf:resource="http://www.w3.org/ns/regorg#RegisteredOrganization"/>
    <rdf:type rdf:resource="http://www.w3.org/2002/07/owl#ObjectProperty"/>
  </rdf:Description>
  <rdf:Description rdf:about="http://www.w3.org/ns/locn#fullAddress">
    <ebg:order rdf:datatype="http://www.w3.org/2001/XMLSchema#integer">28</ebg:order>
    <skos:example>Via Belenzani 19, 38122, Trento</skos:example>
    <skos:example>Aston House, Cornwall Avenue, London N3 1LF, UK</skos:example>
    <skos:definition>Full address, free text.</skos:definition>
    <rdfs:label>full address</rdfs:label>
    <schema:rangeIncludes rdf:resource="http://www.w3.org/1999/02/22-rdf-syntax-ns#langString"/>
    <schema:rangeIncludes rdf:resource="http://www.w3.org/2001/XMLSchema#string"/>
    <schema:domainIncludes rdf:resource="http://www.w3.org/ns/locn#Address"/>
    <rdf:type rdf:resource="http://www.w3.org/2002/07/owl#DatatypeProperty"/>
  </rdf:Description>
  <rdf:Description rdf:about="http://data.businessgraph.io/ontology#geoResolution">
    <ebg:order rdf:datatype="http://www.w3.org/2001/XMLSchema#integer">44</ebg:order>
    <skos:scopeNote>Values must be mapped to the &lt;resolution/&gt; ConceptScheme (lookup list).</skos:scopeNote>
    <skos:scopeNote>If geo coordinates are present, resolution must be present too, even if it's a guess. There is no default value.</skos:scopeNote>
    <skos:definition>Resolution of a geographic coordinate location: from &lt;resolution/L0&gt; continent (least precise) to &lt;resolution/L10&gt; individual house number (most precise).</skos:definition>
    <rdfs:isDefinedBy rdf:resource="http://data.businessgraph.io/ontology#"/>
    <rdfs:label>geocoordinate resolution</rdfs:label>
    <schema:domainIncludes rdf:resource="http://schema.org/GeoCoordinates"/>
    <rdf:type rdf:resource="http://www.w3.org/2002/07/owl#ObjectProperty"/>
  </rdf:Description>
  <rdf:Description rdf:about="http://data.businessgraph.io/ontology#adminUnit">
    <ebg:order rdf:datatype="http://www.w3.org/2001/XMLSchema#integer">107</ebg:order>
    <skos:scopeNote>The lowest-level property of locn:adminUnitL1..2 and ebg:adminUnitL3..6. Used for faceting by place.</skos:scopeNote>
    <skos:definition>Most specific administrative unit related to an address.</skos:definition>
    <schema:rangeIncludes rdf:resource="http://data.businessgraph.io/ontology#LAURegion"/>
    <schema:rangeIncludes rdf:resource="http://rdfdata.eionet.europa.eu/ramon/ontology/NUTSRegion"/>
    <schema:domainIncludes rdf:resource="http://www.w3.org/ns/locn#Address"/>
    <rdfs:label>admin unit</rdfs:label>
    <rdfs:isDefinedBy rdf:resource="http://data.businessgraph.io/ontology#"/>
    <rdf:type rdf:resource="http://www.w3.org/2002/07/owl#ObjectProperty"/>
  </rdf:Description>
  <rdf:Description rdf:about="http://rdfdata.eionet.europa.eu/ramon/ontology/level">
    <ebg:order rdf:datatype="http://www.w3.org/2001/XMLSchema#integer">112</ebg:order>
    <schema:rangeIncludes rdf:resource="http://www.w3.org/2001/XMLSchema#integer"/>
    <schema:domainIncludes rdf:resource="http://data.businessgraph.io/ontology#LAURegion"/>
    <schema:domainIncludes rdf:resource="http://rdfdata.eionet.europa.eu/ramon/ontology/NUTSRegion"/>
    <rdfs:comment>Level of an administrative region: NUTS1..3=1..3, LAU1..2=4..5</rdfs:comment>
    <rdfs:label>admin region level</rdfs:label>
    <rdf:type rdf:resource="http://www.w3.org/2002/07/owl#DatatypeProperty"/>
  </rdf:Description>
  <rdf:Description rdf:about="http://www.w3.org/ns/regorg#orgType">
    <ebg:order rdf:datatype="http://www.w3.org/2001/XMLSchema#integer">3</ebg:order>
    <skos:scopeNote>In addition or alternatively to this field, ebg:orgTypeText may be used.</skos:scopeNote>
    <skos:scopeNote>The types may form a hierarchy, but each company can have maximum one value. E.g. for Italy: Società Di Capitale &gt; Società a responsabilità limitata [ebg:]</skos:scopeNote>
    <skos:scopeNote>There is no agreed set of company types that crosses borders [rov:]. Each jurisdiction will have a limited set of recognized company types and these should be expressed in a consistent manner in a SKOS Concept Scheme [rov:]. Code lists of euBusinessGraph data providers were collected and published in the project repository.</skos:scopeNote>
    <skos:definition>Company Type (Legal Form of the entity)</skos:definition>
    <rdfs:label>type</rdfs:label>
    <schema:domainIncludes rdf:resource="http://www.w3.org/ns/regorg#RegisteredOrganization"/>
    <rdf:type rdf:resource="http://www.w3.org/2002/07/owl#ObjectProperty"/>
  </rdf:Description>
  <rdf:Description rdf:about="http://www.w3.org/ns/person#birthName">
    <ebg:order rdf:datatype="http://www.w3.org/2001/XMLSchema#integer">102</ebg:order>
    <skos:example>Michele Barbera</skos:example>
    <skos:definition>The legal name of the person which is usually determined at or around birth, usually persistent and for this reason usually recorded by some official registers. Although birth names tend to be persistent we do not assume this has to be the case.</skos:definition>
    <rdfs:label>birth name</rdfs:label>
    <schema:rangeIncludes rdf:resource="http://www.w3.org/2001/XMLSchema#string"/>
    <schema:domainIncludes rdf:resource="http://www.w3.org/ns/person#Person"/>
    <rdf:type rdf:resource="http://www.w3.org/2002/07/owl#DatatypeProperty"/>
  </rdf:Description>
  <rdf:Description rdf:about="http://www.w3.org/ns/org#memberDuring">
    <ebg:order rdf:datatype="http://www.w3.org/2001/XMLSchema#integer">105</ebg:order>
    <skos:scopeNote>for the common case of missing time, we prefer to use xsd:date rather than completing it with a fake null time, eg "&lt;date&gt;T00:00:00Z"^^xsd:dateTime.</skos:scopeNote>
    <skos:definition>Interval (beginning and end) of the membership relation. May be an open interval.</skos:definition>
    <schema:rangeIncludes rdf:resource="http://www.w3.org/2006/time#Interval"/>
    <schema:domainIncludes rdf:resource="http://www.w3.org/ns/org#Membership"/>
    <rdfs:label>duration</rdfs:label>
    <rdf:type rdf:resource="http://www.w3.org/2002/07/owl#ObjectProperty"/>
  </rdf:Description>
  <rdf:Description rdf:about="http://data.businessgraph.io/dataset/">
    <dct:publisher rdf:resource="http://businessgraph.io"/>
    <dct:creator rdf:resource="http://businessgraph.io"/>
    <rdfs:comment>Company dataset type: freely avaialable, paid (advertised only), partition</rdfs:comment>
    <rdfs:label>Dataset type</rdfs:label>
    <rdfs:isDefinedBy rdf:resource="http://data.businessgraph.io/ontology#"/>
    <rdf:type rdf:resource="http://www.w3.org/2004/02/skos/core#ConceptScheme"/>
  </rdf:Description>
  <rdf:Description rdf:about="http://data.businessgraph.io/ontology#IdentifierSystem">
    <skos:example>http://www.registryagency.bg keeps the systems used by The Trade Register http://brra.bg for companies, and The Bulstat Register http://www.bulstat.bg/ for other entities</skos:example>
    <skos:scopeNote>Some agencies/registers keep several identifier systems; this ontology doesn't distinguish between an identifier system and its register(s)</skos:scopeNote>
    <skos:definition>A system managed by a publisher (e.g., a register or agency) that is used to issue identifiers to entities (companies, persons, etc).</skos:definition>
    <rdfs:label>Identifier System</rdfs:label>
    <rdfs:isDefinedBy rdf:resource="http://data.businessgraph.io/ontology#"/>
    <rdf:type rdf:resource="http://www.w3.org/2000/01/rdf-schema#Class"/>
  </rdf:Description>
  <rdf:Description rdf:about="http://data.businessgraph.io/ontology#orgTypeText">
    <schema:domainIncludes rdf:resource="http://www.w3.org/ns/regorg#RegisteredOrganization"/>
    <rdf:type rdf:resource="http://www.w3.org/2002/07/owl#DatatypeProperty"/>
    <rdfs:label>type text</rdfs:label>
    <schema:rangeIncludes rdf:resource="http://www.w3.org/1999/02/22-rdf-syntax-ns#langString"/>
    <skos:scopeNote>Include valid language tag (see [iana:] for list).</skos:scopeNote>
    <rdfs:isDefinedBy rdf:resource="http://data.businessgraph.io/ontology#"/>
    <skos:example xml:lang="en">Private Limited Company</skos:example>
    <skos:scopeNote>Because of the difficulties of standardizing Type lookup, we include a free text field</skos:scopeNote>
    <skos:example xml:lang="it">Società a responsabilità limitata</skos:example>
    <ebg:order rdf:datatype="http://www.w3.org/2001/XMLSchema#integer">4</ebg:order>
    <skos:scopeNote>If Type is also present, it must express the same value as Type Text.</skos:scopeNote>
    <skos:example xml:lang="bg">Дружество с ограничена отговорност</skos:example>
    <skos:definition>Company Type (Entity Legal Form) as reported by a national company registe (free text).</skos:definition>
  </rdf:Description>
  <rdf:Description rdf:about="http://www.w3.org/2004/02/skos/core#notation">
    <skos:scopeNote>Should not include leading, trailing and consecutive spaces, to facilitate exact match.</skos:scopeNote>
    <skos:scopeNote>Codes for Identifier Systems are issued locally by euBusinessGraph.&#xD;
For identifier systems published by the sole or preferred official register in a jurisdiction, we use the jurisdiction code (e.g. "BG", "GB"). &#xD;
For others, if the identifier system has no explicit name, we use a short mnemonic code of the publisher:&#xD;
- upper-case for company registers (e.g. "OCORP", "SDATI", "RAL", "EU", "BRIS"),&#xD;
- mixed-case for social network registers (e.g. "Twitter", "Facebook").</skos:scopeNote>
    <rdf:type rdf:resource="http://www.w3.org/2002/07/owl#DatatypeProperty"/>
    <skos:definition>Literal value of the identifier.</skos:definition>
    <skos:scopeNote>adms:Identifier recommends that this value should be "datatyped with the identifier scheme (including the version number if appropriate)". However, we decided not to do this because:&#xD;
- One cannot search by exact literal value unless one also knows the datatype URL&#xD;
- Currently we do not plan to maintain different identifier system versions</skos:scopeNote>
    <rdfs:label>notation (identifier value)</rdfs:label>
    <schema:domainIncludes rdf:resource="http://data.businessgraph.io/ontology#IdentifierSystem"/>
    <schema:domainIncludes rdf:resource="http://www.w3.org/ns/adms#Identifier"/>
    <schema:rangeIncludes rdf:resource="http://www.w3.org/2001/XMLSchema#string"/>
    <ebg:order rdf:datatype="http://www.w3.org/2001/XMLSchema#integer">49</ebg:order>
  </rdf:Description>
  <rdf:Description rdf:about="http://schema.org/license">
    <ebg:order rdf:datatype="http://www.w3.org/2001/XMLSchema#integer">51</ebg:order>
    <skos:scopeNote>If possible, use established license URLs, e.g. from https://creativecommons.org/ or http://rightsstatements.org/</skos:scopeNote>
    <skos:definition>License that applies to an identifier system or dataset</skos:definition>
    <schema:rangeIncludes rdf:resource="http://www.w3.org/1999/02/22-rdf-syntax-ns#Resource"/>
    <schema:domainIncludes rdf:resource="http://rdfs.org/ns/void#Dataset"/>
    <schema:domainIncludes rdf:resource="http://data.businessgraph.io/ontology#IdentifierSystem"/>
    <rdfs:label>license</rdfs:label>
    <rdf:type rdf:resource="http://www.w3.org/2002/07/owl#ObjectProperty"/>
  </rdf:Description>
  <rdf:Description rdf:about="http://www.w3.org/ns/locn#thoroughfare">
    <ebg:order rdf:datatype="http://www.w3.org/2001/XMLSchema#integer">37</ebg:order>
    <schema:domainIncludes rdf:resource="http://www.w3.org/ns/locn#Address"/>
    <schema:rangeIncludes rdf:resource="http://www.w3.org/2001/XMLSchema#string"/>
    <rdf:type rdf:resource="http://www.w3.org/2002/07/owl#DatatypeProperty"/>
    <skos:example>Polygraphia Office Center, floor 4
47A Tsarigradsko Shosse</skos:example>
    <skos:definition>Street name and optionally number.</skos:definition>
    <skos:scopeNote>It is ok if the street number is also here, because many systems do not enter the number separately. There may be several concatenated lines, separated with newlines.</skos:scopeNote>
    <schema:rangeIncludes rdf:resource="http://www.w3.org/1999/02/22-rdf-syntax-ns#langString"/>
    <rdfs:label>thoroughfare (street address)</rdfs:label>
    <skos:example>Via Belenzani 19</skos:example>
  </rdf:Description>
  <rdf:Description rdf:about="http://data.businessgraph.io/ontology#isPersistent">
    <ebg:order rdf:datatype="http://www.w3.org/2001/XMLSchema#integer">54</ebg:order>
    <skos:scopeNote>Some registers “remove” identifiers when the object they relate to is no longer active, whereas the best practice is to make such identifiers Obsolete.</skos:scopeNote>
    <skos:definition>Whether identifiers can be removed from the register (e.g., when a company is dissolved): such are not persistent</skos:definition>
    <schema:rangeIncludes rdf:resource="http://www.w3.org/2001/XMLSchema#boolean"/>
    <schema:domainIncludes rdf:resource="http://data.businessgraph.io/ontology#IdentifierSystem"/>
    <rdfs:label>has persistent identifiers</rdfs:label>
    <rdfs:isDefinedBy rdf:resource="http://data.businessgraph.io/ontology#"/>
    <rdf:type rdf:resource="http://www.w3.org/2002/07/owl#DatatypeProperty"/>
  </rdf:Description>
  <rdf:Description rdf:about="http://data.businessgraph.io/ontology#ralCode">
    <ebg:order rdf:datatype="http://www.w3.org/2001/XMLSchema#integer">50</ebg:order>
    <skos:scopeNote>Used only for official registers.</skos:scopeNote>
    <skos:definition>GLEI RAL code for the identifier system.</skos:definition>
    <schema:rangeIncludes rdf:resource="http://www.w3.org/2001/XMLSchema#string"/>
    <schema:domainIncludes rdf:resource="http://data.businessgraph.io/ontology#IdentifierSystem"/>
    <rdfs:label>identifier system RAL code</rdfs:label>
    <rdfs:isDefinedBy rdf:resource="http://data.businessgraph.io/ontology#"/>
    <rdf:type rdf:resource="http://www.w3.org/2002/07/owl#DatatypeProperty"/>
  </rdf:Description>
  <rdf:Description rdf:about="http://purl.org/dc/terms/creator">
    <rdf:type rdf:resource="http://www.w3.org/2002/07/owl#ObjectProperty"/>
    <skos:example>Dun and Bradstreet issues DUNS numbers.</skos:example>
    <skos:example>http://www.registryagency.bg keeps both Trade Register http://brra.bg for companies, and Bulstat Register http://www.bulstat.bg/ for other entities</skos:example>
    <skos:example>GLEI Foundation (GLEIF) issues identifiers for the world-wide GLEI register (through its Local Operating Units, LOU).</skos:example>
    <schema:domainIncludes rdf:resource="http://data.businessgraph.io/ontology#IdentifierSystem"/>
    <skos:example>Web URLs are not issued by any central agency and there is no register to consult.</skos:example>
    <skos:definition>Agent that issues identifiers and then keeps them in a database (register), and who issued a specific identifier</skos:definition>
    <schema:domainIncludes rdf:resource="http://www.w3.org/ns/adms#Identifier"/>
    <skos:scopeNote>Many agencies keep several registries; this ontology doesn't distinguish between an identifier system and its register(s)</skos:scopeNote>
    <schema:rangeIncludes rdf:resource="http://schema.org/Person"/>
    <schema:rangeIncludes rdf:resource="http://schema.org/Organization"/>
    <skos:example>Companies House is the issuer for the official UK identifier system.</skos:example>
    <rdfs:label>issuer</rdfs:label>
    <ebg:order rdf:datatype="http://www.w3.org/2001/XMLSchema#integer">46</ebg:order>
    <skos:scopeNote>In many countries there is a single registry although in others, such as Spain and Germany, multiple registries exist. [rov:].</skos:scopeNote>
  </rdf:Description>
  <rdf:Description rdf:about="http://www.w3.org/ns/org#Role">
    <skos:scopeNote>Instances of this class describe the abstract role; to denote a specific instance of a person playing that role in a specific organization use an instance of org:Membership.</skos:scopeNote>
    <skos:definition>Denotes a role that a Person can take in an organization.</skos:definition>
    <rdfs:label>Role</rdfs:label>
    <rdf:type rdf:resource="http://www.w3.org/2000/01/rdf-schema#Class"/>
  </rdf:Description>
  <rdf:Description rdf:about="http://data.businessgraph.io/status/">
    <dct:publisher rdf:resource="http://businessgraph.io"/>
    <dct:creator rdf:resource="http://businessgraph.io"/>
    <rdfs:comment>Company status, e.g. active, inactive. Unfortunately different providers use different definitions</rdfs:comment>
    <rdfs:label>Company status</rdfs:label>
    <rdfs:isDefinedBy rdf:resource="http://data.businessgraph.io/ontology#"/>
    <rdf:type rdf:resource="http://www.w3.org/2004/02/skos/core#ConceptScheme"/>
  </rdf:Description>
  <rdf:Description rdf:about="http://data.businessgraph.io/ontology#webResource">
    <ebg:order rdf:datatype="http://www.w3.org/2001/XMLSchema#integer">64</ebg:order>
    <skos:example>http://opendata.government.bg/dataset/tbprobckn-pernctbp is the open data download site for BG TR.</skos:example>
    <rdfs:label>web resource</rdfs:label>
    <schema:rangeIncludes rdf:resource="http://data.businessgraph.io/ontology#WebResource"/>
    <rdf:type rdf:resource="http://www.w3.org/2002/07/owl#ObjectProperty"/>
    <skos:definition>Web resource associated with an identifier system.</skos:definition>
    <schema:domainIncludes rdf:resource="http://rdfs.org/ns/void#Dataset"/>
    <schema:domainIncludes rdf:resource="http://data.businessgraph.io/ontology#IdentifierSystem"/>
    <skos:example>https://brra.bg is the homepage of BG TR.</skos:example>
    <skos:example>https://kbopub.economie.fgov.be/kbopub/zoeknummerform.html is the search URL for BE Banque-Carrefour des Entreprises.</skos:example>
    <rdfs:isDefinedBy rdf:resource="http://data.businessgraph.io/ontology#"/>
  </rdf:Description>
  <rdf:Description rdf:about="http://data.businessgraph.io/ontology#isPublic">
    <skos:definition>whether identifiers from the system are available for public use: consulting, search or download.</skos:definition>
    <schema:rangeIncludes rdf:resource="http://www.w3.org/2001/XMLSchema#boolean"/>
    <skos:example>Italian (IT) company identifiers are public. Even though they are not published openly, they are available for a fee, and then can be used freely</skos:example>
    <schema:domainIncludes rdf:resource="http://data.businessgraph.io/ontology#IdentifierSystem"/>
    <rdfs:isDefinedBy rdf:resource="http://data.businessgraph.io/ontology#"/>
    <ebg:order rdf:datatype="http://www.w3.org/2001/XMLSchema#integer">56</ebg:order>
    <rdf:type rdf:resource="http://www.w3.org/2002/07/owl#DatatypeProperty"/>
    <skos:example>DUNS identifiers are not public, even though there are limited lookup services (e.g., https://www.dnb.com/duns-number/lookup.html). Dun and Bradstreet does not allow their use en-masse.</skos:example>
    <skos:scopeNote>Most public systems (but not all) will have some Publishers, and preferably some web resources.</skos:scopeNote>
    <rdfs:label>is public</rdfs:label>
  </rdf:Description>
  <rdf:Description rdf:about="http://www.w3.org/ns/org#role">
    <ebg:order rdf:datatype="http://www.w3.org/2001/XMLSchema#integer">106</ebg:order>
    <skos:definition>The role played by the officer in the membership</skos:definition>
    <schema:rangeIncludes rdf:resource="http://www.w3.org/ns/org#Role"/>
    <schema:domainIncludes rdf:resource="http://www.w3.org/ns/org#Membership"/>
    <rdfs:label>role</rdfs:label>
    <rdf:type rdf:resource="http://www.w3.org/2002/07/owl#ObjectProperty"/>
  </rdf:Description>
  <rdf:Description rdf:about="http://data.businessgraph.io/ontology#isImmutable">
    <ebg:order rdf:datatype="http://www.w3.org/2001/XMLSchema#integer">55</ebg:order>
    <skos:example>Some registers encode additional information within the identifier (e.g., some identifiers encode the economic sector of the company). In these cases the identifier changes when the extra information that is encoded changes (see “Dumb vs. Intelligent Identifiers” in Section 3.1.2.5).</skos:example>
    <skos:definition>whether identifiers can change</skos:definition>
    <schema:rangeIncludes rdf:resource="http://www.w3.org/2001/XMLSchema#boolean"/>
    <schema:domainIncludes rdf:resource="http://data.businessgraph.io/ontology#IdentifierSystem"/>
    <rdfs:label>has immutable identifiers</rdfs:label>
    <rdfs:isDefinedBy rdf:resource="http://data.businessgraph.io/ontology#"/>
    <rdf:type rdf:resource="http://www.w3.org/2002/07/owl#DatatypeProperty"/>
  </rdf:Description>
  <rdf:Description rdf:about="http://data.businessgraph.io/ontology#isStateOwned">
    <schema:rangeIncludes rdf:resource="http://www.w3.org/2001/XMLSchema#boolean"/>
    <rdf:type rdf:resource="http://www.w3.org/2002/07/owl#DatatypeProperty"/>
    <schema:domainIncludes rdf:resource="http://www.w3.org/ns/regorg#RegisteredOrganization"/>
    <skos:example>True for the Autonomous Province of Trento (local government).</skos:example>
    <rdfs:isDefinedBy rdf:resource="http://data.businessgraph.io/ontology#"/>
    <ebg:order rdf:datatype="http://www.w3.org/2001/XMLSchema#integer">6</ebg:order>
    <skos:definition>Whether this organisation is owned by the government, a government agency, community, city or other public entity.</skos:definition>
    <rdfs:label>is state owned</rdfs:label>
    <skos:example>True for the Norwegian company Statkraft (Norwegian state-owned company).</skos:example>
    <skos:example>False for SpazioDati (a private company).</skos:example>
    <skos:scopeNote>In many cases it's not possible to compute this attribute without access to the shareholder register, so it may be missing.</skos:scopeNote>
  </rdf:Description>
  <rdf:Description rdf:about="http://www.w3.org/ns/locn#postCode">
    <ebg:order rdf:datatype="http://www.w3.org/2001/XMLSchema#integer">39</ebg:order>
    <skos:scopeNote>If possible, a European postal code should correspond to the fixed values given in NUTS Downloads, so we can correlate it to a NUTS region.</skos:scopeNote>
    <skos:definition>Postal code of the address.</skos:definition>
    <rdfs:label>post code</rdfs:label>
    <schema:rangeIncludes rdf:resource="http://www.w3.org/2001/XMLSchema#string"/>
    <schema:domainIncludes rdf:resource="http://www.w3.org/ns/locn#Address"/>
    <rdf:type rdf:resource="http://www.w3.org/2002/07/owl#DatatypeProperty"/>
  </rdf:Description>
  <rdf:Description rdf:about="http://www.w3.org/ns/regorg#RegisteredOrganization">
    <skos:example>Banks and finance companies.</skos:example>
    <skos:example>All entities that trade stock or debt, investment vehicles, including mutual funds, pension funds and alternative investment vehicles constituted as corporate entities or collective investment agreements (including umbrella funds as well as funds under an umbrella structure, hedge funds, private equity funds, etc.).</skos:example>
    <skos:scopeNote>Registered organizations are the main entities that euBusinessGraph works with (the project is not concerned with  unregistered informal groups). The borderline between public organizations and commercial companies is not always clear-cut (a company may be partially owned by government, and e.g.  Public-Private-Partnerships are a prime example), so the project may deal with some organizations that are not companies. But for brevity and convenience we often call  them Companies [ebg:].</skos:scopeNote>
    <skos:example>All entities listed on an exchange.</skos:example>
    <skos:example>Counterparties to financial transactions.</skos:example>
    <skos:example>All financial intermediaries.</skos:example>
    <rdf:type rdf:resource="http://www.w3.org/2000/01/rdf-schema#Class"/>
    <skos:definition>An organization that gains legal entity status by the act of registration. Compare to org:FormalOrganization that applies to any legal entity, including those created by other legal means. Registered organizations are distinct from the broader concept of organizations, groups or, in some jurisdictions, sole traders. Many organizations exist that are not legal entities yet to the outside world they have staff, hierarchies, locations etc. Other organizations exist that are an umbrella for several legal entities (universities are often good examples of this) [rov:].  A legal person or structure that is organized under the laws of any jurisdiction [lei-elf:].</skos:definition>
    <skos:example>All entities that issue equity, debt or other securities for other capital structures.</skos:example>
    <rdfs:label>Registered Organization</rdfs:label>
    <skos:example>All entities under the purview of a financial regulator and their affiliates, subsidiaries and holding companies.</skos:example>
  </rdf:Description>
  <rdf:Description rdf:about="http://data.businessgraph.io/ontology#isSingleValued">
    <schema:domainIncludes rdf:resource="http://data.businessgraph.io/ontology#IdentifierSystem"/>
    <skos:definition>Whether each entity has only one identifier in the system</skos:definition>
    <skos:example>Official person names are single-valued, since each person has one official name (but that can change over time).</skos:example>
    <skos:example>Company IDs are single-valued in most national registers. If two companies merge, the recessive company ID is usually deprecated.</skos:example>
    <ebg:order rdf:datatype="http://www.w3.org/2001/XMLSchema#integer">53</ebg:order>
    <skos:example>Websites are not single-valued since a company may have several websites</skos:example>
    <skos:example>Stock exchange tickers are not single-valued, since a company may have several tickers for different kinds of its stock.</skos:example>
    <rdfs:label>is single-valued</rdfs:label>
    <rdfs:isDefinedBy rdf:resource="http://data.businessgraph.io/ontology#"/>
    <schema:rangeIncludes rdf:resource="http://www.w3.org/2001/XMLSchema#boolean"/>
    <rdf:type rdf:resource="http://www.w3.org/2002/07/owl#DatatypeProperty"/>
    <skos:scopeNote>Similar to owl:FunctionalProperty, and Wikidata Single Value constraint</skos:scopeNote>
  </rdf:Description>
  <rdf:Description rdf:about="http://schema.org/GeoCoordinates">
    <skos:definition>Geographic coordinates, eg of a geo-located address.</skos:definition>
    <rdfs:label>Geographic coordinates</rdfs:label>
    <rdf:type rdf:resource="http://www.w3.org/2000/01/rdf-schema#Class"/>
  </rdf:Description>
  <rdf:Description rdf:about="http://www.w3.org/2001/XMLSchema#date">
    <rdfs:label>Date</rdfs:label>
    <rdf:type rdf:resource="http://www.w3.org/2000/01/rdf-schema#Datatype"/>
  </rdf:Description>
  <rdf:Description rdf:about="http://data.businessgraph.io/ontology#isEnumerated">
    <ebg:order rdf:datatype="http://www.w3.org/2001/XMLSchema#integer">58</ebg:order>
    <skos:example>Websites are not enumerated</skos:example>
    <skos:example>Every official register is enumerated</skos:example>
    <skos:definition>Whether the system has an Issuer and issued identifiers are kept in a database (register)</skos:definition>
    <schema:rangeIncludes rdf:resource="http://www.w3.org/2001/XMLSchema#boolean"/>
    <schema:domainIncludes rdf:resource="http://data.businessgraph.io/ontology#IdentifierSystem"/>
    <rdfs:label>has enumerated identifiers</rdfs:label>
    <rdfs:isDefinedBy rdf:resource="http://data.businessgraph.io/ontology#"/>
    <rdf:type rdf:resource="http://www.w3.org/2002/07/owl#DatatypeProperty"/>
  </rdf:Description>
  <rdf:Description rdf:about="http://data.businessgraph.io/ontology#identifierWebResource">
    <skos:scopeNote>Specifies a template that can be used uniformly to build URLs for all identifiers in the system.</skos:scopeNote>
    <skos:example>'https://opencorporates.com/companies/{}.xml'  with MIME type 'application/xml'</skos:example>
    <schema:domainIncludes rdf:resource="http://data.businessgraph.io/ontology#IdentifierSystem"/>
    <skos:example>'https://opencorporates.com/companies/{}.rdf'  with MIME type 'application/rdf+xml'</skos:example>
    <ebg:order rdf:datatype="http://www.w3.org/2001/XMLSchema#integer">63</ebg:order>
    <skos:example>'https://opencorporates.com/companies/{}'      with MIME type 'text/html'</skos:example>
    <skos:definition>Web resource associated with an identifier system</skos:definition>
    <rdfs:isDefinedBy rdf:resource="http://data.businessgraph.io/ontology#"/>
    <schema:rangeIncludes rdf:resource="http://data.businessgraph.io/ontology#IdentifierWebResource"/>
    <rdfs:label>identifier web resource</rdfs:label>
    <rdf:type rdf:resource="http://www.w3.org/2002/07/owl#ObjectProperty"/>
    <skos:example>'https://opencorporates.com/companies/{}.json' with MIME type 'application/json'</skos:example>
  </rdf:Description>
  <rdf:Description rdf:about="http://schema.org/name">
    <ebg:order rdf:datatype="http://www.w3.org/2001/XMLSchema#integer">66</ebg:order>
    <schema:domainIncludes rdf:resource="http://data.businessgraph.io/ontology#WebResource"/>
    <skos:example>Company data</skos:example>
    <skos:definition>Name or short (generic) description of the resource</skos:definition>
    <skos:example>Homepage</skos:example>
    <schema:rangeIncludes rdf:resource="http://www.w3.org/1999/02/22-rdf-syntax-ns#langString"/>
    <skos:scopeNote>Provide this since it's useful to the user. Can provide it in several languages, in which case the language tag should be specified</skos:scopeNote>
    <skos:example>Search</skos:example>
    <rdfs:label>name</rdfs:label>
    <schema:rangeIncludes rdf:resource="http://www.w3.org/2001/XMLSchema#string"/>
    <rdf:type rdf:resource="http://www.w3.org/2002/07/owl#DatatypeProperty"/>
    <schema:domainIncludes rdf:resource="http://data.businessgraph.io/ontology#IdentifierWebResource"/>
    <skos:example>Download</skos:example>
  </rdf:Description>
  <rdf:Description rdf:about="http://www.w3.org/ns/org#member">
    <ebg:order rdf:datatype="http://www.w3.org/2001/XMLSchema#integer">104</ebg:order>
    <skos:definition>The officer that the membership is about</skos:definition>
    <schema:rangeIncludes rdf:resource="http://www.w3.org/ns/person#Person"/>
    <schema:domainIncludes rdf:resource="http://www.w3.org/ns/org#Membership"/>
    <rdfs:label>member</rdfs:label>
    <rdf:type rdf:resource="http://www.w3.org/2002/07/owl#ObjectProperty"/>
  </rdf:Description>
  <rdf:Description rdf:about="http://www.w3.org/ns/regorg#orgActivity">
    <skos:scopeNote>Only the most specific classification code(s) should be provided since we have a skos:broader hierarchy.</skos:scopeNote>
    <rdf:type rdf:resource="http://www.w3.org/2002/07/owl#ObjectProperty"/>
    <rdfs:label>economic activity</rdfs:label>
    <skos:scopeNote>Recorded using a controlled vocabulary: EC NACE 2. Values should be like nace:A, nace:42.50, etc</skos:scopeNote>
    <skos:scopeNote>More detailed national classifications could also useful (e.g. IT ATECO, UK SIC, BG NKID) but are not supported for now. Providers should drop eventual NACE National Extensions trailing digits.</skos:scopeNote>
    <skos:scopeNote>Values are taken from the euBusinessGraph NACE ConceptScheme. URL template: nace:([A-Z]|[0-9]{2}|[0-9]{2}\.[0-9]{1,2}). Providers must use exact codes of the specified form</skos:scopeNote>
    <skos:definition>Economic activity of the organization (NACE code)</skos:definition>
    <schema:domainIncludes rdf:resource="http://www.w3.org/ns/regorg#RegisteredOrganization"/>
    <schema:rangeIncludes rdf:resource="http://www.w3.org/2004/02/skos/core#Concept"/>
    <ebg:order rdf:datatype="http://www.w3.org/2001/XMLSchema#integer">10</ebg:order>
  </rdf:Description>
  <rdf:Description rdf:about="http://schema.org/expires">
    <ebg:order rdf:datatype="http://www.w3.org/2001/XMLSchema#integer">74</ebg:order>
    <skos:scopeNote>This may or may not be the same as the dissolution date of the company. Even when it is about the official registration, the two dates may differ, depending on business rules.</skos:scopeNote>
    <skos:definition>Date when the identifier expires (end date)</skos:definition>
    <schema:rangeIncludes rdf:resource="http://www.w3.org/2001/XMLSchema#date"/>
    <schema:domainIncludes rdf:resource="http://www.w3.org/ns/adms#Identifier"/>
    <rdfs:label>expires</rdfs:label>
    <rdf:type rdf:resource="http://www.w3.org/2002/07/owl#DatatypeProperty"/>
  </rdf:Description>
  <rdf:Description rdf:about="http://www.w3.org/ns/regorg#legalName">
    <ebg:order rdf:datatype="http://www.w3.org/2001/XMLSchema#integer">0</ebg:order>
    <schema:rangeIncludes rdf:resource="http://www.w3.org/1999/02/22-rdf-syntax-ns#langString"/>
    <rdfs:label>legal name</rdfs:label>
    <skos:example>CHRINON LTD</skos:example>
    <skos:example xml:lang="en">Ontotext</skos:example>
    <skos:scopeNote>A business may have more than one legal name, particularly in jurisdictions with more than one official language (e.g. Belgium). Some registries also treat a transliterated name as official (e.g. Онтотекст vs Ontotext) [ebg:]</skos:scopeNote>
    <skos:scopeNote>Provide a legal language tag (see [iana:] for a list) if possible.</skos:scopeNote>
    <skos:definition>The legal name of the business, i.e. official name of the company [ebg:]</skos:definition>
    <schema:domainIncludes rdf:resource="http://www.w3.org/ns/regorg#RegisteredOrganization"/>
    <skos:example xml:lang="it">PROGIENE 2.000 I PROFESSIONISTI DELL'IGIENE S.R.L. ENUNCIABILE ANCHE: PROGIENE 2.000 S.R.L.</skos:example>
    <skos:example xml:lang="bg">Онтотекст</skos:example>
    <rdf:type rdf:resource="http://www.w3.org/2002/07/owl#DatatypeProperty"/>
    <skos:scopeNote>Don't allow leading, trailing and two consecutive spaces.</skos:scopeNote>
  </rdf:Description>
  <rdf:Description rdf:about="http://data.businessgraph.io/ontology#isStartup">
    <ebg:order rdf:datatype="http://www.w3.org/2001/XMLSchema#integer">5</ebg:order>
    <skos:example>A special section of the IT Business Register http://startup.registroimprese.it/ includes pitch, sectors and business model of startups and innovative SMEs</skos:example>
    <skos:definition>Whether the company is a startup [ebg:]</skos:definition>
    <schema:rangeIncludes rdf:resource="http://www.w3.org/2001/XMLSchema#boolean"/>
    <schema:domainIncludes rdf:resource="http://www.w3.org/ns/regorg#RegisteredOrganization"/>
    <rdfs:label>is startup</rdfs:label>
    <rdfs:isDefinedBy rdf:resource="http://data.businessgraph.io/ontology#"/>
    <rdf:type rdf:resource="http://www.w3.org/2002/07/owl#DatatypeProperty"/>
  </rdf:Description>
  <rdf:Description rdf:about="http://data.businessgraph.io/ontology#WebResource">
    <skos:definition>URL complemented with name, language and MIME type(s) to specify what the URL is about</skos:definition>
    <rdfs:label>Web Resource</rdfs:label>
    <rdfs:isDefinedBy rdf:resource="http://data.businessgraph.io/ontology#"/>
    <rdf:type rdf:resource="http://www.w3.org/2000/01/rdf-schema#Class"/>
  </rdf:Description>
</rdf:RDF>
